@base <http://data.europa.eu/949/> .
@prefix : <http://data.europa.eu/949/> .
@prefix dcterms: <http://purl.org/dc/terms/> .
@prefix ns1: <http://www.w3.org/2003/06/sw-vocab-status/ns#> .
@prefix ns2: <http://www.w3.org/2004/02/skos/core#> .
@prefix ns3: <http://purl.org/dc/elements/1.1/> .
@prefix ns4: <http://creativecommons.org/ns#> .
@prefix owl: <http://www.w3.org/2002/07/owl#> .
@prefix rdf: <http://www.w3.org/1999/02/22-rdf-syntax-ns#> .
@prefix rdfs: <http://www.w3.org/2000/01/rdf-schema#> .
@prefix xsd: <http://www.w3.org/2001/XMLSchema#> .

<IdPhoneErtmsRadioBlockCenter> a owl:DatatypeProperty ;
    rdfs:label "ID and phone number of ERTMS/ETCS Radio Block Center"@en ;
    <rinfIndex> "1.1.1.3.2.17",
        "1.2.1.1.1.17" ;
    dcterms:created "2023-03-14"^^xsd:date ;
    rdfs:comment "Unique RBC identification (NID_C+NID_RBC) and calling number (NID_RADIO) as defined in the specification referenced in Appendix A-1, index [C]."@en ;
    rdfs:domain [ a owl:Class ;
            owl:unionOf ( <SubsetWithCommonCharacteristics> <Track> ) ] ;
    rdfs:isDefinedBy <> ;
    rdfs:range xsd:string ;
    ns1:term_status "stable" .

<TSIMagneticFields> a owl:FunctionalProperty,
        owl:ObjectProperty ;
    rdfs:label "Existence and TSI compliance of rules for magnetic fields emitted by a vehicle"@en ;
    <XMLName> "CEI_TSIMagneticFields" ;
    <inSkosConceptScheme> <concepts/tsi-existence-and-compliances/TSIExistenceAndCompliances> ;
    <rinfIndex> "1.1.1.3.9.1",
        "1.2.1.1.8.1" ;
    dcterms:created "2021-08-09"^^xsd:date ;
    dcterms:modified "2024-04-25"^^xsd:date ;
    rdfs:comment "Indication whether rules exist and are compliant with the TSI."@en ;
    rdfs:domain [ a owl:Class ;
            owl:unionOf ( <SubsetWithCommonCharacteristics> <Track> ) ] ;
    rdfs:isDefinedBy <> ;
    rdfs:range ns2:Concept ;
    ns1:term_status "stable" .

<TSITractionHarmonics> a owl:FunctionalProperty,
        owl:ObjectProperty ;
    rdfs:label "Existence and TSI compliance of limits in harmonics in the traction current of vehicles"@en ;
    <XMLName> "CEI_TSITractionHarmonics" ;
    <inSkosConceptScheme> <concepts/tsi-existence-and-compliances/TSIExistenceAndCompliances> ;
    <rinfIndex> "1.1.1.3.9.2",
        "1.2.1.1.8.2" ;
    dcterms:created "2021-08-09"^^xsd:date ;
    dcterms:modified "2024-04-25"^^xsd:date ;
    rdfs:comment "Indication whether rules exist and are compliant with the TSI."@en ;
    rdfs:domain [ a owl:Class ;
            owl:unionOf ( <SubsetWithCommonCharacteristics> <Track> ) ] ;
    rdfs:isDefinedBy <> ;
    rdfs:range ns2:Concept ;
    ns1:term_status "stable" .

<accelerationLevelCrossing> a owl:DatatypeProperty,
        owl:FunctionalProperty ;
    rdfs:label "Acceleration allowed near level crossing"@en ;
    <XMLName> "IHS_AccelerationLevelCrossing" ;
    <rinfIndex> "1.1.1.1.7.3" ;
    dcterms:created "2021-08-03"^^xsd:date ;
    dcterms:modified "2024-01-08"^^xsd:date ;
    rdfs:comment "Existence of limit for acceleration of train if stopping or recovering speed close to a level crossing expressed in a specific reference acceleration curve."@en ;
    rdfs:domain [ a owl:Class ;
            owl:unionOf ( <SubsetWithCommonCharacteristics> <Track> ) ] ;
    rdfs:isDefinedBy <> ;
    rdfs:range xsd:string ;
    ns1:term_status "stable" .

<additionalBrakingInformationDocument> a owl:ObjectProperty ;
    rdfs:label "Documents available by the IM relating to braking performance"@en ;
    <XMLName> "CBP_BrakePerfDocRef" ;
    <rinfIndex> "1.1.1.3.11.3" ;
    <usedInRCCCalculations> true ;
    dcterms:created "2020-08-24"^^xsd:date ;
    dcterms:modified "2024-04-23"^^xsd:date ;
    rdfs:comment "Electronic document available in two EU languages from the IM stored by the Agency providing additional information as defined in point (2) of point 4.2.2.6.2 of TSI OPE."@en ;
    rdfs:domain [ a owl:Class ;
            owl:unionOf ( <SubsetWithCommonCharacteristics> <Track> ) ] ;
    rdfs:isDefinedBy <> ;
    rdfs:range <Document> ;
    ns1:term_status "stable" ;
    ns2:changeNote "Change from datatype property to object property in order to point to the class Document (reference document)"@en .

<areaBoardingAid> a owl:DatatypeProperty,
        owl:FunctionalProperty ;
    rdfs:label "Range of use of the platform boarding aid"@en ;
    <XMLName> "IPL_AreaBoardingAid" ;
    <rinfIndex> "1.2.1.0.6.7" ;
    <unitOfMeasure> <http://qudt.org/vocab/unit/MilliM> ;
    dcterms:created "2021-08-02"^^xsd:date ;
    dcterms:modified "2023-01-20"^^xsd:date ;
    rdfs:comment "Information of the train access level for which the boarding aid can be used. Data is presented as the vertical difference that is overcome by the platform boarding aid in millimetres. The value “0” means that the platform is not equipped with a platform boarding aid."@en ;
    rdfs:domain <PlatformEdge> ;
    rdfs:isDefinedBy <> ;
    rdfs:range xsd:integer ;
    ns1:term_status "stable" .

<assistanceStartingTrain> a owl:DatatypeProperty,
        owl:FunctionalProperty ;
    rdfs:label "Existence of platform assistance for starting train"@en ;
    <XMLName> "IPL_AssistanceStartingTrain" ;
    <rinfIndex> "1.2.1.0.6.6" ;
    dcterms:created "2021-08-02"^^xsd:date ;
    dcterms:modified "2021-08-02"^^xsd:date ;
    rdfs:comment "Indication of existence of equipment or staff supporting the train crew in starting the train."@en ;
    rdfs:domain <PlatformEdge> ;
    rdfs:isDefinedBy <> ;
    rdfs:range xsd:boolean ;
    ns1:term_status "stable" .

<atoCommunicationSystem> a owl:ObjectProperty ;
    rdfs:label "ATO communication system"@en ;
    <rinfIndex> "1.1.1.3.13.3",
        "1.2.1.1.10.3" ;
    dcterms:created "2023-03-14"^^xsd:date ;
    rdfs:comment "Supported ATO communication systems from trackside."@en ;
    rdfs:domain [ a owl:Class ;
            owl:unionOf ( <SubsetWithCommonCharacteristics> <Track> ) ] ;
    rdfs:isDefinedBy <> ;
    rdfs:range ns2:Concept ;
    ns1:term_status "unstable" .

<atoErrorCorrectionsOnboard> a owl:DatatypeProperty ;
    rdfs:label "ATO error corrections required for the on-board"@en ;
    <rinfIndex> "1.1.1.3.13.4" ;
    dcterms:created "2023-03-14"^^xsd:date ;
    rdfs:comment "List of unacceptable errors impacting the IM network that are required to be solved in the on-board according to the CCS TSI point 7.2.10.3 specification maintenance point."@en ;
    rdfs:domain [ a owl:Class ;
            owl:unionOf ( <SubsetWithCommonCharacteristics> <Track> ) ] ;
    rdfs:isDefinedBy <> ;
    rdfs:range xsd:anyURI ;
    ns1:term_status "stable" .

<atoGradeAutomation> a owl:ObjectProperty ;
    rdfs:label "ATO Grade of Automation"@en ;
    <rinfIndex> "1.1.1.3.13.1",
        "1.2.1.1.10.1" ;
    dcterms:created "2023-03-14"^^xsd:date ;
    rdfs:comment "ATO grade of automation installed lineside."@en ;
    rdfs:domain [ a owl:Class ;
            owl:unionOf ( <SubsetWithCommonCharacteristics> <Track> ) ] ;
    rdfs:isDefinedBy <> ;
    rdfs:range ns2:Concept ;
    ns1:term_status "unstable" .

<atoSystemVersion> a owl:ObjectProperty ;
    rdfs:label "ATO System version"@en ;
    <rinfIndex> "1.1.1.3.13.2",
        "1.2.1.1.10.2" ;
    dcterms:created "2023-03-14"^^xsd:date ;
    rdfs:comment "ATO system version according to the specification referenced in Appendix A-1, index [C]."@en ;
    rdfs:domain [ a owl:Class ;
            owl:unionOf ( <SubsetWithCommonCharacteristics> <Track> ) ] ;
    rdfs:isDefinedBy <> ;
    rdfs:range ns2:Concept ;
    ns1:term_status "unstable" .

<automaticDroppingDeviceRequired> a owl:DatatypeProperty,
        owl:FunctionalProperty ;
    rdfs:label "Automatic dropping device required"@en ;
    <XMLName> "ERS_AutoDropRequired" ;
    <rinfIndex> "1.1.1.2.5.3" ;
    <usedInRCCCalculations> true ;
    dcterms:created "2020-08-25"^^xsd:date ;
    dcterms:modified "2021-09-12"^^xsd:date ;
    rdfs:comment "Indication of whether an automatic dropping device (ADD) required on the vehicle."@en ;
    rdfs:domain [ a owl:Class ;
            owl:unionOf ( <SubsetWithCommonCharacteristics> <Track> ) ] ;
    rdfs:isDefinedBy <> ;
    rdfs:range xsd:boolean ;
    ns1:term_status "stable" .

<bigMetalMass> a owl:DatatypeProperty ;
    rdfs:label "Big Metal Mass"@en ;
    <rinfIndex> "1.1.1.3.2.18",
        "1.2.1.1.1.18" ;
    dcterms:created "2023-03-14"^^xsd:date ;
    dcterms:modified "2024-01-08"^^xsd:date ;
    rdfs:comment "Indication of existence of metal mass in the vicinity of the location, susceptible of perturbating the reading of balises by the on-board system."@en ;
    rdfs:domain [ a owl:Class ;
            owl:unionOf ( <SubsetWithCommonCharacteristics> <Track> ) ] ;
    rdfs:isDefinedBy <> ;
    rdfs:range xsd:boolean ;
    ns1:term_status "stable" .

<bridge> a owl:DatatypeProperty ;
    rdfs:label "Is bridge"@en ;
    rdfs:domain <Track> ;
    rdfs:isDefinedBy <> ;
    rdfs:range xsd:boolean ;
    ns1:term_status "stable" ;
    ns2:definition "Whether or not a track is associated with a bridge."@en .

<canonicalURI> a owl:AnnotationProperty ;
    rdfs:label "Canonical URI"@en ;
    dcterms:created "2022-12-13"^^xsd:date ;
    dcterms:modified "2024-02-06"^^xsd:date ;
    rdfs:comment """The canonical URI is defined for each instance of an Infrastructure element, e.g. section of line, operational point, track, tunnel, siding.
Objects of the infrastructure generated through RML mappings include (when provided) their validity start and end dates. With its identifier, plus all identifiers of its "parent" elements, and its validity dates, a hash URI is generated.
The canonical URI is the element's URI with its identifiers and without the validity dates. All of the hash URIs of an element point to its canonical URI.
Additionally, SoLs point to the canonical URIs of their start OP and end OP."""@en ;
    rdfs:domain <InfrastructureObject> ;
    rdfs:isDefinedBy <> ;
    rdfs:range xsd:anyURI .

<cantDeficiency> a owl:DatatypeProperty,
        owl:FunctionalProperty ;
    rdfs:label "Cant deficiency"@en ;
    <XMLName> "ITP_CantDeficiency" ;
    <rinfIndex> "1.1.1.1.4.2" ;
    <unitOfMeasure> <http://qudt.org/vocab/unit/MilliM> ;
    <usedInRCCCalculations> true ;
    dcterms:created "2020-08-24"^^xsd:date ;
    dcterms:modified "2021-09-10"^^xsd:date ;
    rdfs:comment "Maximum cant deficiency expressed in millimetres defined as difference between the applied cant and a higher equilibrium cant the line has been designed for."@en ;
    rdfs:domain [ a owl:Class ;
            owl:unionOf ( <SubsetWithCommonCharacteristics> <Track> ) ] ;
    rdfs:isDefinedBy <> ;
    rdfs:range xsd:integer ;
    ns1:term_status "stable" .

<cantDeficiencyBasicSSP> a owl:ObjectProperty ;
    rdfs:label "Cant Deficiency used for the basic SSP"@en ;
    <rinfIndex> "1.1.1.3.2.14",
        "1.2.1.1.1.14" ;
    dcterms:created "2023-03-14"^^xsd:date ;
    dcterms:modified "2024-01-08"^^xsd:date ;
    rdfs:comment """Essential information for drivers of trains with a worse (lower) tolerated cant deficiency than those for which the ETCS trackside provides SSP (Static Speed Profiles) in conjunction with  parameter "Other Cant Deficiency train categories for which the ETCS trackside is configured to provide SSP".
According to the specification referenced in Appendix A-1, index [C]."""@en ;
    rdfs:domain [ a owl:Class ;
            owl:unionOf ( <SubsetWithCommonCharacteristics> <Track> ) ] ;
    rdfs:isDefinedBy <> ;
    rdfs:range ns2:Concept ;
    ns1:term_status "stable" .

<compatibilityProcedureDocument> a owl:ObjectProperty ;
    rdfs:label "Document with the procedure(s) for static and dynamic route compatibility checks"@en ;
    <XMLName> "IPP_StructureCheckDocRef" ;
    <rinfIndex> "1.1.1.1.2.4.4" ;
    <usedInRCCCalculations> true ;
    dcterms:created "2023-03-14"^^xsd:date ;
    dcterms:modified "2024-04-23"^^xsd:date ;
    rdfs:comment """Electronic document available in two EU languages from the IM stored by the Agency with:
- precise procedures for the static and dynamic route compatibility checks;
Or
- relevant information for carrying out the checks for specific structures."""@en ;
    rdfs:domain [ a owl:Class ;
            owl:unionOf ( <SubsetWithCommonCharacteristics> <Track> ) ] ;
    rdfs:isDefinedBy <> ;
    rdfs:range <Document> ;
    ns1:term_status "stable" ;
    ns2:changeNote "Change from datatype property to object property in order to point to the class Document (reference document)"@en .

<complianceInfTsi> a owl:DatatypeProperty,
        owl:FunctionalProperty ;
    rdfs:label "Compliance of the tunnel with TSI INF"@en ;
    <XMLName> "ITU_TSITunnel" ;
    <rinfIndex> "1.1.1.1.8.8.1" ;
    dcterms:created "2021-08-03"^^xsd:date ;
    dcterms:modified "2024-01-08"^^xsd:date ;
    rdfs:comment "Compliance of the tunnel with TSI INF at the maximum permitted speed."@en ;
    rdfs:domain <Tunnel> ;
    rdfs:isDefinedBy <> ;
    rdfs:range xsd:boolean ;
    ns1:term_status "stable" .

<conditionalRegenerativeBrake> a owl:DatatypeProperty ;
    rdfs:label "Permission for regenerative braking"@en ;
    <XMLName> "ECS_RegenerativeBraking" ;
    <rinfIndex> "1.1.1.2.2.4" ;
    <usedInRCCCalculations> true ;
    dcterms:created "2020-08-24"^^xsd:date ;
    dcterms:modified "2023-01-20"^^xsd:date ;
    rdfs:comment "Indication whether regenerative braking is permitted, not permitted, or permitted under specific conditions."@en ;
    rdfs:domain <ContactLineSystem> ;
    rdfs:isDefinedBy <> ;
    rdfs:range xsd:boolean ;
    ns1:term_status "stable" .

<conditionsAppliedRegenerativeBraking> a owl:DatatypeProperty ;
    rdfs:label "Conditions applying in regards to regenerative braking"@en ;
    <appendixD2Index> "3.3.7" ;
    <rinfIndex> "1.1.1.2.2.4.1" ;
    dcterms:created "2022-11-10"^^xsd:date ;
    dcterms:modified "2023-03-14"^^xsd:date ;
    dcterms:source <https://eur-lex.europa.eu/eli/reg_impl/2019/773/oj>,
        <https://eur-lex.europa.eu/legal-content/EN/TXT/HTML/?uri=CELEX:32019R0777&from=EN> ;
    rdfs:comment "Name and/or reference of the document specifying the conditions applying in regards to regenerative braking."@en ;
    rdfs:domain <ContactLineSystem> ;
    rdfs:isDefinedBy <> ;
    rdfs:range xsd:anyURI ;
    ns1:term_status "stable" .

<conditionsChargingElectricEnergyStorage> a owl:DatatypeProperty ;
    rdfs:label "Permitted conditions for charging electric energy storage for traction purposes at standstill"@en ;
    <rinfIndex> "1.2.1.0.7.2" ;
    dcterms:created "2023-03-14"^^xsd:date ;
    rdfs:comment "Conditions set by IMs according to a standardised document."@en ;
    rdfs:domain <ContactLineSystem> ;
    rdfs:isDefinedBy <> ;
    rdfs:range xsd:anyURI ;
    ns1:term_status "stable" .

<conditionsSwitchClassBSystems> a owl:DatatypeProperty ;
    rdfs:label "Special technical conditions required to switch over between ERTMS/ETCS and Class B systems"@en ;
    <appendixD2Index> "3.4.3" ;
    <rinfIndex> "1.1.1.3.8.3",
        "1.2.1.1.7.3" ;
    dcterms:created "2022-10-28"^^xsd:date ;
    dcterms:modified "2023-03-14"^^xsd:date ;
    dcterms:source <https://eur-lex.europa.eu/eli/reg_impl/2019/773/oj> ;
    rdfs:comment "Name and/or reference of the document specifying the Special technical conditions required to switch over between ERTMS/ETCS and Class B systems."@en ;
    rdfs:domain [ a owl:Class ;
            owl:unionOf ( <SubsetWithCommonCharacteristics> <Track> ) ] ;
    rdfs:isDefinedBy <> ;
    rdfs:range xsd:anyURI ;
    ns1:term_status "stable" .

<conditionsSwitchTrainProtectionSystems> a owl:DatatypeProperty ;
    rdfs:label "Special conditions to switch over between different class B train protection, control and warning systems"@en ;
    <appendixD2Index> "3.4.2" ;
    <rinfIndex> "1.1.1.3.8.1.1",
        "1.2.1.1.7.1.1" ;
    dcterms:created "2022-10-28"^^xsd:date ;
    dcterms:source <https://eur-lex.europa.eu/eli/reg_impl/2019/773/oj> ;
    rdfs:comment "Conditions to switch over between different class B train protection, control and warning systems."@en ;
    rdfs:domain [ a owl:Class ;
            owl:unionOf ( <SubsetWithCommonCharacteristics> <Track> ) ] ;
    rdfs:isDefinedBy <> ;
    rdfs:range xsd:anyURI ;
    ns1:term_status "stable" .

<conditionsUseReflectivePlates> a owl:ObjectProperty ;
    rdfs:label "Conditions for use of reflective plates"@en ;
    <rinfIndex> "1.1.1.1.7.12.1" ;
    dcterms:created "2023-03-14"^^xsd:date ;
    rdfs:comment "Details of any conditions for using the reflective plates on freight corridors. Specific case for Portugal and Spain until 1.1.2025 and Belgium and France until 1.1.2026."@en ;
    rdfs:domain [ a owl:Class ;
            owl:unionOf ( <SubsetWithCommonCharacteristics> <Track> ) ] ;
    rdfs:isDefinedBy <> ;
    rdfs:range ns2:Concept ;
    ns1:term_status "unstable" .

<contactLineSystem> a owl:ObjectProperty ;
    rdfs:label "Contact line system"@en ;
    dcterms:created "2020-08-24"^^xsd:date ;
    dcterms:modified "2021-09-11"^^xsd:date ;
    rdfs:comment "Contact line system present in the section of line."@en ;
    rdfs:domain [ a owl:Class ;
            owl:unionOf ( <SubsetWithCommonCharacteristics> <Track> ) ] ;
    rdfs:isDefinedBy <> ;
    rdfs:range <ContactLineSystem> ;
    ns1:term_status "stable" .

<contactLineSystemType> a owl:ObjectProperty ;
    rdfs:label "Type of contact line system"@en ;
    <XMLName> "ECS_SystemType" ;
    <inSkosConceptScheme> <concepts/contact-line-systems/ContactLineSystems> ;
    <rinfIndex> "1.1.1.2.2.1.1" ;
    <usedInRCCCalculations> true ;
    dcterms:created "2021-08-06"^^xsd:date ;
    dcterms:modified "2021-08-06"^^xsd:date ;
    rdfs:comment "Indication of the type of the contact line system."@en ;
    rdfs:domain <ContactLineSystem> ;
    rdfs:isDefinedBy <> ;
    rdfs:range ns2:Concept ;
    ns1:term_status "stable" .

<contactStripMaterial> a owl:ObjectProperty ;
    rdfs:label "Permitted contact strip material"@en ;
    <XMLName> "EPA_StripMaterial" ;
    <eratvIndex> "4.10.10" ;
    <inSkosConceptScheme> <concepts/contact-strip-materials/ContactStripMaterials> ;
    <rinfIndex> "1.1.1.2.3.4" ;
    <usedInRCCCalculations> true ;
    dcterms:created "2020-08-25"^^xsd:date ;
    dcterms:modified "2021-09-12"^^xsd:date ;
    rdfs:comment "Indication of which contact strip materials are permitted to be used."@en ;
    rdfs:domain [ a owl:Class ;
            owl:unionOf ( <SubsetWithCommonCharacteristics> <Track> <VehicleType> ) ] ;
    rdfs:isDefinedBy <> ;
    rdfs:range ns2:Concept ;
    ns1:term_status "stable" .

<contactStripMaterialMetallicContent> a owl:DatatypeProperty ;
    rdfs:label "Contact strip material metallic content"@en ;
    <XMLName> "EPA_StripMaterial" ;
    <rinfIndex> "1.1.1.2.3.4" ;
    <usedInRCCCalculations> true ;
    dcterms:created "2023-01-25"^^xsd:date ;
    rdfs:comment "In case that the value of the property era:contactStripMaterial is \"impregnated carbon\", it is the metallic content in % (this value must be added). This is the maximum percentage allowed."@en ;
    rdfs:domain [ a owl:Class ;
            owl:unionOf ( <SubsetWithCommonCharacteristics> <Track> ) ] ;
    rdfs:isDefinedBy <> ;
    rdfs:range xsd:integer ;
    ns1:term_status "stable" .

<crossSectionArea> a owl:DatatypeProperty,
        owl:FunctionalProperty ;
    rdfs:label "Cross section area"@en ;
    <XMLName> "ITU_CrossSectionArea" ;
    <rinfIndex> "1.1.1.1.8.8" ;
    <unitOfMeasure> <http://qudt.org/vocab/unit/M2> ;
    dcterms:created "2021-08-03"^^xsd:date ;
    dcterms:modified "2021-08-03"^^xsd:date ;
    rdfs:comment "Smallest cross section area in square metres of the tunnel."@en ;
    rdfs:domain <Tunnel> ;
    rdfs:isDefinedBy <> ;
    rdfs:range xsd:integer ;
    ns1:term_status "stable" .

<currentLimitationRequired> a owl:DatatypeProperty ;
    rdfs:label "Current or power limitation on board required"@en ;
    <XMLName> "ERS_PowerLimitOnBoard" ;
    <rinfIndex> "1.1.1.2.5.1" ;
    <usedInRCCCalculations> true ;
    dcterms:created "2020-08-25"^^xsd:date ;
    dcterms:modified "2021-09-12"^^xsd:date ;
    rdfs:comment "Indication of whether an on board current or power limitation function on vehicles is required."@en ;
    rdfs:domain <ContactLineSystem> ;
    rdfs:isDefinedBy <> ;
    rdfs:range xsd:boolean ;
    ns1:term_status "stable" .

<dNvovtrp> a owl:DatatypeProperty ;
    rdfs:label "D_NVOVTRP"@en ;
    <appendixD3Index> "1.5.5" ;
    <rinfIndex> "1.1.1.3.2.16.5",
        "1.2.1.1.1.16.5" ;
    dcterms:created "2022-11-07"^^xsd:date ;
    dcterms:modified "2024-01-08"^^xsd:date ;
    rdfs:comment """Maximum distance for overriding the train trip in metres
According to the specification referenced in Appendix A-1, index [C]. 
In Subset 26, chapter 7. 7.5.1.15 D_NVOVTRP https://www.era.europa.eu/sites/default/files/filesystem/ertms/ccs_tsi_annex_a_-_mandatory_specifications/set_of_specifications_3_etcs_b3_r2_gsm-r_b1/index004_-_subset-026_v360.zip."""@en ;
    rdfs:domain [ a owl:Class ;
            owl:unionOf ( <SubsetWithCommonCharacteristics> <Track> ) ] ;
    rdfs:isDefinedBy <> ;
    rdfs:range xsd:integer ;
    ns1:term_status "stable" .

<dNvpotrp> a owl:DatatypeProperty ;
    rdfs:label "D_NVPOTRP"@en ;
    <appendixD3Index> "1.5.7" ;
    <rinfIndex> "1.1.1.3.2.16.7",
        "1.2.1.1.1.16.7 " ;
    dcterms:created "2022-11-07"^^xsd:date ;
    dcterms:modified "2023-03-14"^^xsd:date ;
    rdfs:comment """Maximum distance for reversing in Post Trip mode  in metres. 
According to the specification referenced in Appendix A-1, index [C]. 
In https://www.era.europa.eu/sites/default/files/filesystem/ertms/ccs_tsi_annex_a_-_mandatory_specifications/set_of_specifications_3_etcs_b3_r2_gsm-r_b1/index004_-_subset-026_v360.zip
 Subset 26, chapter 7. 7.5.1.16 D_NVPOTRP."""@en ;
    rdfs:domain [ a owl:Class ;
            owl:unionOf ( <SubsetWithCommonCharacteristics> <Track> ) ] ;
    rdfs:isDefinedBy <> ;
    rdfs:range xsd:integer ;
    ns1:term_status "stable" .

<dNvroll> a owl:DatatypeProperty ;
    rdfs:label "D_NVROLL"@en ;
    <appendixD3Index> "1.5.1" ;
    <rinfIndex> "1.1.1.3.2.16.1",
        "1.2.1.1.1.16.1 " ;
    dcterms:created "2022-11-07"^^xsd:date ;
    dcterms:modified "2023-03-14"^^xsd:date ;
    rdfs:comment """Parameter used by the ETCS on-board to supervise the distance allowed to be travelled under the roll-away protection and the reverse movement protection, in metres.
According to the specification referenced in Appendix A-1, index [C].
In https://www.era.europa.eu/sites/default/files/filesystem/ertms/ccs_tsi_annex_a_-_mandatory_specifications/set_of_specifications_3_etcs_b3_r2_gsm-r_b1/index004_-_subset-026_v360.zip
 Subset 26, chapter 7. 7.5.1.17 D_NVROLL."""@en ;
    rdfs:domain [ a owl:Class ;
            owl:unionOf ( <SubsetWithCommonCharacteristics> <Track> ) ] ;
    rdfs:isDefinedBy <> ;
    rdfs:range xsd:integer ;
    ns1:term_status "stable" .

<dataRadioCompatible> a owl:ObjectProperty ;
    rdfs:label "Radio system compatibility data"@en ;
    <XMLName> "CRG_RadioCompData" ;
    <eratvIndex> "4.13.2.8" ;
    <inSkosConceptScheme> <concepts/radio-system-compatibilities-data/RadioSystemCompatibilitiesData> ;
    <rinfIndex> "1.1.1.3.3.10",
        "1.2.1.1.2.10" ;
    dcterms:created "2020-08-31"^^xsd:date ;
    dcterms:modified "2021-09-12"^^xsd:date ;
    rdfs:comment "Radio requirements used for demonstrating technical compatibility data."@en ;
    rdfs:domain [ a owl:Class ;
            owl:unionOf ( <SubsetWithCommonCharacteristics> <Track> <VehicleType> ) ] ;
    rdfs:isDefinedBy <> ;
    rdfs:range ns2:Concept ;
    ns1:term_status "stable" .

<demonstrationENE> a owl:DatatypeProperty ;
    rdfs:label "EI declaration of demonstration (as defined Recommendation 2014/881/EU) for track relating to compliance with the requirements from TSIs applicable to energy subsystem"@en ;
    <XMLName> "EDE_EIDemonstration" ;
    <rinfIndex> "1.1.1.2.1.2" ;
    dcterms:created "2021-08-08"^^xsd:date ;
    dcterms:modified "2024-01-08"^^xsd:date ;
    rdfs:comment "Unique number for EI declarations following the same format requirements as specified for EC declarations in Annex VII of Commission Implementing Regulation (EU) 2019/250." ;
    rdfs:domain [ a owl:Class ;
            owl:unionOf ( <SubsetWithCommonCharacteristics> <Track> ) ] ;
    rdfs:range xsd:string ;
    ns1:term_status "stable" .

<demonstrationINF> a owl:DatatypeProperty ;
    rdfs:label "EI declaration of demonstration (as defined Commission 2014/881/EU) for track relating to compliance with the requirements from TSIs applicable to infrastructure subsystem"@en ;
    <XMLName> "IDE_EIDemonstration" ;
    <rinfIndex> "1.1.1.1.1.2",
        "1.2.1.0.1.2",
        "1.2.2.0.1.2" ;
    dcterms:created "2021-08-03"^^xsd:date ;
    dcterms:modified "2024-01-08"^^xsd:date ;
    rdfs:comment """Unique number for EI declarations following the same format requirements as specified for EC declarations in Annex VII of Commission Implementing Regulation (EU) 2019/250.
In https://eur-lex.europa.eu/legal-content/EN/TXT/HTML/?uri=CELEX:32019R0777&from=EN"""@en ;
    rdfs:domain [ a owl:Class ;
            owl:unionOf ( <Siding> <Track> ) ] ;
    rdfs:isDefinedBy <> ;
    rdfs:range xsd:string ;
    ns1:term_status "stable" .

<demonstrationSRT> a owl:DatatypeProperty ;
    rdfs:label "EI declaration of demonstration (as defined in Recommendation 2014/881/EU) relating to compliance with the requirements from TSIs applicable to railway tunnel"@en ;
    <XMLName> "ITU_EIDemonstration" ;
    <rinfIndex> "1.1.1.1.8.6",
        "1.2.1.0.5.4",
        "1.2.2.0.5.4" ;
    dcterms:created "2021-08-03"^^xsd:date ;
    dcterms:modified "2024-01-08"^^xsd:date ;
    rdfs:comment "Unique number for EI declarations following the same format requirements as specified for EC declarations in Annex VII of Commission Implementing Regulation (EU) 2019/250."@en ;
    rdfs:domain <Tunnel> ;
    rdfs:isDefinedBy <> ;
    rdfs:range xsd:string ;
    ns1:term_status "stable" .

<dieselThermalAllowed> a owl:DatatypeProperty,
        owl:FunctionalProperty ;
    rdfs:label "Diesel or other thermal traction allowed"@en ;
    <XMLName> "ITU_DieselThermAllowed" ;
    <rinfIndex> "1.2.1.0.5.9" ;
    dcterms:created "2021-08-09"^^xsd:date ;
    dcterms:modified "2021-08-09"^^xsd:date ;
    rdfs:comment "Indication whether it is allowed to use diesel or other thermal traction in the tunnel."@en ;
    rdfs:domain <Tunnel> ;
    rdfs:isDefinedBy <> ;
    rdfs:range xsd:boolean ;
    ns1:term_status "stable" .

<digitalSchematicOverview> a owl:DatatypeProperty ;
    rdfs:label "Digital schematic overview"@en ;
    <rinfIndex> "1.2.0.0.0.7.2" ;
    dcterms:created "2023-03-14"^^xsd:date ;
    rdfs:comment "Diagrammatic representation of the operational point in Well Known Text polyline"@en ;
    rdfs:domain <OperationalPoint> ;
    rdfs:isDefinedBy <> ;
    rdfs:range <http://www.opengis.net/ont/geosparql#wktLiteral> ;
    ns1:term_status "stable" .

<distSignToPhaseEnd> a owl:DatatypeProperty,
        owl:FunctionalProperty ;
    rdfs:label "Distance between signboard and phase separation ending"@en ;
    <XMLName> "EOS_DistSignToPhaseEnd" ;
    <rinfIndex> "1.1.1.2.4.3" ;
    <unitOfMeasure> <http://qudt.org/vocab/unit/M> ;
    <usedInRCCCalculations> true ;
    dcterms:created "2021-08-08"^^xsd:date ;
    dcterms:modified "2021-09-12"^^xsd:date ;
    rdfs:comment """Specific for route compatibility check on French network.
Distance between the signboard authorizing the driver to ‘raise pantograph’ or ‘close the circuit breaker’ after passing the phase separation and the end of the phase separation section."""@en ;
    rdfs:domain [ a owl:Class ;
            owl:unionOf ( <SubsetWithCommonCharacteristics> <Track> ) ] ;
    rdfs:isDefinedBy <> ;
    rdfs:range xsd:integer ;
    ns1:term_status "stable" .

<documentRestrictionPositionContactLineSeparation> a owl:DatatypeProperty ;
    rdfs:label "Document with restriction related to the position of Multiple Traction unit(s) to comply with contact line separation"@en ;
    <rinfIndex> "1.1.1.2.5.5" ;
    dcterms:created "2023-03-14"^^xsd:date ;
    rdfs:comment "Name and/or reference of the document specifying the restriction(s) related to the position of Multiple Traction unit(s) to comply with contact line separation."@en ;
    rdfs:domain [ a owl:Class ;
            owl:unionOf ( <SubsetWithCommonCharacteristics> <Track> ) ] ;
    rdfs:isDefinedBy <> ;
    rdfs:range xsd:anyURI ;
    ns1:term_status "stable" .

<documentRestrictionPowerConsumption> a owl:DatatypeProperty ;
    rdfs:label "Document with restriction related to power consumption of specific electric traction unit(s)"@en ;
    <rinfIndex> "1.1.1.2.5.4" ;
    dcterms:created "2023-03-14"^^xsd:date ;
    rdfs:comment "Name and/or reference of the document specifying the restriction(s) related to power consumption of specific electric traction unit(s)."@en ;
    rdfs:domain [ a owl:Class ;
            owl:unionOf ( <SubsetWithCommonCharacteristics> <Track> ) ] ;
    rdfs:isDefinedBy <> ;
    rdfs:range xsd:anyURI ;
    ns1:term_status "stable" .

<eddyCurrentBraking> a owl:FunctionalProperty,
        owl:ObjectProperty ;
    rdfs:label "Use of eddy current brakes"@en ;
    <XMLName> "ILR_EddyCurrentBrakes" ;
    <appendixD2Index> "3.4.5" ;
    <inSkosConceptScheme> <concepts/eddy-current-braking/EddyCurrentBraking> ;
    <rinfIndex> "1.1.1.1.6.2",
        "1.2.1.0.4.2" ;
    <usedInRCCCalculations> true ;
    dcterms:created "2020-08-24"^^xsd:date ;
    dcterms:modified "2022-09-06"^^xsd:date ;
    dcterms:source <https://eur-lex.europa.eu/eli/reg_impl/2019/773/oj> ;
    rdfs:comment "Indication of limitations on the use of eddy current brakes."@en,
        "This property has been modified to be a RINF parameter (its eratvIndex is deleted). It is treated as a SKOS by RINF and as a boolean by ERATV. A new ERATV datatype property has been defined, eddyCurrentBrakingFitted with boolean values."@en ;
    rdfs:domain [ a owl:Class ;
            owl:unionOf ( <SubsetWithCommonCharacteristics> <Track> ) ] ;
    rdfs:isDefinedBy <> ;
    rdfs:range ns2:Concept ;
    ns1:term_status "stable" .

<eddyCurrentBrakingConditionsDocument> a owl:ObjectProperty ;
    rdfs:label "Document with the conditions for the use of eddy current brakes"@en ;
    <XMLName> "ILR_ECBDocRef" ;
    <appendixD2Index> "3.4.5" ;
    <rinfIndex> "1.1.1.1.6.4" ;
    <usedInRCCCalculations> true ;
    dcterms:created "2020-08-24"^^xsd:date ;
    dcterms:modified "2024-04-23"^^xsd:date ;
    dcterms:source <https://eur-lex.europa.eu/eli/reg_impl/2019/773/oj> ;
    rdfs:comment "Electronic document available in two EU languages from the IM stored by the Agency with conditions for the use of eddy current brakes identified in 1.1.1.1.6.2."@en ;
    rdfs:domain [ a owl:Class ;
            owl:unionOf ( <SubsetWithCommonCharacteristics> <Track> ) ] ;
    rdfs:isDefinedBy <> ;
    rdfs:range <Document> ;
    ns1:term_status "stable" ;
    ns2:changeNote "Change from datatype property to object property in order to point to the class Document (reference document)"@en .

<endLocation> a owl:ObjectProperty ;
    rdfs:label "End of tunnel location"@en ;
    <XMLName> "SOLTunnelEnd" ;
    <rinfIndex> "1.1.1.1.8.4" ;
    dcterms:created "2020-07-29"^^xsd:date ;
    dcterms:modified "2024-02-05"^^xsd:date ;
    rdfs:comment """Part of the End of tunnel that indicates the Geographical coordinates according to the standard World Geodetic System (WGS). Precision for both geographical latitude and geographical longitude is assumed as [NN.NNNNNNN] in degrees with decimals what gives discretion of 10 m cm in the network.
The End of tunnel is the Geographical coordinates in decimal degrees and km of the line at the end of a tunnel."""@en ;
    rdfs:domain <Tunnel> ;
    rdfs:isDefinedBy <> ;
    rdfs:range [ a owl:Class ;
            owl:unionOf ( <http://www.opengis.net/ont/geosparql#Geometry> <http://www.w3.org/2003/01/geo/wgs84_pos#Point> ) ] ;
    rdfs:subPropertyOf <http://www.opengis.net/ont/geosparql#hasGeometry>,
        <http://www.w3.org/2003/01/geo/wgs84_pos#location> ;
    ns1:term_status "stable" .

<energySupplySystemTSICompliant> a owl:DatatypeProperty ;
    rdfs:label "Energy supply system TSI compliant"@en ;
    <XMLName> "ECS_TSIVoltFreq" ;
    <rinfIndex> "1.1.1.2.2.1.2.1" ;
    <usedInRCCCalculations> true ;
    dcterms:created "2020-08-24"^^xsd:date ;
    dcterms:modified "2021-08-06"^^xsd:date ;
    rdfs:comment "Indication if the traction supply system (nominal voltage and frequency) is fully compliant with TSI."@en ;
    rdfs:domain <ContactLineSystem> ;
    rdfs:isDefinedBy <> ;
    rdfs:range xsd:boolean ;
    ns1:term_status "stable" .

<ertmsErrorCorrectionsOnBoard> a owl:DatatypeProperty ;
    rdfs:label "ERTMS error corrections required for the on-board"@en ;
    <rinfIndex> "1.1.1.3.1.2" ;
    dcterms:created "2024-01-08"^^xsd:date ;
    rdfs:comment "List of unacceptable errors impacting the IM network that are required to be solved in the on-board according to the TSI CCS point 7.2.10.3 specification maintenance point."@en ;
    rdfs:domain [ a owl:Class ;
            owl:unionOf ( <SubsetWithCommonCharacteristics> <Track> ) ] ;
    rdfs:isDefinedBy <> ;
    rdfs:range xsd:anyURI ;
    ns1:term_status "stable" .

<etcsDegradedSituation> a owl:ObjectProperty ;
    rdfs:label "ETCS level for degraded situation"@en ;
    <XMLName> "CLD_ETCSSituation" ;
    <appendixD2Index> "3.1.7" ;
    <inSkosConceptScheme> <concepts/etcs-situation/ETCSSituations> ;
    <rinfIndex> "1.1.1.3.10.1",
        "1.2.1.1.9.1" ;
    dcterms:created "2021-08-09"^^xsd:date ;
    dcterms:modified "2021-09-12"^^xsd:date ;
    dcterms:source <https://eur-lex.europa.eu/eli/reg_impl/2019/773/oj> ;
    rdfs:comment "ERTMS / ETCS application level for degraded situation related to the track side equipment."@en ;
    rdfs:domain [ a owl:Class ;
            owl:unionOf ( <SubsetWithCommonCharacteristics> <Track> ) ] ;
    rdfs:isDefinedBy <> ;
    rdfs:range ns2:Concept ;
    ns1:term_status "stable" .

<etcsErrorCorrectionsOnboard> a owl:DatatypeProperty ;
    rdfs:label "ETCS error corrections required for the on-board"@en ;
    <rinfIndex> "1.2.1.1.1.19" ;
    dcterms:created "2023-03-14"^^xsd:date ;
    dcterms:modified "2024-01-08"^^xsd:date ;
    rdfs:comment "List of unacceptable errors impacting the IM network that are required to be solved in the on-board according to the CCS TSI point 7.2.10.3 specification maintenance point."@en ;
    rdfs:domain [ a owl:Class ;
            owl:unionOf ( <SubsetWithCommonCharacteristics> <Track> ) ] ;
    rdfs:isDefinedBy <> ;
    rdfs:range xsd:anyURI ;
    ns1:term_status "stable" .

<etcsImplementsLevelCrossingProcedure> a owl:DatatypeProperty ;
    rdfs:label "ETCS trackside implements level crossing procedure or an equivalent solution"@en ;
    <appendixD3Index> "1.2" ;
    <rinfIndex> "1.1.1.3.2.13",
        "1.2.1.1.1.13" ;
    dcterms:created "2022-11-04"^^xsd:date ;
    rdfs:comment "If the trackside does not implement any solution to cover defective LXs (which are normally protected by means of a technical system), then drivers will be required to comply with instructions received from other sources."@en ;
    rdfs:domain [ a owl:Class ;
            owl:unionOf ( <SubsetWithCommonCharacteristics> <Track> ) ] ;
    rdfs:isDefinedBy <> ;
    rdfs:range xsd:boolean ;
    ns1:term_status "stable" .

<etcsInfill> a owl:FunctionalProperty,
        owl:ObjectProperty ;
    rdfs:label "ETCS infill installed line-side"@en ;
    <XMLName> "CPE_InfillLineSide" ;
    <eratvIndex> "4.13.1.3" ;
    <inSkosConceptScheme> <concepts/etcs-infills/ETCSInfills> ;
    <rinfIndex> "1.1.1.3.2.4",
        "1.2.1.1.1.4" ;
    dcterms:created "2021-08-08"^^xsd:date ;
    dcterms:modified "2021-09-12"^^xsd:date ;
    rdfs:comment "Information about installed trackside equipment capable to transmit infill information by loop or Global System for Mobile communications for Railways (GSM-R) for level 1 installations."@en ;
    rdfs:domain [ a owl:Class ;
            owl:unionOf ( <SubsetWithCommonCharacteristics> <Track> <VehicleType> ) ] ;
    rdfs:isDefinedBy <> ;
    rdfs:range ns2:Concept ;
    ns1:term_status "stable" .

<etcsInfillLineAccess> a owl:DatatypeProperty,
        owl:FunctionalProperty ;
    rdfs:label "ETCS infill necessary for line access"@en ;
    <XMLName> "CPE_Infill" ;
    <rinfIndex> "1.1.1.3.2.3",
        "1.2.1.1.1.3" ;
    dcterms:created "2021-08-08"^^xsd:date ;
    dcterms:modified "2021-09-12"^^xsd:date ;
    rdfs:comment "Indication whether infill is required to access the line for safety reasons."@en ;
    rdfs:domain [ a owl:Class ;
            owl:unionOf ( <SubsetWithCommonCharacteristics> <Track> ) ] ;
    rdfs:isDefinedBy <> ;
    rdfs:range xsd:boolean ;
    ns1:term_status "stable" .

<etcsLevel> a owl:ObjectProperty ;
    rdfs:label "European Train Control System (ETCS) level"@en ;
    <rinfIndex> "1.2.1.1.1.1" ;
    dcterms:created "2021-08-07"^^xsd:date ;
    dcterms:modified "2021-09-12"^^xsd:date ;
    rdfs:comment "ETCS application level related to the track side equipment."@en ;
    rdfs:domain [ a owl:Class ;
            owl:unionOf ( <SubsetWithCommonCharacteristics> <Track> ) ] ;
    rdfs:isDefinedBy <> ;
    rdfs:range <ETCSLevel> ;
    ns1:term_status "stable" .

<etcsMVersion> a owl:FunctionalProperty,
        owl:ObjectProperty ;
    rdfs:label "ETCS M_version"@en ;
    <XMLName> "CPE_MVersion" ;
    <inSkosConceptScheme> <concepts/etcs-m-versions/ETCSMVersions> ;
    <rinfIndex> "1.1.1.3.2.10",
        "1.2.1.1.1.10" ;
    <usedInRCCCalculations> true ;
    dcterms:created "2021-08-08"^^xsd:date ;
    dcterms:modified "2021-09-12"^^xsd:date ;
    rdfs:comment "ETCS M_version according to the specification referenced in Appendix A-1, index [C]."@en ;
    rdfs:domain [ a owl:Class ;
            owl:unionOf ( <SubsetWithCommonCharacteristics> <Track> ) ] ;
    rdfs:isDefinedBy <> ;
    rdfs:range ns2:Concept ;
    ns1:term_status "stable" .

<etcsNationalPacket44> a owl:DatatypeProperty,
        owl:FunctionalProperty ;
    rdfs:label "ETCS national packet 44 application implemented"@en ;
    <XMLName> "CPE_NatApplication" ;
    <rinfIndex> "1.1.1.3.2.5",
        "1.2.1.1.1.5" ;
    dcterms:created "2021-08-08"^^xsd:date ;
    dcterms:modified "2021-09-12"^^xsd:date ;
    rdfs:comment "Indication whether data for national packet 44 applications is transmitted between track and train."@en ;
    rdfs:domain [ a owl:Class ;
            owl:unionOf ( <SubsetWithCommonCharacteristics> <Track> ) ] ;
    rdfs:isDefinedBy <> ;
    rdfs:range xsd:boolean ;
    ns1:term_status "stable" .

<etcsOptionalFunctions> a owl:DatatypeProperty ;
    rdfs:label "ETCS optional functions"@en ;
    <rinfIndex> "1.1.1.3.2.7" ;
    dcterms:created "2021-08-08"^^xsd:date ;
    dcterms:modified "2023-03-14"^^xsd:date ;
    rdfs:comment "Deprecated according to the ammendment to the Regulation (EU) 2019/777. Optional ETCS functions which might improve operation on the line."@en ;
    rdfs:domain [ a owl:Class ;
            owl:unionOf ( <SubsetWithCommonCharacteristics> <Track> ) ] ;
    rdfs:isDefinedBy <> ;
    rdfs:range xsd:string ;
    owl:deprecated true ;
    ns1:term_status "unstable" .

<etcsSystemCompatibility> a owl:ObjectProperty ;
    rdfs:label "ETCS system compatibility"@en ;
    <XMLName> "CPE_SystemCompatibility" ;
    <eratvIndex> "4.13.1.8" ;
    <inSkosConceptScheme> <concepts/etcs-system-compatibilities/ETCSSystemCompatibilities> ;
    <rinfIndex> "1.1.1.3.2.9",
        "1.2.1.1.1.9" ;
    <usedInRCCCalculations> true ;
    dcterms:created "2020-08-31"^^xsd:date ;
    dcterms:modified "2021-09-12"^^xsd:date ;
    rdfs:comment "ETCS requirements used for demonstrating technical compatibility."@en ;
    rdfs:domain [ a owl:Class ;
            owl:unionOf ( <Track> <VehicleType> ) ] ;
    rdfs:isDefinedBy <> ;
    rdfs:range ns2:Concept ;
    ns1:term_status "stable" .

<etcsSystemFunctionalitiesNextFiveYears> a owl:DatatypeProperty ;
    rdfs:label "ETCS system version 2.2 or 3.0 functionalities to be required in the next 5 years"@en ;
    <rinfIndex> "1.1.1.3.2.19",
        "1.2.1.1.1.20" ;
    dcterms:created "2023-03-14"^^xsd:date ;
    dcterms:modified "2024-01-08"^^xsd:date ;
    rdfs:comment "List of ETCS system version 2.2 or 3.0 functionalities to be required in the next 5 years according to TSI CCS point 6.1.1.2 and Appendix G."@en ;
    rdfs:domain [ a owl:Class ;
            owl:unionOf ( <SubsetWithCommonCharacteristics> <Track> ) ] ;
    rdfs:isDefinedBy <> ;
    rdfs:range xsd:anyURI ;
    rdfs:subPropertyOf owl:topDataProperty ;
    ns1:term_status "stable" .

<etcsTransmitsTrackConditions> a owl:DatatypeProperty ;
    rdfs:label "Is the ETCS trackside engineered to transmit Track Conditions"@en ;
    <appendixD3Index> "1.1" ;
    <rinfIndex> "1.1.1.3.2.12",
        "1.2.1.1.1.12" ;
    dcterms:created "2022-11-04"^^xsd:date ;
    dcterms:modified "2023-03-14"^^xsd:date ;
    rdfs:comment """According to the specification referenced in Appendix A-1, index [C]
If the trackside does not provide Track Conditions, the driver will need to be informed about such conditions via alternative methods."""@en ;
    rdfs:domain [ a owl:Class ;
            owl:unionOf ( <SubsetWithCommonCharacteristics> <Track> ) ] ;
    rdfs:isDefinedBy <> ;
    rdfs:range xsd:boolean ;
    ns1:term_status "stable" .

<etcsTransmittedTrackConditions> a owl:ObjectProperty ;
    rdfs:label "Track conditions which can be transmitted"@en ;
    <appendixD3Index> "1.1" ;
    <rinfIndex> "1.1.1.3.2.12.1",
        "1.2.1.1.1.12.1" ;
    dcterms:created "2022-11-16"^^xsd:date ;
    dcterms:modified "2023-03-14"^^xsd:date ;
    rdfs:comment """According to the specification referenced in Appendix A-1, index [C]. 
In https://www.era.europa.eu/sites/default/files/filesystem/ertms/ccs_tsi_annex_a_-_mandatory_specifications/set_of_specifications_3_etcs_b3_r2_gsm-r_b1/index004_-_subset-026_v360.zip
Chapter 5, section 5.18.1.1."""@en ;
    rdfs:domain [ a owl:Class ;
            owl:unionOf ( <SubsetWithCommonCharacteristics> <Track> ) ] ;
    rdfs:isDefinedBy <> ;
    rdfs:range ns2:Concept ;
    ns1:term_status "unstable" .

<flangeLubeForbidden> a owl:DatatypeProperty,
        owl:FunctionalProperty ;
    rdfs:label "Use of flange lubrication forbidden"@en ;
    <XMLName> "IHS_FlangeLubeForbidden" ;
    <rinfIndex> "1.1.1.1.7.1" ;
    dcterms:created "2021-08-08"^^xsd:date ;
    dcterms:modified "2021-09-11"^^xsd:date ;
    rdfs:comment "Indication whether the use of on-board device for flange lubrication is forbidden."@en ;
    rdfs:domain [ a owl:Class ;
            owl:unionOf ( <SubsetWithCommonCharacteristics> <Track> ) ] ;
    rdfs:isDefinedBy <> ;
    rdfs:range xsd:boolean ;
    ns1:term_status "stable" .

<flangeLubeRules> a owl:DatatypeProperty ;
    rdfs:label "Existence of rules on on-board flange lubrication"@en ;
    <XMLName> "CTD_FlangeLubeRules" ;
    <rinfIndex> "1.1.1.3.7.20" ;
    dcterms:created "2021-08-08"^^xsd:date ;
    dcterms:modified "2023-03-14"^^xsd:date ;
    rdfs:comment "Deprecated according to the ammendment to the Regulation (EU) 2019/777. Indication whether rules for activation or deactivation of flange lubrication exist."@en ;
    rdfs:domain <TrainDetectionSystem> ;
    rdfs:isDefinedBy <> ;
    rdfs:range xsd:boolean ;
    owl:deprecated true ;
    ns1:term_status "stable" .

<freightCorridor> a owl:ObjectProperty ;
    rdfs:label "Part of a Railway Freight Corridor"@en ;
    <XMLName> "IPP_FreightCorridor" ;
    <inSkosConceptScheme> <concepts/freight-corridor/FreightCorridors> ;
    <rinfIndex> "1.1.1.1.2.3",
        "1.2.1.0.2.3" ;
    dcterms:created "2021-08-03"^^xsd:date ;
    dcterms:modified "2024-01-08"^^xsd:date ;
    rdfs:comment "Indication whether the line is designated to a Railway Freight Corridor."@en ;
    rdfs:domain [ a owl:Class ;
            owl:unionOf ( <SubsetWithCommonCharacteristics> <Track> ) ] ;
    rdfs:isDefinedBy <> ;
    rdfs:range ns2:Concept ;
    ns1:term_status "stable" .

<frenchTrainDetectionSystemLimitation> a owl:ObjectProperty ;
    rdfs:label "Section with train detection limitation, only for the French network"@en ;
    <XMLName> "CTD_TCLimitation" ;
    <inSkosConceptScheme> <concepts/train-detection/FrenchTrainDetectionSystemLimitations> ;
    <rinfIndex> "1.1.1.3.7.1.4",
        "1.2.1.1.6.3" ;
    dcterms:created "2020-08-24"^^xsd:date ;
    dcterms:isReplacedBy <frenchTrainDetectionSystemLimitationApplicable>,
        <frenchTrainDetectionSystemLimitationNumber>,
        <tdsFrenchTrainDetectionSystemLimitation> ;
    dcterms:modified "2022-04-05"^^xsd:date ;
    rdfs:comment "Specific for route compatibility check on French network.The reason for deprecation is because of replacement by a class, an object property and two datatype properties. The reason is that the property is composed of two values: A boolean [Y/N] and  a number N is between 1 and 8."@en ;
    rdfs:domain <TrainDetectionSystem> ;
    rdfs:isDefinedBy <> ;
    rdfs:range ns2:Concept ;
    owl:deprecated true ;
    ns1:term_status "stable" .

<frequencyBandsForDetection> a owl:ObjectProperty ;
    rdfs:label "Frequency bands for detection"@en ;
    <rinfIndex> "1.1.1.3.4.2",
        "1.2.1.1.3.2" ;
    dcterms:created "2023-03-14"^^xsd:date ;
    rdfs:comment "Bands of the frequency management of the train detection systems as defined in the specification referenced in Appendix A-1, index [D], and in the specific cases or technical documents referred to in Article 13 of TSI CCS when they are available."@en ;
    rdfs:domain <TrainDetectionSystem> ;
    rdfs:isDefinedBy <> ;
    rdfs:range ns2:Concept ;
    ns1:term_status "unstable" .

<gaugingCheckLocation> a owl:DatatypeProperty ;
    rdfs:label "Railway location of particular points requiring specific checks"@en ;
    <XMLName> "ILL_GaugeCheckLoc" ;
    <rinfIndex> "1.1.1.1.3.1.2",
        "1.2.1.0.3.5" ;
    <usedInRCCCalculations> true ;
    dcterms:created "2020-07-29"^^xsd:date ;
    dcterms:modified "2024-01-08"^^xsd:date ;
    rdfs:comment "Location of particular points requiring specific checks due to deviations from gauging referred to in parameter \"Gauging\"."@en ;
    rdfs:domain [ a owl:Class ;
            owl:unionOf ( <SubsetWithCommonCharacteristics> <Track> ) ] ;
    rdfs:isDefinedBy <> ;
    rdfs:range xsd:string ;
    ns1:term_status "stable" .

<gaugingProfile> a owl:ObjectProperty ;
    rdfs:label "Gauging"@en ;
    <XMLName> "ILL_Gauging" ;
    <eratvIndex> "4.2.1" ;
    <inSkosConceptScheme> <concepts/gaugings/GaugingProfiles> ;
    <rinfIndex> "1.1.1.1.3.1.1",
        "1.2.1.0.3.4" ;
    <usedInRCCCalculations> true ;
    dcterms:created "2020-07-29"^^xsd:date ;
    dcterms:modified "2023-03-14"^^xsd:date ;
    rdfs:comment """Gauges as defined in European standard or other local gauges, including lower or upper part.
In accordance with point 7.3.2.2 of LOC&PAS TSI, sections of lines of the United Kingdom of Great Britain network may not have gauge reference profile."""@en ;
    rdfs:domain [ a owl:Class ;
            owl:unionOf ( <SubsetWithCommonCharacteristics> <Track> <VehicleType> ) ] ;
    rdfs:isDefinedBy <> ;
    rdfs:range ns2:Concept ;
    ns1:term_status "stable" .

<gaugingTransversalDocument> a owl:ObjectProperty ;
    rdfs:label "Document with the transversal section of the particular points requiring specific checks"@en ;
    <XMLName> "ILL_GaugeCheckDocRef" ;
    <rinfIndex> "1.1.1.1.3.1.3",
        "1.2.1.0.3.6" ;
    <usedInRCCCalculations> true ;
    dcterms:created "2020-08-24"^^xsd:date ;
    dcterms:modified "2024-04-23"^^xsd:date ;
    rdfs:comment "Electronic document available from the IM stored by the Agency with the transversal section of the particular points requiring specific checks due to deviations from gauging referred to in parameter \"Gauging\". Where relevant, guidance for the check with the particular point may be attached to the document with the transversal section."@en ;
    rdfs:domain [ a owl:Class ;
            owl:unionOf ( <SubsetWithCommonCharacteristics> <Track> ) ] ;
    rdfs:isDefinedBy <> ;
    rdfs:range <Document> ;
    ns1:term_status "stable" ;
    ns2:changeNote "Change from datatype property to object property in order to point to the class Document (reference document)"@en .

<gprsForETCS> a owl:DatatypeProperty,
        owl:FunctionalProperty ;
    rdfs:label "GPRS for ETCS"@en ;
    <XMLName> "CRG_GPRSForETCS" ;
    <rinfIndex> "1.1.1.3.3.3.2",
        "1.2.1.1.2.3.2" ;
    dcterms:created "2021-08-08"^^xsd:date ;
    dcterms:modified "2021-09-12"^^xsd:date ;
    rdfs:comment "Indication if GPRS can be used for ETCS."@en ;
    rdfs:domain [ a owl:Class ;
            owl:unionOf ( <SubsetWithCommonCharacteristics> <Track> ) ] ;
    rdfs:isDefinedBy <> ;
    rdfs:range xsd:boolean ;
    ns1:term_status "stable" .

<gprsImplementationArea> a owl:DatatypeProperty ;
    rdfs:label "Area of implementation of GPRS"@en ;
    <XMLName> "CRG_GPRSAreaOfImpl" ;
    <rinfIndex> "1.1.1.3.3.3.3",
        "1.2.1.1.2.3.3" ;
    dcterms:created "2021-08-09"^^xsd:date ;
    dcterms:modified "2021-09-12"^^xsd:date ;
    rdfs:comment "Indication of the area in which GPRS can be used for ETCS."@en ;
    rdfs:domain [ a owl:Class ;
            owl:unionOf ( <SubsetWithCommonCharacteristics> <Track> ) ] ;
    rdfs:isDefinedBy <> ;
    rdfs:range xsd:string ;
    ns1:term_status "stable" .

<gradient> a owl:DatatypeProperty,
        owl:FunctionalProperty ;
    rdfs:label "Gradient for stabling tracks"@en ;
    <XMLName> "ILL_Gradient" ;
    <rinfIndex> "1.2.2.0.3.1" ;
    <unitOfMeasure> <http://qudt.org/vocab/unit/MilliM-PER-M> ;
    <usedInRCCCalculations> true ;
    dcterms:created "2021-08-10"^^xsd:date ;
    dcterms:modified "2021-08-10"^^xsd:date ;
    dcterms:source <https://rsm-evolution.org/220927_RSM/EARoot/EA2/EA1/EA166.html> ;
    rdfs:comment "Maximum value of the gradient for stabling tracks expressed in millimetres per metre."@en ;
    rdfs:domain <Siding> ;
    rdfs:isDefinedBy <> ;
    rdfs:range xsd:double ;
    ns1:term_status "stable" .

<gradientProfile> a owl:DatatypeProperty ;
    rdfs:label "Gradient profile"@en ;
    <XMLName> "ILL_GradProfile" ;
    <appendixD2Index> "3.2.1",
        "3.2.2" ;
    <rinfIndex> "1.1.1.1.3.6" ;
    <usedInRCCCalculations> true ;
    dcterms:created "2020-08-24"^^xsd:date ;
    dcterms:modified "2021-09-10"^^xsd:date ;
    dcterms:source <https://rsm-evolution.org/220927_RSM/EARoot/EA2/EA1/EA166.html> ;
    rdfs:comment "Sequence of gradient values and locations of change in gradient."@en ;
    rdfs:domain [ a owl:Class ;
            owl:unionOf ( <SubsetWithCommonCharacteristics> <Track> ) ] ;
    rdfs:isDefinedBy <> ;
    rdfs:range xsd:string ;
    ns1:term_status "stable" .

<gsmRActiveMobiles> a owl:FunctionalProperty,
        owl:ObjectProperty ;
    rdfs:label "Number of active GSM-R mobiles (EDOR) or simultaneous communication session on-board for ETCS Level 2 (or level 3) needed to perform radio block centre handovers without having an operational disruption"@en ;
    <XMLName> "CRG_NumActiveMob" ;
    <inSkosConceptScheme> <concepts/gsmr-number-active-mobiles/NumberActiveMobiles> ;
    <rinfIndex> "1.1.1.3.3.2",
        "1.2.1.1.2.2" ;
    dcterms:created "2021-08-08"^^xsd:date ;
    dcterms:modified "2021-09-12"^^xsd:date ;
    rdfs:comment "Number of simultaneous communication session on board for ETCS level R required for a smooth running of the train. This relates to the radio block centre (RBC) handling of communication sessions. Not safety critical and no matter of interoperability."@en ;
    rdfs:domain [ a owl:Class ;
            owl:unionOf ( <SubsetWithCommonCharacteristics> <Track> ) ] ;
    rdfs:isDefinedBy <> ;
    rdfs:range ns2:Concept ;
    ns1:term_status "stable" .

<gsmRAdditionalInfo> a owl:ObjectProperty ;
    rdfs:label "Additional information on network characteristics"@en ;
    <XMLName> "CRG_AdditionalnetworkInfo" ;
    <rinfIndex> "1.1.1.3.3.3.1",
        "1.2.1.1.2.3.1" ;
    dcterms:created "2021-08-08"^^xsd:date ;
    dcterms:modified "2024-04-23"^^xsd:date ;
    rdfs:comment "Any additional information on network characteristics or corresponding document available from the IM and stored by the Agency, e.g.; interference level, leading to the recommendation of additional on-board protection."@en ;
    rdfs:domain [ a owl:Class ;
            owl:unionOf ( <SubsetWithCommonCharacteristics> <Track> ) ] ;
    rdfs:isDefinedBy <> ;
    rdfs:range <Document> ;
    ns1:term_status "stable" ;
    ns2:changeNote "Change from datatype property to object property in order to point to the class Document (reference document)"@en .

<gsmRNoCoverage> a owl:DatatypeProperty,
        owl:FunctionalProperty ;
    rdfs:label "No GSMR coverage"@en ;
    <XMLName> "CRG_GSMRNoCoverage" ;
    <rinfIndex> "1.1.1.3.3.8",
        "1.2.1.1.2.8" ;
    dcterms:created "2021-08-09"^^xsd:date ;
    dcterms:modified "2021-09-12"^^xsd:date ;
    rdfs:comment "Indication if there is no GSMR coverage."@en ;
    rdfs:domain [ a owl:Class ;
            owl:unionOf ( <SubsetWithCommonCharacteristics> <Track> ) ] ;
    rdfs:isDefinedBy <> ;
    rdfs:range xsd:boolean ;
    ns1:term_status "stable" .

<gsmROptionalFunctions> a owl:ObjectProperty ;
    rdfs:label "Optional GSM-R functions"@en ;
    <XMLName> "CRG_OptionalFunctions" ;
    <inSkosConceptScheme> <concepts/gsmr-optional-functions/OptionalFunctions> ;
    <rinfIndex> "1.1.1.3.3.3",
        "1.2.1.1.2.3" ;
    dcterms:created "2021-08-08"^^xsd:date ;
    dcterms:modified "2021-09-12"^^xsd:date ;
    rdfs:comment "Use of optional GSM-R functions which might improve operation on the line. They are for information only and not for network access criteria."@en ;
    rdfs:domain [ a owl:Class ;
            owl:unionOf ( <SubsetWithCommonCharacteristics> <Track> ) ] ;
    rdfs:isDefinedBy <> ;
    rdfs:range ns2:Concept ;
    ns1:term_status "stable" .

<gsmrConstraintsOperateOnlyInCircuitSwitch> a owl:ObjectProperty ;
    rdfs:label "Specific constraints imposed by the GSM-R network operator on ETCS on-board units only able to operate in circuit-switch"@en ;
    <appendixD3Index> "2.2" ;
    <rinfIndex> "1.2.1.1.2.12" ;
    dcterms:created "2023-03-14"^^xsd:date ;
    rdfs:comment """These constraints, where applicable, are meant to manage the limited number of circuit-switched radio connections that can be handled simultaneously by a Radio Block Center.
"""@en ;
    rdfs:domain [ a owl:Class ;
            owl:unionOf ( <SubsetWithCommonCharacteristics> <Track> ) ] ;
    rdfs:isDefinedBy <> ;
    rdfs:range ns2:Concept ;
    ns1:term_status "stable" .

<gsmrErrorCorrectionsOnboard> a owl:DatatypeProperty ;
    rdfs:label "GSM-R error corrections required for the on-board"@en ;
    dcterms:created "2023-03-14"^^xsd:date ;
    dcterms:modified "2024-01-08"^^xsd:date ;
    rdfs:comment """List of unacceptable errors impacting the IM network that are required to be solved in the on-board according to the CCS TSI point 7.2.10.3 specification maintenance point.
The reason for deprecation is that this parameter does not appear in the latest legal text."""@en ;
    rdfs:domain [ a owl:Class ;
            owl:unionOf ( <SubsetWithCommonCharacteristics> <Track> ) ] ;
    rdfs:isDefinedBy <> ;
    rdfs:range xsd:anyURI ;
    owl:deprecated true ;
    ns1:term_status "stable" .

<gsmrForcedDeregistrationFunctionalNumber> a owl:DatatypeProperty ;
    rdfs:label "GSM-R network is configured to allow forced de-registration of a functional number by another driver"@en ;
    <appendixD3Index> "2.1" ;
    <rinfIndex> "1.1.1.3.3.11",
        "1.2.1.1.2.11" ;
    dcterms:created "2022-11-07"^^xsd:date ;
    dcterms:modified "2023-03-14"^^xsd:date ;
    rdfs:comment "This feature will condition the applicable operational rules for drivers and signallers when dealing with cab radios registered under wrong numbers."@en ;
    rdfs:domain [ a owl:Class ;
            owl:unionOf ( <SubsetWithCommonCharacteristics> <Track> ) ] ;
    rdfs:isDefinedBy <> ;
    rdfs:range xsd:boolean ;
    ns1:term_status "stable" .

<gsmrNetworkCoverage> a owl:ObjectProperty ;
    rdfs:label "GSM-R networks covered by a roaming agreement"@en ;
    <XMLName> "CRG_RoamingAgreement" ;
    <inSkosConceptScheme> <concepts/gsmr-networks/GSMRNetworks> ;
    <rinfIndex> "1.1.1.3.3.5",
        "1.2.1.1.2.5" ;
    <usedInRCCCalculations> true ;
    dcterms:created "2020-08-31"^^xsd:date ;
    dcterms:modified "2021-09-12"^^xsd:date ;
    rdfs:comment "List of GSM-R networks which are covered by a roaming agreement."@en ;
    rdfs:domain [ a owl:Class ;
            owl:unionOf ( <SubsetWithCommonCharacteristics> <Track> ) ] ;
    rdfs:isDefinedBy <> ;
    rdfs:range ns2:Concept ;
    ns1:term_status "stable" .

<hasAdditionalBrakingInformation> a owl:DatatypeProperty,
        owl:FunctionalProperty ;
    rdfs:label "Availability by the IM of additional information"@en ;
    <XMLName> "CBP_AddInfoAvailable" ;
    <rinfIndex> "1.1.1.3.11.2" ;
    <usedInRCCCalculations> true ;
    dcterms:created "2020-08-24"^^xsd:date ;
    dcterms:modified "2024-01-08"^^xsd:date ;
    rdfs:comment "Availability by the IM of additional information as defined in point (2) of point 4.2.2.6.2 of TSI OPE."@en ;
    rdfs:domain [ a owl:Class ;
            owl:unionOf ( <SubsetWithCommonCharacteristics> <Track> ) ] ;
    rdfs:isDefinedBy <> ;
    rdfs:range xsd:boolean ;
    ns1:term_status "stable" .

<hasBallast> a owl:DatatypeProperty,
        owl:FunctionalProperty ;
    rdfs:label "Existence of ballast"@en ;
    <XMLName> "ITP_Ballast" ;
    <rinfIndex> "1.1.1.1.4.4" ;
    dcterms:created "2021-08-03"^^xsd:date ;
    dcterms:modified "2021-09-10"^^xsd:date ;
    rdfs:comment "Specifies whether track construction is with sleepers embedded in ballast or not."@en ;
    rdfs:domain [ a owl:Class ;
            owl:unionOf ( <SubsetWithCommonCharacteristics> <Track> ) ] ;
    rdfs:isDefinedBy <> ;
    rdfs:range xsd:boolean ;
    ns1:term_status "stable" .

<hasETCSRestrictionsConditions> a owl:DatatypeProperty,
        owl:FunctionalProperty ;
    rdfs:label "Existence of operating restrictions or conditions"@en ;
    <XMLName> "CPE_RestrictionsConditions" ;
    <rinfIndex> "1.1.1.3.2.6",
        "1.2.1.1.1.6" ;
    dcterms:created "2021-08-08"^^xsd:date ;
    dcterms:modified "2024-01-08"^^xsd:date ;
    rdfs:comment "Indication whether restrictions or conditions due to partial compliance with the TSI CCS exist."@en ;
    rdfs:domain [ a owl:Class ;
            owl:unionOf ( <SubsetWithCommonCharacteristics> <Track> ) ] ;
    rdfs:isDefinedBy <> ;
    rdfs:range xsd:boolean ;
    ns1:term_status "stable" .

<hasElectricShoreSupply> a owl:DatatypeProperty,
        owl:FunctionalProperty ;
    rdfs:label "Existence of electric shore supply"@en ;
    <XMLName> "ITS_ElectricShoreSupply" ;
    <rinfIndex> "1.2.2.0.4.6" ;
    dcterms:created "2021-08-10"^^xsd:date ;
    dcterms:modified "2021-08-10"^^xsd:date ;
    rdfs:comment "Indication whether an installation for electric shore supply exists (fixed installation for servicing trains)."@en ;
    rdfs:domain <Siding> ;
    rdfs:isDefinedBy <> ;
    rdfs:range xsd:boolean ;
    ns1:term_status "stable" .

<hasEmergencyPlan> a owl:DatatypeProperty,
        owl:FunctionalProperty ;
    rdfs:label "Existence of emergency plan"@en ;
    <XMLName> "ITU_EmergencyPlan" ;
    <rinfIndex> "1.1.1.1.8.9",
        "1.2.1.0.5.6",
        "1.2.2.0.5.6" ;
    dcterms:created "2021-08-03"^^xsd:date ;
    dcterms:modified "2021-08-10"^^xsd:date ;
    rdfs:comment "Indication whether emergency plan exists."@en ;
    rdfs:domain <Tunnel> ;
    rdfs:isDefinedBy <> ;
    rdfs:range xsd:boolean ;
    ns1:term_status "stable" .

<hasEvacuationAndRescuePoints> a owl:DatatypeProperty ;
    rdfs:label "Existence of evacuation and rescue points"@en ;
    <appendixD2Index> "3.2.3" ;
    <rinfIndex> "1.1.1.1.8.13",
        "1.2.1.0.5.11",
        "1.2.2.0.5.10" ;
    dcterms:created "2022-10-27"^^xsd:date ;
    dcterms:modified "2023-03-14"^^xsd:date ;
    dcterms:source <https://eur-lex.europa.eu/eli/reg_impl/2019/773/oj> ;
    rdfs:comment "Indication of existence of evacuation and rescue points."@en ;
    rdfs:domain <Tunnel> ;
    rdfs:isDefinedBy <> ;
    rdfs:range xsd:boolean ;
    ns1:term_status "stable" .

<hasExternalCleaning> a owl:DatatypeProperty,
        owl:FunctionalProperty ;
    rdfs:label "Existence of external cleaning facilities"@en ;
    <XMLName> "ITS_ExternalCleaning" ;
    <rinfIndex> "1.2.2.0.4.2" ;
    dcterms:created "2021-08-10"^^xsd:date ;
    dcterms:modified "2024-01-08"^^xsd:date ;
    rdfs:comment "Indication whether exists an installation for external cleaning facility (fixed installation for servicing trains) as defined in TSI INF."@en ;
    rdfs:domain <Siding> ;
    rdfs:isDefinedBy <> ;
    rdfs:range xsd:boolean ;
    ns1:term_status "stable" .

<hasHotAxleBoxDetector> a owl:DatatypeProperty,
        owl:FunctionalProperty ;
    rdfs:label "Existence of trackside hot axle box detector (HABD)"@en ;
    <XMLName> "IHS_HABDExist" ;
    <rinfIndex> "1.1.1.1.7.4" ;
    <usedInRCCCalculations> true ;
    dcterms:created "2020-08-24"^^xsd:date ;
    dcterms:modified "2024-01-08"^^xsd:date ;
    rdfs:comment "Existence of trackside HABD."@en ;
    rdfs:domain [ a owl:Class ;
            owl:unionOf ( <SubsetWithCommonCharacteristics> <Track> ) ] ;
    rdfs:isDefinedBy <> ;
    rdfs:range xsd:boolean ;
    ns1:term_status "stable" .

<hasLevelCrossings> a owl:DatatypeProperty,
        owl:FunctionalProperty ;
    rdfs:label "Existence of level crossings"@en ;
    <XMLName> "IHS_LevelCrossing" ;
    <rinfIndex> "1.1.1.1.7.2" ;
    dcterms:created "2021-08-03"^^xsd:date ;
    dcterms:modified "2021-09-11"^^xsd:date ;
    rdfs:comment "Indication whether level crossings (including pedestrian track crossing) exist on the section of line."@en ;
    rdfs:domain [ a owl:Class ;
            owl:unionOf ( <SubsetWithCommonCharacteristics> <Track> ) ] ;
    rdfs:isDefinedBy <> ;
    rdfs:range xsd:boolean ;
    ns1:term_status "stable" .

<hasOtherTrainProtection> a owl:DatatypeProperty,
        owl:FunctionalProperty ;
    rdfs:label "Existence of other train protection, control and warning systems installed"@en ;
    <rinfIndex> "1.1.1.3.5.1" ;
    dcterms:created "2021-08-09"^^xsd:date ;
    dcterms:modified "2023-03-14"^^xsd:date ;
    rdfs:comment "Deprecated according to the ammendment to the Regulation (EU) 2019/777. Indication if other train protection, control and warning systems in normal operation are installed lineside."@en ;
    rdfs:domain [ a owl:Class ;
            owl:unionOf ( <SubsetWithCommonCharacteristics> <Track> ) ] ;
    rdfs:isDefinedBy <> ;
    rdfs:range xsd:boolean ;
    owl:deprecated true ;
    ns1:term_status "unstable" .

<hasPlatformCurvature> a owl:DatatypeProperty ;
    rdfs:label "Curvature of the platform"@en ;
    <appendixD2Index> "2.3.8" ;
    <rinfIndex> "1.2.1.0.6.8" ;
    dcterms:created "2022-10-27"^^xsd:date ;
    dcterms:modified "2023-03-14"^^xsd:date ;
    dcterms:source <https://eur-lex.europa.eu/eli/reg_impl/2019/773/oj> ;
    rdfs:comment "Indication of the existence of the curvature of the platform."@en ;
    rdfs:domain <PlatformEdge> ;
    rdfs:isDefinedBy <> ;
    rdfs:range xsd:boolean ;
    ns1:term_status "stable" .

<hasRefuelling> a owl:DatatypeProperty,
        owl:FunctionalProperty ;
    rdfs:label "Existence of refuelling"@en ;
    <XMLName> "ITS_Refuelling" ;
    <rinfIndex> "1.2.2.0.4.4" ;
    dcterms:created "2021-08-10"^^xsd:date ;
    dcterms:modified "2024-01-08"^^xsd:date ;
    rdfs:comment "Indication whether exists an installation for refuelling (fixed installation for servicing trains) as defined in TSI INF."@en ;
    rdfs:domain <Siding> ;
    rdfs:isDefinedBy <> ;
    rdfs:range xsd:boolean ;
    ns1:term_status "stable" .

<hasSandRestocking> a owl:DatatypeProperty,
        owl:FunctionalProperty ;
    rdfs:label "Existence of sand restocking"@en ;
    <XMLName> "ITS_SandRestocking" ;
    <rinfIndex> "1.2.2.0.4.5" ;
    dcterms:created "2021-08-10"^^xsd:date ;
    dcterms:modified "2021-08-10"^^xsd:date ;
    rdfs:comment "Indication whether an installation for sand restocking exists (fixed installation for servicing trains)."@en ;
    rdfs:domain <Siding> ;
    rdfs:isDefinedBy <> ;
    rdfs:range xsd:boolean ;
    ns1:term_status "stable" .

<hasSchematicOverviewOPDigitalForm> a owl:DatatypeProperty ;
    rdfs:label "Schematic overview of the operational point in digital form"@en ;
    <rinfIndex> "1.2.0.0.0.7" ;
    dcterms:created "2023-03-14"^^xsd:date ;
    dcterms:modified "2024-01-08"^^xsd:date ;
    rdfs:comment "The existence of a schematic overview of the operational point in digital form."@en ;
    rdfs:domain <OperationalPoint> ;
    rdfs:isDefinedBy <> ;
    rdfs:range xsd:boolean ;
    ns1:term_status "stable" .

<hasSevereWeatherConditions> a owl:DatatypeProperty,
        owl:FunctionalProperty ;
    rdfs:label "Existence of severe climatic conditions"@en ;
    <XMLName> "IPP_SevereClimateCon" ;
    <rinfIndex> "1.1.1.1.2.8" ;
    <usedInRCCCalculations> true ;
    dcterms:created "2020-08-24"^^xsd:date ;
    dcterms:modified "2021-09-10"^^xsd:date ;
    rdfs:comment "Climatic conditions on the line are severe according to European standard."@en ;
    rdfs:domain [ a owl:Class ;
            owl:unionOf ( <SubsetWithCommonCharacteristics> <Track> ) ] ;
    rdfs:isDefinedBy <> ;
    rdfs:range xsd:boolean ;
    ns1:term_status "stable" .

<hasSystemSeparation> a owl:DatatypeProperty,
        owl:FunctionalProperty ;
    rdfs:label "System separation"@en ;
    <XMLName> "EOS_System" ;
    <rinfIndex> "1.1.1.2.4.2.1" ;
    dcterms:created "2021-08-08"^^xsd:date ;
    dcterms:modified "2021-09-12"^^xsd:date ;
    rdfs:comment "Indication of existence of system separation."@en ;
    rdfs:domain [ a owl:Class ;
            owl:unionOf ( <SubsetWithCommonCharacteristics> <Track> ) ] ;
    rdfs:isDefinedBy <> ;
    rdfs:range xsd:boolean ;
    ns1:term_status "stable" .

<hasTSITrainDetection> a owl:DatatypeProperty ;
    rdfs:label "Existence of train detection system fully compliant with the TSI"@en ;
    <XMLName> "CCD_TSITrainDetection" ;
    <rinfIndex> "1.1.1.3.4.1",
        "1.2.1.1.3.1" ;
    dcterms:created "2021-08-09"^^xsd:date ;
    dcterms:modified "2024-01-08"^^xsd:date ;
    rdfs:comment "Indication if there is any train detection system installed and fully compliant with the TSI CCS."@en ;
    rdfs:domain [ a owl:Class ;
            owl:unionOf ( <SubsetWithCommonCharacteristics> <Track> ) ] ;
    rdfs:isDefinedBy <> ;
    rdfs:range xsd:boolean ;
    ns1:term_status "stable" .

<hasToiletDischarge> a owl:DatatypeProperty,
        owl:FunctionalProperty ;
    rdfs:label "Existence of toilet discharge"@en ;
    <XMLName> "ITS_ToiletDischarge" ;
    <rinfIndex> "1.2.2.0.4.1" ;
    dcterms:created "2021-08-10"^^xsd:date ;
    dcterms:modified "2024-01-08"^^xsd:date ;
    rdfs:comment "Indication whether exists an installation for toilet discharge (fixed installation for servicing trains) as defined in TSI INF."@en ;
    rdfs:domain <Siding> ;
    rdfs:isDefinedBy <> ;
    rdfs:range xsd:boolean ;
    ns1:term_status "stable" .

<hasWalkway> a owl:DatatypeProperty ;
    rdfs:label "Existence of walkways"@en ;
    <appendixD2Index> "3.2.3" ;
    <rinfIndex> "1.1.1.1.8.12",
        "1.2.1.0.5.10",
        "1.2.2.0.5.9" ;
    dcterms:created "2022-10-27"^^xsd:date ;
    dcterms:modified "2023-03-14"^^xsd:date ;
    dcterms:source <https://eur-lex.europa.eu/eli/reg_impl/2019/773/oj> ;
    rdfs:comment "Indication of existence of walkways."@en ;
    rdfs:domain <Tunnel> ;
    rdfs:isDefinedBy <> ;
    rdfs:range xsd:boolean ;
    ns1:term_status "stable" .

<hasWaterRestocking> a owl:DatatypeProperty,
        owl:FunctionalProperty ;
    rdfs:label "Existence of water restocking"@en ;
    <XMLName> "ITS_WaterRestocking" ;
    <rinfIndex> "1.2.2.0.4.3" ;
    dcterms:created "2021-08-10"^^xsd:date ;
    dcterms:modified "2024-01-08"^^xsd:date ;
    rdfs:comment "Indication whether exists an installation for water restocking (fixed installation for servicing trains) as defined in TSI INF."@en ;
    rdfs:domain <Siding> ;
    rdfs:isDefinedBy <> ;
    rdfs:range xsd:boolean ;
    ns1:term_status "stable" .

<highSpeedLoadModelCompliance> a owl:DatatypeProperty,
        owl:FunctionalProperty ;
    rdfs:label "Compliance of structures with the High Speed Load Model (HSLM)"@en ;
    <XMLName> "IPP_HSLMCompliant" ;
    <rinfIndex> "1.1.1.1.2.4.2" ;
    <usedInRCCCalculations> true ;
    dcterms:created "2020-08-24"^^xsd:date ;
    dcterms:modified "2024-01-08"^^xsd:date ;
    rdfs:comment """For sections of line with a maximum permitted speed of 200 km/h or more.
Information regarding the procedure to be used to perform the dynamic compatibility check."""@en ;
    rdfs:domain [ a owl:Class ;
            owl:unionOf ( <SubsetWithCommonCharacteristics> <Track> ) ] ;
    rdfs:isDefinedBy <> ;
    rdfs:range xsd:boolean ;
    ns1:term_status "stable" .

<hotAxleBoxDetectorDirection> a owl:ObjectProperty ;
    rdfs:label "Direction of measurement of trackside HABD"@en ;
    <XMLName> "IHS_HABDDirecton" ;
    <inSkosConceptScheme> <concepts/hot-axle/HotAxleBoxDetectorDirections> ;
    <rinfIndex> "1.1.1.1.7.9" ;
    <usedInRCCCalculations> true ;
    dcterms:created "2022-07-08"^^xsd:date ;
    dcterms:modified "2024-01-08"^^xsd:date ;
    rdfs:comment """Specific for the French Italian and Swedish networks.
Applicable if trackside HABD is not TSI compliant, direction of measurement of trackside Hot Axle Box Detector.
If the direction of measurement is:
—	the same as the direction defined by the start and end of the SoL: (N)
—	the opposite to the direction defined by the start and end of the SoL: (O)
—	both directions: (B)."""@en,
        "This property was previously a datatype property with domain Track and range string. As its values are a list of three predefined values, it is now a SKOS."@en ;
    rdfs:domain [ a owl:Class ;
            owl:unionOf ( <SubsetWithCommonCharacteristics> <Track> ) ] ;
    rdfs:isDefinedBy <> ;
    rdfs:range ns2:Concept ;
    rdfs:subPropertyOf owl:topObjectProperty ;
    ns1:term_status "stable" .

<hotAxleBoxDetectorGeneration> a owl:DatatypeProperty,
        owl:FunctionalProperty ;
    rdfs:label "Generation of trackside HABD"@en ;
    <XMLName> "IHS_HABDGen" ;
    <rinfIndex> "1.1.1.1.7.7" ;
    <usedInRCCCalculations> true ;
    dcterms:created "2020-08-24"^^xsd:date ;
    dcterms:modified "2021-09-11"^^xsd:date ;
    rdfs:comment """Specific for the French Italian and Swedish networks.
Generation of trackside hot axle box detector."""@en ;
    rdfs:domain [ a owl:Class ;
            owl:unionOf ( <SubsetWithCommonCharacteristics> <Track> ) ] ;
    rdfs:isDefinedBy <> ;
    rdfs:range xsd:string ;
    ns1:term_status "stable" .

<hotAxleBoxDetectorIdentification> a owl:DatatypeProperty,
        owl:FunctionalProperty ;
    rdfs:label "Identification of trackside HABD"@en ;
    <XMLName> "IHS_HABDID" ;
    <rinfIndex> "1.1.1.1.7.6" ;
    <usedInRCCCalculations> true ;
    dcterms:created "2020-08-24"^^xsd:date ;
    dcterms:modified "2021-09-11"^^xsd:date ;
    rdfs:comment """Specific for the French, Italian and Swedish networks.
Applicable if trackside HABD is not TSI compliant, identification of trackside hot axle box detector."""@en ;
    rdfs:domain [ a owl:Class ;
            owl:unionOf ( <SubsetWithCommonCharacteristics> <Track> ) ] ;
    rdfs:isDefinedBy <> ;
    rdfs:range xsd:string ;
    ns1:term_status "stable" .

<hotAxleBoxDetectorLocation> a owl:DatatypeProperty ;
    rdfs:label "Railway location of trackside HABD"@en ;
    <XMLName> "IHS_HABDLoc" ;
    <rinfIndex> "1.1.1.1.7.8" ;
    <usedInRCCCalculations> true ;
    dcterms:created "2020-08-24"^^xsd:date ;
    dcterms:modified "2021-09-11"^^xsd:date ;
    rdfs:comment """Specific for the French Italian and Swedish networks.
Applicable if trackside HABD is not TSI compliant, localisation of trackside hot axle box detector."""@en ;
    rdfs:domain [ a owl:Class ;
            owl:unionOf ( <SubsetWithCommonCharacteristics> <Track> ) ] ;
    rdfs:isDefinedBy <> ;
    rdfs:range xsd:double ;
    ns1:term_status "stable" .

<hotAxleBoxDetectorTSICompliant> a owl:DatatypeProperty,
        owl:FunctionalProperty ;
    rdfs:label "Trackside HABD TSI compliant"@en ;
    <XMLName> "IHS_TSIHABD" ;
    <rinfIndex> "1.1.1.1.7.5" ;
    <usedInRCCCalculations> true ;
    dcterms:created "2020-08-24"^^xsd:date ;
    dcterms:modified "2021-09-11"^^xsd:date ;
    rdfs:comment """Specific for the French, Italian and Swedish networks.
Trackside hot axle box detector TSI compliant."""@en ;
    rdfs:domain [ a owl:Class ;
            owl:unionOf ( <SubsetWithCommonCharacteristics> <Track> ) ] ;
    rdfs:isDefinedBy <> ;
    rdfs:range xsd:boolean ;
    ns1:term_status "stable" .

<imCode> a owl:DatatypeProperty,
        owl:FunctionalProperty ;
    rdfs:label "Infrastructure manager (IM)'s code"@en ;
    <XMLName> "OPSidingIMCode",
        "OPSidingTunnelIMCode",
        "OPTrackIMCode",
        "OPTrackPlatformIMCode",
        "OPTrackTunnelIMCode",
        "SOLIMCode",
        "SOLTunnelIMCode" ;
    <appendixD2Index> "1.1" ;
    <rinfIndex> "1.1.0.0.0.1",
        "1.1.1.1.8.1",
        "1.2.1.0.0.1",
        "1.2.1.0.5.1",
        "1.2.1.0.6.1",
        "1.2.2.0.0.1",
        "1.2.2.0.5.1" ;
    dcterms:created "2021-08-02"^^xsd:date ;
    dcterms:modified "2024-01-08"^^xsd:date ;
    dcterms:source <https://eur-lex.europa.eu/eli/reg_impl/2019/773/oj> ;
    rdfs:comment "Infrastructure manager means anybody or undertaking that is responsible in particular for establishing and maintaining railway infrastructure or a part thereof."@en ;
    rdfs:domain <InfrastructureManager> ;
    rdfs:isDefinedBy <> ;
    rdfs:range xsd:string ;
    rdfs:subPropertyOf dcterms:identifier ;
    ns1:term_status "stable" .

<instructionsSwitchRadioSystems> a owl:DatatypeProperty ;
    rdfs:label "Special instructions to switch over between different radio systems"@en ;
    <appendixD2Index> "3.4.4" ;
    <rinfIndex> "1.1.1.3.8.2.1",
        "1.2.1.1.7.2.1" ;
    dcterms:created "2022-10-28"^^xsd:date ;
    dcterms:modified "2023-03-14"^^xsd:date ;
    dcterms:source <https://eur-lex.europa.eu/eli/reg_impl/2019/773/oj> ;
    rdfs:comment "Name and/or reference of the document specifying the Special instructions to switch over between different radio systems."@en ;
    rdfs:domain [ a owl:Class ;
            owl:unionOf ( <SubsetWithCommonCharacteristics> <Track> ) ] ;
    rdfs:isDefinedBy <> ;
    rdfs:range xsd:anyURI ;
    ns1:term_status "stable" .

<isQuietRoute> a owl:DatatypeProperty,
        owl:FunctionalProperty ;
    rdfs:label "Belonging to a quieter route"@en ;
    <XMLName> "IHS_QuietRoute" ;
    <rinfIndex> "1.1.1.1.7.11" ;
    dcterms:created "2020-11-04"^^xsd:date ;
    dcterms:modified "2024-01-08"^^xsd:date ;
    rdfs:comment "Belonging to a ‘quieter route’ in accordance with Article 5b of TSI NOI."@en ;
    rdfs:domain [ a owl:Class ;
            owl:unionOf ( <SubsetWithCommonCharacteristics> <Track> ) ] ;
    rdfs:isDefinedBy <> ;
    rdfs:range xsd:boolean ;
    ns1:term_status "stable" .

<legacyRadioSystem> a owl:ObjectProperty ;
    rdfs:label "Other radio systems installed (Radio Legacy Systems)"@en ;
    <XMLName> "CRS_Installed" ;
    <appendixD2Index> "3.2.8" ;
    <eratvIndex> "4.13.2.3" ;
    <inSkosConceptScheme> <concepts/legacy-radio-systems/LegacyRadioSystems> ;
    <rinfIndex> "1.1.1.3.6.1",
        "1.2.1.1.5.1" ;
    <usedInRCCCalculations> true ;
    dcterms:created "2020-08-31"^^xsd:date ;
    dcterms:modified "2021-09-12"^^xsd:date ;
    dcterms:source <https://eur-lex.europa.eu/eli/reg_impl/2019/773/oj> ;
    rdfs:comment "Indication of radio legacy systems installed."@en ;
    rdfs:domain [ a owl:Class ;
            owl:unionOf ( <SubsetWithCommonCharacteristics> <Track> <VehicleType> ) ] ;
    rdfs:isDefinedBy <> ;
    rdfs:range ns2:Concept ;
    ns1:term_status "stable" .

<lengthOfPlatform> a owl:DatatypeProperty ;
    rdfs:label "Usable length of platform"@en ;
    <XMLName> "IPL_Length" ;
    <rinfIndex> "1.2.1.0.6.4" ;
    <unitOfMeasure> <http://qudt.org/vocab/unit/M> ;
    <usedInRCCCalculations> true ;
    dcterms:created "2024-05-16"^^xsd:date ;
    rdfs:comment "The maximum continuous length (expressed in metres) of that part of platform in front of which a train is intended to remain stationary in normal operating conditions for passengers to board and alight from the train, making appropriate allowance for stopping tolerances."@en ;
    rdfs:domain <PlatformEdge> ;
    rdfs:isDefinedBy <> ;
    rdfs:range xsd:double ;
    rdfs:subPropertyOf <length> ;
    ns1:term_status "stable" .

<lengthOfSectionOfLine> a owl:DatatypeProperty ;
    rdfs:label "Length of section of line"@en ;
    <XMLName> "SOLLength" ;
    <rinfIndex> "1.1.0.0.0.5" ;
    <unitOfMeasure> <http://qudt.org/vocab/unit/KiloM> ;
    <usedInRCCCalculations> true ;
    dcterms:created "2024-05-16"^^xsd:date ;
    rdfs:comment "Length between operational points at start and end of section of line."@en ;
    rdfs:domain <SectionOfLine> ;
    rdfs:isDefinedBy <> ;
    rdfs:range xsd:double ;
    rdfs:subPropertyOf <length> ;
    ns1:term_status "stable" .

<lengthOfSiding> a owl:DatatypeProperty ;
    rdfs:label "Usable length of siding"@en ;
    <XMLName> "IPP_Length" ;
    <rinfIndex> "1.2.2.0.2.1" ;
    <unitOfMeasure> <http://qudt.org/vocab/unit/M> ;
    <usedInRCCCalculations> true ;
    dcterms:created "2024-05-16"^^xsd:date ;
    rdfs:comment """Total length of the siding/stabling track expressed in metres
where trains can be parked safely."""@en ;
    rdfs:domain <Siding> ;
    rdfs:isDefinedBy <> ;
    rdfs:range xsd:double ;
    rdfs:subPropertyOf <length> ;
    ns1:term_status "stable" .

<lengthOfTunnel> a owl:DatatypeProperty ;
    rdfs:label "Length of tunnel"@en ;
    <XMLName> "ITU_Length" ;
    <rinfIndex> "1.1.1.1.8.7",
        "1.2.1.0.5.5",
        "1.2.2.0.5.5" ;
    <unitOfMeasure> <http://qudt.org/vocab/unit/M> ;
    <usedInRCCCalculations> true ;
    dcterms:created "2024-05-16"^^xsd:date ;
    rdfs:comment "Length of a tunnel in metres from entrance portal to exit portal."@en ;
    rdfs:domain <Tunnel> ;
    rdfs:isDefinedBy <> ;
    rdfs:range xsd:double ;
    rdfs:subPropertyOf <length> ;
    ns1:term_status "stable" .

<lineCategory> a owl:ObjectProperty ;
    rdfs:label "Category of line"@en ;
    <XMLName> "IPP_LineCat" ;
    <inSkosConceptScheme> <concepts/line-category/LineCategories> ;
    <rinfIndex> "1.1.1.1.2.2",
        "1.2.1.0.2.2" ;
    dcterms:created "2021-08-02"^^xsd:date ;
    dcterms:modified "2024-01-08"^^xsd:date ;
    rdfs:comment "Classification of a line according to the TSI INF."@en ;
    rdfs:domain [ a owl:Class ;
            owl:unionOf ( <SubsetWithCommonCharacteristics> <Track> ) ] ;
    rdfs:isDefinedBy <> ;
    rdfs:range ns2:Concept ;
    ns1:term_status "stable" .

<linesideDistanceIndicationAppearance> a owl:ObjectProperty ;
    rdfs:label "Lineside distance indication appearance"@en ;
    <appendixD2Index> "3.1.3" ;
    <rinfIndex> "1.1.1.0.0.3" ;
    dcterms:created "2022-10-27"^^xsd:date ;
    dcterms:modified "2023-03-14"^^xsd:date ;
    dcterms:source <https://eur-lex.europa.eu/eli/reg_impl/2019/773/oj> ;
    rdfs:comment "Indication of types of appearance of track lineside distance indications."@en ;
    rdfs:domain [ a owl:Class ;
            owl:unionOf ( <SubsetWithCommonCharacteristics> <Track> ) ] ;
    rdfs:isDefinedBy <> ;
    rdfs:range ns2:Concept ;
    ns1:term_status "unstable" .

<linesideDistanceIndicationFrequency> a owl:DatatypeProperty ;
    rdfs:label "Lineside distance indication frequency"@en ;
    <appendixD2Index> "3.1.3" ;
    <rinfIndex> "1.1.1.0.0.3" ;
    dcterms:created "2022-10-27"^^xsd:date ;
    dcterms:modified "2023-03-14"^^xsd:date ;
    dcterms:source <https://eur-lex.europa.eu/eli/reg_impl/2019/773/oj> ;
    rdfs:comment "Frequency of track lineside distance indications."@en ;
    rdfs:domain [ a owl:Class ;
            owl:unionOf ( <SubsetWithCommonCharacteristics> <Track> ) ] ;
    rdfs:isDefinedBy <> ;
    rdfs:range xsd:integer ;
    ns1:term_status "stable" .

<linesideDistanceIndicationPositioning> a owl:ObjectProperty ;
    rdfs:label "Lineside distance indication positioning"@en ;
    <appendixD2Index> "3.1.3" ;
    <rinfIndex> "1.1.1.0.0.3" ;
    dcterms:created "2023-03-14"^^xsd:date ;
    dcterms:source <https://eur-lex.europa.eu/eli/reg_impl/2019/773/oj> ;
    rdfs:comment "Indication of the side along the track where the lineside indication is positioned (left or right)."@en ;
    rdfs:domain [ a owl:Class ;
            owl:unionOf ( <SubsetWithCommonCharacteristics> <Track> ) ] ;
    rdfs:isDefinedBy <> ;
    rdfs:range ns2:Concept ;
    rdfs:subPropertyOf owl:topObjectProperty ;
    ns1:term_status "unstable" .

<loadCapability> a owl:ObjectProperty ;
    rdfs:label "Load Capability"@en ;
    <XMLName> "IPP_LoadCap" ;
    <inSkosConceptScheme> <concepts/load-capabilities/LoadCapabilities> ;
    <rinfIndex> "1.1.1.1.2.4" ;
    dcterms:created "2020-08-24"^^xsd:date ;
    dcterms:isReplacedBy <LoadCapability>,
        <loadCapabilityLineCategory>,
        <loadCapabilitySpeed>,
        <trackLoadCapability> ;
    dcterms:modified "2023-01-20"^^xsd:date ;
    rdfs:comment "A combination of the line category and speed at the weakest point of the track.The reason for deprecation is that the load capability property 1.1.1.1.2.4 was defined incorrectly as a SKOS property. It is composed of two values: (1)  line category, and (2) speed. Only line category is a list of predefined values (SKOS), whereas speed is an integer (according to the RINF application guide)."@en ;
    rdfs:domain [ a owl:Class ;
            owl:unionOf ( <SubsetWithCommonCharacteristics> <Track> ) ] ;
    rdfs:isDefinedBy <> ;
    rdfs:range ns2:Concept ;
    owl:deprecated true ;
    ns1:term_status "stable" .

<localRulesOrRestrictions> a owl:DatatypeProperty ;
    rdfs:label "Existence of rules and restrictions of a strictly local nature"@en ;
    <XMLName> "RUL_LocalRulesOrRestrictions" ;
    <rinfIndex> "1.1.1.4.1",
        "1.2.3.1" ;
    dcterms:created "2021-08-09"^^xsd:date ;
    dcterms:modified "2021-09-12"^^xsd:date ;
    rdfs:comment "Existence of rules and restrictions of a strictly local nature."@en ;
    rdfs:domain [ a owl:Class ;
            owl:unionOf ( <OperationalPoint> <Track> ) ] ;
    rdfs:isDefinedBy <> ;
    rdfs:range xsd:boolean ;
    ns1:term_status "stable" .

<localRulesOrRestrictionsDoc> a owl:ObjectProperty ;
    rdfs:label "Documents regarding the rules or restrictions of a strictly local nature available by the IM"@en ;
    <XMLName> "RUL_LocalRulesOrRestrictionsDocRef" ;
    <rinfIndex> "1.1.1.4.2",
        "1.2.3.2" ;
    dcterms:created "2021-08-09"^^xsd:date ;
    dcterms:modified "2024-04-23"^^xsd:date ;
    rdfs:comment "Electronic document available from the IM stored by the Agency providing additional information."@en ;
    rdfs:domain [ a owl:Class ;
            owl:unionOf ( <OperationalPoint> <Track> ) ] ;
    rdfs:isDefinedBy <> ;
    rdfs:range <Document> ;
    ns1:term_status "stable" ;
    ns2:changeNote "Change from datatype property to object property in order to point to the class Document (reference document)"@en .

<mNvcontact> a owl:ObjectProperty ;
    rdfs:label "M_NVCONTACT"@en ;
    <appendixD3Index> "1.5.9" ;
    <rinfIndex> "1.1.1.3.2.16.9",
        "1.2.1.1.1.16.9 " ;
    dcterms:created "2022-11-07"^^xsd:date ;
    dcterms:modified "2023-03-14"^^xsd:date ;
    rdfs:comment """On-Board system reaction when T_NVCONTACT expires.  
According to the specification referenced in Appendix A-1, index [C]. 
In https://www.era.europa.eu/sites/default/files/filesystem/ertms/ccs_tsi_annex_a_-_mandatory_specifications/set_of_specifications_3_etcs_b3_r2_gsm-r_b1/index004_-_subset-026_v360.zip
 Subset 26, chapter 7. 7.5.1.74 M_NVCONTACT."""@en ;
    rdfs:domain [ a owl:Class ;
            owl:unionOf ( <SubsetWithCommonCharacteristics> <Track> ) ] ;
    rdfs:isDefinedBy <> ;
    rdfs:range ns2:Concept ;
    ns1:term_status "unstable" .

<mNvderun> a owl:DatatypeProperty ;
    rdfs:label "M_NVDERUN"@en ;
    <appendixD3Index> "1.5.10" ;
    <rinfIndex> "1.1.1.3.2.16.10",
        "1.2.1.1.1.16.10 " ;
    dcterms:created "2022-11-07"^^xsd:date ;
    dcterms:modified "2023-03-14"^^xsd:date ;
    rdfs:comment """Entry of Driver ID permitted while running. According to the specification referenced in Appendix A-1, index [C]. 
In https://www.era.europa.eu/sites/default/files/filesystem/ertms/ccs_tsi_annex_a_-_mandatory_specifications/set_of_specifications_3_etcs_b3_r2_gsm-r_b1/index004_-_subset-026_v360.zip
 Subset 26, chapter 7. 7.5.1.75 M_NVDERUN."""@en ;
    rdfs:domain [ a owl:Class ;
            owl:unionOf ( <SubsetWithCommonCharacteristics> <Track> ) ] ;
    rdfs:isDefinedBy <> ;
    rdfs:range xsd:boolean ;
    ns1:term_status "stable" .

<magneticBraking> a owl:FunctionalProperty,
        owl:ObjectProperty ;
    rdfs:label "Use of magnetic brakes"@en ;
    <XMLName> "ILR_MagneticBrakes" ;
    <appendixD2Index> "3.4.6" ;
    <inSkosConceptScheme> <concepts/magnetic-braking/MagneticBraking> ;
    <rinfIndex> "1.1.1.1.6.3",
        "1.2.1.0.4.3" ;
    <usedInRCCCalculations> true ;
    dcterms:created "2020-08-24"^^xsd:date ;
    dcterms:modified "2022-09-12"^^xsd:date ;
    dcterms:source <https://eur-lex.europa.eu/eli/reg_impl/2019/773/oj> ;
    rdfs:comment "Indication of limitations on the use of magnetic brakes."@en,
        "This property has been modified to be a RINF parameter (its eratvIndex is deleted). It is treated as a SKOS by RINF and as a boolean by ERATV. A new ERATV datatype property has been defined, magneticBrakingFitted with boolean values."@en ;
    rdfs:domain [ a owl:Class ;
            owl:unionOf ( <SubsetWithCommonCharacteristics> <Track> ) ] ;
    rdfs:isDefinedBy <> ;
    rdfs:range ns2:Concept ;
    ns1:term_status "stable" .

<magneticBrakingConditionsDocument> a owl:ObjectProperty ;
    rdfs:label "Document with the conditions for the use of magnetic brakes"@en ;
    <XMLName> "ILR_MBDocRef" ;
    <appendixD2Index> "3.4.6" ;
    <rinfIndex> "1.1.1.1.6.5" ;
    <usedInRCCCalculations> true ;
    dcterms:created "2020-08-24"^^xsd:date ;
    dcterms:modified "2024-04-23"^^xsd:date ;
    dcterms:source <https://eur-lex.europa.eu/eli/reg_impl/2019/773/oj> ;
    rdfs:comment "Electronic document available in two EU languages from the IM stored by the Agency with conditions for the use of magnetic brakes identified in 1.1.1.1.6.3."@en ;
    rdfs:domain [ a owl:Class ;
            owl:unionOf ( <SubsetWithCommonCharacteristics> <Track> ) ] ;
    rdfs:isDefinedBy <> ;
    rdfs:range <Document> ;
    ns1:term_status "stable" ;
    ns2:changeNote "Change from datatype property to object property in order to point to the class Document (reference document)"@en .

<maxDistEndTrainFirstAxle> a owl:DatatypeProperty ;
    rdfs:label "Maximum distance between end of train and first axle"@en ;
    <XMLName> "CTD_MaxDistEndTrainFirstAxle" ;
    <rinfIndex> "1.1.1.3.7.5" ;
    <unitOfMeasure> <http://qudt.org/vocab/unit/MilliM> ;
    dcterms:created "2021-08-08"^^xsd:date ;
    dcterms:modified "2023-03-14"^^xsd:date ;
    rdfs:comment "Deprecated according to the ammendment to the Regulation (EU) 2019/777. Indication of maximum distance between end of train and first axle, given in millimetres, applicable for both sides (front and rear) of a vehicle or train."@en ;
    rdfs:domain <TrainDetectionSystem> ;
    rdfs:isDefinedBy <> ;
    rdfs:range xsd:integer ;
    owl:deprecated true ;
    ns1:term_status "stable" .

<maxSandingOutput> a owl:ObjectProperty ;
    rdfs:label "Maximum amount of sand"@en ;
    <XMLName> "CTD_MaxSandOutput" ;
    <inSkosConceptScheme> <concepts/max-amount-sandings/MaxAmountSandings> ;
    <rinfIndex> "1.1.1.3.7.17" ;
    dcterms:created "2021-08-08"^^xsd:date ;
    dcterms:modified "2023-03-14"^^xsd:date ;
    rdfs:comment """Maximum amount of sand accepted on the track within value of sanding output for 30s, given in grams.
Deprecated according to the ammendment to the Regulation (EU) 2019/777."""@en ;
    rdfs:domain <TrainDetectionSystem> ;
    rdfs:isDefinedBy <> ;
    rdfs:range ns2:Concept ;
    owl:deprecated true ;
    ns1:term_status "stable" .

<maxTrainCurrent> a owl:DatatypeProperty ;
    rdfs:label "Maximum train current"@en ;
    <XMLName> "ECS_MaxTrainCurrent" ;
    <appendixD2Index> "3.3.2" ;
    <rinfIndex> "1.1.1.2.2.2" ;
    <unitOfMeasure> <http://qudt.org/vocab/unit/A> ;
    dcterms:created "2021-08-06"^^xsd:date ;
    dcterms:modified "2021-08-06"^^xsd:date ;
    dcterms:source "https://wiki2.railml.org/wiki/IS:maxTrainCurrent_electrification"^^xsd:anyURI ;
    rdfs:comment "Indication of the maximum allowable train current expressed in amperes."@en ;
    rdfs:domain <ContactLineSystem> ;
    rdfs:isDefinedBy <> ;
    rdfs:range xsd:integer ;
    ns1:term_status "stable" .

<maximumAltitude> a owl:DatatypeProperty,
        owl:FunctionalProperty ;
    rdfs:label "Maximum altitude"@en ;
    <rinfIndex> "1.1.1.1.2.7" ;
    <unitOfMeasure> <http://qudt.org/vocab/unit/M> ;
    dcterms:created "2021-08-03"^^xsd:date ;
    dcterms:modified "2022-10-20"^^xsd:date ;
    rdfs:comment "Highest point of the section of line above sea level in reference to Normal Amsterdam's Peil (NAP)."@en ;
    rdfs:domain [ a owl:Class ;
            owl:unionOf ( <SubsetWithCommonCharacteristics> <Track> ) ] ;
    rdfs:isDefinedBy <> ;
    rdfs:range xsd:double ;
    ns1:term_status "stable" .

<maximumContactWireHeight> a owl:DatatypeProperty,
        owl:FunctionalProperty ;
    rdfs:label "Maximum contact wire height"@en ;
    <XMLName> "ECS_MaxWireHeight" ;
    <eratvIndex> "4.10.5" ;
    <rinfIndex> "1.1.1.2.2.5" ;
    <unitOfMeasure> <http://qudt.org/vocab/unit/M> ;
    <usedInRCCCalculations> true ;
    dcterms:created "2020-08-25"^^xsd:date ;
    dcterms:modified "2021-09-11"^^xsd:date ;
    rdfs:comment "Indication of the maximum contact wire height expressed in metres."@en ;
    rdfs:domain [ a owl:Class ;
            owl:unionOf ( <SubsetWithCommonCharacteristics> <Track> <VehicleType> ) ] ;
    rdfs:isDefinedBy <> ;
    rdfs:range xsd:double ;
    ns1:term_status "stable" .

<maximumInterferenceCurrent> a owl:DatatypeProperty ;
    rdfs:label "Maximum interference current"@en ;
    <rinfIndex> "1.1.1.3.4.2.1",
        "1.2.1.1.3.2.1" ;
    dcterms:created "2023-03-14"^^xsd:date ;
    rdfs:comment "Maximum interference current limits allowed for track circuits for a defined frequency band."@en ;
    rdfs:domain <TrainDetectionSystem> ;
    rdfs:isDefinedBy <> ;
    rdfs:range xsd:integer ;
    ns1:term_status "stable" .

<maximumPermittedSpeed> a owl:DatatypeProperty,
        owl:FunctionalProperty ;
    rdfs:label "Maximum permitted speed"@en ;
    <XMLName> "IPP_MaxSpeed" ;
    <appendixD2Index> "3.1.4" ;
    <rinfIndex> "1.1.1.1.2.5" ;
    <unitOfMeasure> <http://qudt.org/vocab/unit/KiloM-PER-HR> ;
    <usedInRCCCalculations> true ;
    dcterms:created "2020-08-24"^^xsd:date ;
    dcterms:modified "2023-03-14"^^xsd:date ;
    rdfs:comment "Nominal maximum operational speed on the line as a result of infrastructure, energy and control, command and signalling subsystem characteristics expressed in kilometres/hour."@en ;
    rdfs:domain [ a owl:Class ;
            owl:unionOf ( <SubsetWithCommonCharacteristics> <Track> ) ] ;
    rdfs:isDefinedBy <> ;
    rdfs:range xsd:integer ;
    ns1:term_status "stable" .

<maximumTemperature> a owl:DatatypeProperty ;
    rdfs:label "Temperature range (maximum)"@en ;
    <XMLName> "IPP_TempRange" ;
    <eratvIndex> "4.3.1" ;
    <rinfIndex> "1.1.1.1.2.6" ;
    <usedInRCCCalculations> true ;
    dcterms:created "2020-08-24"^^xsd:date ;
    dcterms:modified "2021-09-10"^^xsd:date ;
    rdfs:comment "Maximum temperature allowed for unrestricted operation access, according to European standard."@en ;
    rdfs:domain [ a owl:Class ;
            owl:unionOf ( <SubsetWithCommonCharacteristics> <Track> <VehicleType> ) ] ;
    rdfs:isDefinedBy <> ;
    rdfs:range xsd:integer ;
    ns1:term_status "stable" .

<maximumTrainDeceleration> a owl:DatatypeProperty,
        owl:FunctionalProperty ;
    rdfs:label "Maximum train deceleration"@en ;
    <XMLName> "ILR_MaxDeceleration" ;
    <rinfIndex> "1.1.1.1.6.1" ;
    <usedInRCCCalculations> true ;
    dcterms:created "2020-08-24"^^xsd:date ;
    dcterms:modified "2021-09-10"^^xsd:date ;
    rdfs:comment "Limit for longitudinal track resistance given as a maximum allowed train deceleration and expressed in metres per square second."@en ;
    rdfs:domain [ a owl:Class ;
            owl:unionOf ( <SubsetWithCommonCharacteristics> <Track> ) ] ;
    rdfs:isDefinedBy <> ;
    rdfs:range xsd:double ;
    ns1:term_status "stable" .

<minDistConsecutiveAxles> a owl:DatatypeProperty ;
    rdfs:label "Minimum permitted distance between two consecutive axles"@en ;
    <XMLName> "CTD_MinDistConsecutiveAxles" ;
    <eratvIndex> "4.14.2.2" ;
    <rinfIndex> "1.1.1.3.7.3" ;
    <unitOfMeasure> <http://qudt.org/vocab/unit/MilliM> ;
    dcterms:created "2021-08-08"^^xsd:date ;
    dcterms:modified "2023-03-14"^^xsd:date ;
    rdfs:comment "Deprecated according to the ammendment to the Regulation (EU) 2019/777. However, the parameter remains as it is also an ERATV parameter."@en,
        "Indication of minimum permitted distance between two consecutive axles, given in millimetres."@en ;
    rdfs:domain [ a owl:Class ;
            owl:unionOf ( <SubsetWithCommonCharacteristics> <Track> <VehicleType> ) ] ;
    rdfs:isDefinedBy <> ;
    rdfs:range xsd:integer ;
    ns1:term_status "stable" .

<minDistFirstLastAxle> a owl:DatatypeProperty ;
    rdfs:label "Minimum permitted distance between first and last axle"@en ;
    <XMLName> "CTD_MinDistFirstLastAxles" ;
    <eratvIndex> "4.14.2.3" ;
    <rinfIndex> "1.1.1.3.7.4" ;
    <unitOfMeasure> <http://qudt.org/vocab/unit/MilliM> ;
    dcterms:created "2021-08-08"^^xsd:date ;
    dcterms:modified "2023-03-14"^^xsd:date ;
    rdfs:comment "Deprecated according to the ammendment to the Regulation (EU) 2019/777. However, the parameter remains as it is also an ERATV parameter."@en,
        "Indication of minimum permitted distance between first and last axles, given in millimetres."@en ;
    rdfs:domain [ a owl:Class ;
            owl:unionOf ( <SubsetWithCommonCharacteristics> <Track> <VehicleType> ) ] ;
    rdfs:isDefinedBy <> ;
    rdfs:range xsd:integer ;
    ns1:term_status "stable" .

<minFlangeHeight> a owl:DatatypeProperty ;
    rdfs:label "Minimum permitted height of the flange"@en ;
    <XMLName> "CTD_MinFlangeHeight" ;
    <eratvIndex> "4.14.2.8" ;
    <rinfIndex> "1.1.1.3.7.9" ;
    <unitOfMeasure> <http://qudt.org/vocab/unit/MilliM> ;
    dcterms:created "2021-08-08"^^xsd:date ;
    dcterms:modified "2021-09-01"^^xsd:date ;
    rdfs:comment "Deprecated according to the ammendment to the Regulation (EU) 2019/777. However, the parameter remains as it is also an ERATV parameter."@en,
        "Minimum permitted flange height, given in millimiters."@en ;
    rdfs:domain [ a owl:Class ;
            owl:unionOf ( <SubsetWithCommonCharacteristics> <Track> <VehicleType> ) ] ;
    rdfs:isDefinedBy <> ;
    rdfs:range xsd:double ;
    ns1:term_status "stable" .

<minFlangeThickness> a owl:DatatypeProperty ;
    rdfs:label "Minimum permitted thickness of the flange"@en ;
    <XMLName> "CTD_MinFlangeThickness" ;
    <eratvIndex> "4.14.2.7" ;
    <rinfIndex> "1.1.1.3.7.8" ;
    <unitOfMeasure> <http://qudt.org/vocab/unit/MilliM> ;
    dcterms:created "2021-08-08"^^xsd:date ;
    dcterms:modified "2021-09-01"^^xsd:date ;
    rdfs:comment "Deprecated according to the ammendment to the Regulation (EU) 2019/777. However, the parameter remains as it is also an ERATV parameter."@en,
        "Minimum permitted flange thickness, given in millimiters."@en ;
    rdfs:domain [ a owl:Class ;
            owl:unionOf ( <SubsetWithCommonCharacteristics> <Track> <VehicleType> ) ] ;
    rdfs:isDefinedBy <> ;
    rdfs:range xsd:double ;
    ns1:term_status "stable" .

<minRimWidth> a owl:DatatypeProperty ;
    rdfs:label "Minimum permitted width of the rim"@en ;
    <XMLName> "CTD_MinRimWidth" ;
    <eratvIndex> "4.14.2.5" ;
    <rinfIndex> "1.1.1.3.7.6" ;
    <unitOfMeasure> <http://qudt.org/vocab/unit/MilliM> ;
    dcterms:created "2021-08-08"^^xsd:date ;
    dcterms:modified "2023-03-14"^^xsd:date ;
    rdfs:comment "Deprecated according to the ammendment to the Regulation (EU) 2019/777. However, the parameter remains as it is also an ERATV parameter."@en ;
    rdfs:domain [ a owl:Class ;
            owl:unionOf ( <SubsetWithCommonCharacteristics> <Track> <VehicleType> ) ] ;
    rdfs:isDefinedBy <> ;
    rdfs:range xsd:double ;
    ns1:term_status "stable" .

<minWheelDiameter> a owl:DatatypeProperty ;
    rdfs:label "Minimum permitted wheel diameter"@en ;
    <XMLName> "CTD_MinWheelDiameter" ;
    <eratvIndex> "4.14.2.6" ;
    <rinfIndex> "1.1.1.3.7.7" ;
    <unitOfMeasure> <http://qudt.org/vocab/unit/MilliM> ;
    dcterms:created "2021-08-08"^^xsd:date ;
    dcterms:modified "2023-03-14"^^xsd:date ;
    rdfs:comment "Deprecated according to the ammendment to the Regulation (EU) 2019/777. However, the parameter remains as it is also an ERATV parameter."@en,
        "Minimum permitted wheel diameter, given in millimiters."@en ;
    rdfs:domain [ a owl:Class ;
            owl:unionOf ( <SubsetWithCommonCharacteristics> <Track> <VehicleType> ) ] ;
    rdfs:isDefinedBy <> ;
    rdfs:range xsd:integer ;
    ns1:term_status "stable" .

<minimumContactWireHeight> a owl:DatatypeProperty,
        owl:FunctionalProperty ;
    rdfs:label "Minimum contact wire height"@en ;
    <XMLName> "ECS_MinWireHeight" ;
    <eratvIndex> "4.10.5" ;
    <rinfIndex> "1.1.1.2.2.6" ;
    <unitOfMeasure> <http://qudt.org/vocab/unit/M> ;
    <usedInRCCCalculations> true ;
    dcterms:created "2020-08-25"^^xsd:date ;
    dcterms:modified "2021-09-11"^^xsd:date ;
    rdfs:comment "Indication of the minimum contact wire height expressed in metres."@en ;
    rdfs:domain [ a owl:Class ;
            owl:unionOf ( <SubsetWithCommonCharacteristics> <Track> <VehicleType> ) ] ;
    rdfs:isDefinedBy <> ;
    rdfs:range xsd:double ;
    ns1:term_status "stable" .

<minimumHorizontalRadius> a owl:DatatypeProperty,
        owl:FunctionalProperty ;
    rdfs:label "Minimum radius of horizontal curve"@en ;
    <XMLName> "ILL_MinRadHorzCurve" ;
    <eratvIndex> "4.8.4" ;
    <rinfIndex> "1.1.1.1.3.7",
        "1.2.2.0.3.2" ;
    <unitOfMeasure> <http://qudt.org/vocab/unit/M> ;
    <usedInRCCCalculations> true ;
    dcterms:created "2020-08-24"^^xsd:date ;
    dcterms:modified "2021-09-10"^^xsd:date ;
    rdfs:comment "Radius of the smallest horizontal curve of the track in metres."@en ;
    rdfs:domain [ a owl:Class ;
            owl:unionOf ( <Siding> <SubsetWithCommonCharacteristics> <Track> <VehicleType> ) ] ;
    rdfs:isDefinedBy <> ;
    rdfs:range xsd:integer ;
    ns1:term_status "stable" .

<minimumTemperature> a owl:DatatypeProperty ;
    rdfs:label "Temperature range (minimum)"@en ;
    <XMLName> "IPP_TempRange" ;
    <eratvIndex> "4.3.1" ;
    <rinfIndex> "1.1.1.1.2.6" ;
    <usedInRCCCalculations> true ;
    dcterms:created "2020-08-24"^^xsd:date ;
    dcterms:modified "2021-09-10"^^xsd:date ;
    rdfs:comment "Minimum temperature allowed for unrestricted operation access, according to European standard."@en ;
    rdfs:domain [ a owl:Class ;
            owl:unionOf ( <SubsetWithCommonCharacteristics> <Track> <VehicleType> ) ] ;
    rdfs:isDefinedBy <> ;
    rdfs:range xsd:integer ;
    ns1:term_status "stable" .

<minimumVerticalRadius> a owl:DatatypeProperty,
        owl:FunctionalProperty ;
    rdfs:label "Minimum radius of vertical curve"@en ;
    <XMLName> "ILL_MinRadVertCurve" ;
    <rinfIndex> "1.2.2.0.3.3" ;
    <unitOfMeasure> <http://qudt.org/vocab/unit/M> ;
    dcterms:created "2020-08-24"^^xsd:date ;
    dcterms:isReplacedBy <minimumVerticalRadiusCrest>,
        <minimumVerticalRadiusHollow> ;
    dcterms:modified "2023-04-05"^^xsd:date ;
    rdfs:comment """Radius of the smallest vertical curve expressed in metres. 
Deprecated because of replacement by  two integer properties The reason is that the property is composed of two values: The first ‘NNN’ is a value of crest, the second ‘NNN’ is a value of hollow, both expressed in metres."""@en ;
    rdfs:domain <Siding> ;
    rdfs:isDefinedBy <> ;
    rdfs:range xsd:string ;
    owl:deprecated true ;
    ns1:term_status "stable" .

<minimumWheelDiameter> a owl:DatatypeProperty,
        owl:FunctionalProperty ;
    rdfs:label "Minimum wheel diameter for fixed obtuse crossings"@en ;
    <XMLName> "ISC_MinWheelDiaFixObtuseCrossings" ;
    <eratvIndex> "4.8.2" ;
    <rinfIndex> "1.1.1.1.5.2" ;
    <unitOfMeasure> <http://qudt.org/vocab/unit/MilliM> ;
    <usedInRCCCalculations> true ;
    dcterms:created "2020-08-24"^^xsd:date ;
    dcterms:modified "2021-09-10"^^xsd:date ;
    rdfs:comment "Maximum unguided length of fixed obtuse crossings is based on a minimum wheel diameter in service expressed in millimetres."@en ;
    rdfs:domain [ a owl:Class ;
            owl:unionOf ( <SubsetWithCommonCharacteristics> <Track> <VehicleType> ) ] ;
    rdfs:isDefinedBy <> ;
    rdfs:range xsd:integer ;
    ns1:term_status "stable" .

<multipleTrainProtectionRequired> a owl:DatatypeProperty,
        owl:FunctionalProperty ;
    rdfs:label "Need for more than one train protection, control and warning system required on board"@en ;
    <rinfIndex> "1.1.1.3.5.2" ;
    dcterms:created "2021-08-09"^^xsd:date ;
    dcterms:modified "2023-03-14"^^xsd:date ;
    rdfs:comment "Deprecated according to the ammendment to the Regulation (EU) 2019/777. Indication whether more than one train protection, control and warning system is required to be on-board and active simultaneously."@en ;
    rdfs:domain [ a owl:Class ;
            owl:unionOf ( <SubsetWithCommonCharacteristics> <Track> ) ] ;
    rdfs:isDefinedBy <> ;
    rdfs:range xsd:boolean ;
    owl:deprecated true ;
    ns1:term_status "unstable" .

<nationalLoadCapability> a owl:DatatypeProperty ;
    rdfs:label "National classification for load capability"@en ;
    <XMLName> "IPP_NCLoadCap" ;
    <rinfIndex> "1.1.1.1.2.4.1" ;
    <usedInRCCCalculations> true ;
    dcterms:created "2020-08-24"^^xsd:date ;
    dcterms:modified "2021-09-10"^^xsd:date ;
    rdfs:comment "National classification for load capability."@en ;
    rdfs:domain [ a owl:Class ;
            owl:unionOf ( <SubsetWithCommonCharacteristics> <Track> ) ] ;
    rdfs:isDefinedBy <> ;
    rdfs:range xsd:string ;
    ns1:term_status "stable" .

<nationalRollingStockFireCategory> a owl:DatatypeProperty,
        owl:FunctionalProperty ;
    rdfs:label "National fire category of rolling stock required"@en ;
    <XMLName> "ITU_NatFireCatReq" ;
    <rinfIndex> "1.1.1.1.8.11",
        "1.2.1.0.5.8",
        "1.2.2.0.5.8" ;
    <usedInRCCCalculations> true ;
    dcterms:created "2020-07-29"^^xsd:date ;
    dcterms:modified "2024-01-08"^^xsd:date ;
    rdfs:comment "Categorisation how a passenger train with a fire on board will continue to operate for a defined time period - according to national rules if they exist."@en ;
    rdfs:domain <Tunnel> ;
    rdfs:isDefinedBy <> ;
    rdfs:range xsd:string ;
    ns1:term_status "stable" .

<nationalValuesBrakeModel> a owl:DatatypeProperty ;
    rdfs:label "National Values used for the brake model"@en ;
    <rinfIndex> "1.1.1.3.2.16.13",
        "1.2.1.1.1.16.13" ;
    dcterms:created "2023-03-14"^^xsd:date ;
    dcterms:modified "2024-01-08"^^xsd:date ;
    rdfs:comment """Set of parameters for adapting the braking curves calculated by the ETCS on-board system to match accuracy, performance and safety margins imposed by the infrastructure manager.
It copies the content of Packet 3 or of Packet 203 as defined in the specification referenced in Appendix A-1, index [C]."""@en ;
    rdfs:domain [ a owl:Class ;
            owl:unionOf ( <SubsetWithCommonCharacteristics> <Track> ) ] ;
    rdfs:isDefinedBy <> ;
    rdfs:range xsd:string ;
    ns1:term_status "stable" .

<opName> a owl:DatatypeProperty,
        owl:FunctionalProperty ;
    rdfs:label "Name of operational point"@en ;
    <XMLName> "OPName" ;
    <appendixD2Index> "2.3.1" ;
    <rinfIndex> "1.2.0.0.0.1" ;
    dcterms:created "2021-09-13"^^xsd:date ;
    dcterms:modified "2021-09-13"^^xsd:date ;
    dcterms:source <https://eur-lex.europa.eu/eli/reg_impl/2019/773/oj> ;
    rdfs:comment "Name normally related to the town or village or to traffic control purpose."@en ;
    rdfs:domain <OperationalPoint> ;
    rdfs:isDefinedBy <> ;
    rdfs:range xsd:string ;
    ns1:term_status "stable" .

<opType> a owl:FunctionalProperty,
        owl:ObjectProperty ;
    rdfs:label "Type of operational point"@en ;
    <XMLName> "OPType" ;
    <appendixD2Index> "2.2.2",
        "2.3.2" ;
    <inSkosConceptScheme> <concepts/op-types/OperationalPointTypes> ;
    <rinfIndex> "1.2.0.0.0.4" ;
    dcterms:created "2020-07-29"^^xsd:date ;
    dcterms:modified "2021-08-03"^^xsd:date ;
    dcterms:source <https://eur-lex.europa.eu/eli/reg_impl/2019/773/oj> ;
    rdfs:comment "Type of facility in relation to the dominating operational functions."@en ;
    rdfs:domain <OperationalPoint> ;
    rdfs:isDefinedBy <> ;
    rdfs:range ns2:Concept ;
    ns1:term_status "stable" .

<opTypeGaugeChangeover> a owl:DatatypeProperty,
        owl:FunctionalProperty ;
    rdfs:label "Type of track gauge changeover facility"@en ;
    <XMLName> "OPTypeGaugeChangeover" ;
    <rinfIndex> "1.2.0.0.0.4.1" ;
    <usedInRCCCalculations> true ;
    dcterms:created "2021-08-11"^^xsd:date ;
    dcterms:modified "2021-08-11"^^xsd:date ;
    rdfs:comment "Type of track gauge changeover facility."@en ;
    rdfs:domain <OperationalPoint> ;
    rdfs:isDefinedBy <> ;
    rdfs:range xsd:string ;
    ns1:term_status "stable" .

<osmClass> a owl:ObjectProperty ;
    rdfs:label "Open street map class"@en ;
    <inSkosConceptScheme> <concepts/osmclass/OSMClasses> ;
    rdfs:domain [ a owl:Class ;
            owl:unionOf ( <SubsetWithCommonCharacteristics> <Track> ) ] ;
    rdfs:isDefinedBy <> ;
    rdfs:range ns2:Concept ;
    ns1:term_status "stable" ;
    ns2:definition "Additional concept class according to OpenStreetMap."@en .

<otherCantDeficiencyBasicSSP> a owl:ObjectProperty ;
    rdfs:label "Other Cant Deficiency train categories for which the ETCS trackside is configured to provide SSP"@en ;
    <rinfIndex> "1.1.1.3.2.14.1",
        "1.2.1.1.1.14.1" ;
    dcterms:created "2023-03-14"^^xsd:date ;
    rdfs:comment """Essential information for drivers of trains with a worse (lower) tolerated cant deficiency than those for which the ETCS trackside provides SSP (Static Speed Profiles) in conjunction with parameter "Cant Deficiency used for the basic SSP". 
According to the specification referenced in Appendix A-1, index [C]."""@en ;
    rdfs:domain [ a owl:Class ;
            owl:unionOf ( <SubsetWithCommonCharacteristics> <Track> ) ] ;
    rdfs:isDefinedBy <> ;
    rdfs:range ns2:Concept ;
    ns1:term_status "unstable" .

<otherPantographHead> a owl:ObjectProperty ;
    rdfs:label "Accepted other pantograph heads"@en ;
    <XMLName> "EPA_OtherHeads" ;
    <inSkosConceptScheme> <concepts/other-pantograph-heads/OtherPantographHeads> ;
    <rinfIndex> "1.1.1.2.3.2" ;
    <usedInRCCCalculations> true ;
    dcterms:created "2022-06-03"^^xsd:date ;
    dcterms:modified "2022-06-03"^^xsd:date ;
    rdfs:comment "Indication of pantograph heads which are allowed to be used."@en ;
    rdfs:domain [ a owl:Class ;
            owl:unionOf ( <SubsetWithCommonCharacteristics> <Track> ) ] ;
    rdfs:isDefinedBy <> ;
    rdfs:range ns2:Concept ;
    ns1:term_status "stable" .

<otherTrainProtection> a owl:FunctionalProperty,
        owl:ObjectProperty ;
    rdfs:label "Other train protection, control and warning systems for degraded situation"@en ;
    <XMLName> "CLD_OtherProtectControlWarn" ;
    <inSkosConceptScheme> <concepts/other-protection-control-warning/OtherProtectionControlWarnings> ;
    <rinfIndex> "1.1.1.3.10.2",
        "1.2.1.1.9.2" ;
    dcterms:created "2021-08-09"^^xsd:date ;
    dcterms:modified "2021-09-12"^^xsd:date ;
    rdfs:comment "Indication of existence of other system than ETCS for degraded situation."@en ;
    rdfs:domain [ a owl:Class ;
            owl:unionOf ( <SubsetWithCommonCharacteristics> <Track> ) ] ;
    rdfs:isDefinedBy <> ;
    rdfs:range ns2:Concept ;
    ns1:term_status "stable" .

<passesThroughTunnel> a owl:ObjectProperty ;
    rdfs:label "Passes through tunnel"@en ;
    dcterms:created "2020-07-29"^^xsd:date ;
    dcterms:modified "2022-10-27"^^xsd:date ;
    rdfs:comment "References a tunnel that a track goes through."@en ;
    rdfs:domain [ a owl:Class ;
            owl:unionOf ( <SubsetWithCommonCharacteristics> <Track> ) ] ;
    rdfs:isDefinedBy <> ;
    rdfs:range <Tunnel> ;
    ns1:term_status "stable" .

<permissionChargingElectricEnergyTractionStandstill> a owl:DatatypeProperty ;
    rdfs:label "Permission for charging electric energy storage for traction purposes at standstill"@en ;
    <rinfIndex> "1.2.1.0.7.1" ;
    dcterms:created "2023-03-14"^^xsd:date ;
    rdfs:comment "Point at which IM authorises charging of electric energy storage for traction purposes at standstill."@en ;
    rdfs:domain <ContactLineSystem> ;
    rdfs:isDefinedBy <> ;
    rdfs:range xsd:boolean ;
    rdfs:subPropertyOf owl:topDataProperty ;
    ns1:term_status "stable" .

<permitUseReflectivePlates> a owl:DatatypeProperty ;
    rdfs:label "Permit of use of reflective plates"@en ;
    <rinfIndex> "1.1.1.1.7.12" ;
    dcterms:created "2023-03-14"^^xsd:date ;
    rdfs:comment "Sections where is permitted to use the reflective plates on rail freight corridors, with a view to prioritise the current bottlenecks. Specific case for Belgium, France, Italy, Portugal and Spain until 1.1.2026."@en ;
    rdfs:domain [ a owl:Class ;
            owl:unionOf ( <SubsetWithCommonCharacteristics> <Track> ) ] ;
    rdfs:isDefinedBy <> ;
    rdfs:range xsd:boolean ;
    ns1:term_status "stable" .

<permittedContactForce> a owl:DatatypeProperty,
        owl:FunctionalProperty ;
    rdfs:label "Contact force permitted"@en ;
    <XMLName> "ERS_ContactForce" ;
    <rinfIndex> "1.1.1.2.5.2" ;
    <unitOfMeasure> <http://qudt.org/vocab/unit/N> ;
    <usedInRCCCalculations> true ;
    dcterms:created "2020-08-25"^^xsd:date ;
    dcterms:modified "2024-01-08"^^xsd:date ;
    rdfs:comment "Indication of contact force allowed expressed in newton."@en ;
    rdfs:domain [ a owl:Class ;
            owl:unionOf ( <SubsetWithCommonCharacteristics> <Track> ) ] ;
    rdfs:isDefinedBy <> ;
    rdfs:range xsd:string ;
    ns1:term_status "stable" .

<phaseInfo> a owl:DatatypeProperty,
        owl:FunctionalProperty ;
    rdfs:label "Information on phase separation"@en ;
    <XMLName> "EOS_InfoPhase" ;
    <rinfIndex> "1.1.1.2.4.1.2" ;
    dcterms:created "2021-08-08"^^xsd:date ;
    dcterms:isReplacedBy <phaseInfoLength>,
        <phaseInfoPantographLowered>,
        <phaseInfoSwitchOffBreaker>,
        "http://data.europa.eu/949/PhaseInfo",
        "http://data.europa.eu/949/phaseInfoKm",
        "http://data.europa.eu/949/trackPhaseInfo" ;
    dcterms:modified "2023-04-05"^^xsd:date ;
    rdfs:comment """Indication of required several information on phase separation. 
Deprecated because of replacement by three properties. The reason is that the property is composed of three values: length [NNN]’ – the length of the phase separation in metres; switch off breaker [Y/N], single selection of ‘Y=yes’ or ‘N=no’ to show whether the breaker has to be switched off; and lower pantograph [Y/N]’, single selection of ‘Y=yes’ or ‘N=no’ to show whether the pantograph has to be lowered,  Km [NNN.NNN] - the location from the start of the line where the new value is valid."""@en ;
    rdfs:domain [ a owl:Class ;
            owl:unionOf ( <SubsetWithCommonCharacteristics> <Track> ) ] ;
    rdfs:isDefinedBy <> ;
    rdfs:range xsd:string ;
    owl:deprecated true ;
    ns1:term_status "stable" .

<phaseSeparation> a owl:DatatypeProperty,
        owl:FunctionalProperty ;
    rdfs:label "Phase separation"@en ;
    <XMLName> "EOS_Phase" ;
    <rinfIndex> "1.1.1.2.4.1.1" ;
    dcterms:created "2021-08-08"^^xsd:date ;
    dcterms:modified "2021-09-12"^^xsd:date ;
    rdfs:comment "Indication of existence of phase separation and required information."@en ;
    rdfs:domain [ a owl:Class ;
            owl:unionOf ( <SubsetWithCommonCharacteristics> <Track> ) ] ;
    rdfs:isDefinedBy <> ;
    rdfs:range xsd:boolean ;
    ns1:term_status "stable" .

<platformEdge> a owl:ObjectProperty ;
    rdfs:label "Platform edge"@en ;
    dcterms:created "2021-08-09"^^xsd:date ;
    dcterms:modified "2023-11-10"^^xsd:date ;
    rdfs:comment "Reference to a related platform edge."@en ;
    rdfs:domain [ a owl:Class ;
            owl:unionOf ( <SubsetWithCommonCharacteristics> <Track> ) ] ;
    rdfs:isDefinedBy <> ;
    rdfs:range <PlatformEdge> ;
    ns1:term_status "stable" .

<platformHeight> a owl:FunctionalProperty,
        owl:ObjectProperty ;
    rdfs:label "Height of platform"@en ;
    <XMLName> "IPL_Height" ;
    <appendixD2Index> "2.3.7" ;
    <inSkosConceptScheme> <concepts/platform-heights/PlatformHeights> ;
    <rinfIndex> "1.2.1.0.6.5" ;
    <usedInRCCCalculations> true ;
    dcterms:created "2021-08-02"^^xsd:date ;
    dcterms:modified "2021-08-02"^^xsd:date ;
    dcterms:source <https://eur-lex.europa.eu/eli/reg_impl/2019/773/oj> ;
    rdfs:comment "Distance between the upper surface of platform and running surface of the neighbouring track. It is the nominal value expressed in millimetres."@en ;
    rdfs:domain <PlatformEdge> ;
    rdfs:isDefinedBy <> ;
    rdfs:range ns2:Concept ;
    ns1:term_status "stable" .

<platformId> a owl:DatatypeProperty,
        owl:FunctionalProperty ;
    rdfs:label "Identification of platform"@en ;
    <XMLName> "OPTrackPlatformIdentification" ;
    <appendixD2Index> "2.3.5" ;
    <rinfIndex> "1.2.1.0.6.2" ;
    dcterms:created "2021-09-13"^^xsd:date ;
    dcterms:modified "2023-03-14"^^xsd:date ;
    dcterms:source <https://eur-lex.europa.eu/eli/reg_impl/2019/773/oj> ;
    rdfs:comment "Unique platform identification or platform number within an Operational Point."@en ;
    rdfs:domain <PlatformEdge> ;
    rdfs:isDefinedBy <> ;
    rdfs:range xsd:string ;
    ns1:term_status "stable" .

<profileNumberSemiTrailers> a owl:ObjectProperty ;
    rdfs:label "Standard combined transport profile number for semi-trailers"@en ;
    <XMLName> "ILL_ProfileNumSemiTrailers" ;
    <inSkosConceptScheme> <concepts/profile-num-semi-trailers/ProfileNumbersSemiTrailers> ;
    <rinfIndex> "1.1.1.1.3.5" ;
    dcterms:created "2021-08-03"^^xsd:date ;
    dcterms:modified "2023-03-14"^^xsd:date ;
    rdfs:comment "Coding for combined transport for semi-trailers (for all freight and mixed-traffic lines) in accordance with the specification referenced in Appendix A-1, index [B]."@en ;
    rdfs:domain [ a owl:Class ;
            owl:unionOf ( <SubsetWithCommonCharacteristics> <Track> ) ] ;
    rdfs:isDefinedBy <> ;
    rdfs:range ns2:Concept ;
    ns1:term_status "stable" .

<profileNumberSwapBodies> a owl:ObjectProperty ;
    rdfs:label "Standard combined transport profile number for swap bodies"@en ;
    <XMLName> "ILL_ProfileNumSwapBodies" ;
    <inSkosConceptScheme> <concepts/profile-num-swap-bodies/ProfileNumbersSwapBodies> ;
    <rinfIndex> "1.1.1.1.3.4" ;
    dcterms:created "2021-08-03"^^xsd:date ;
    dcterms:modified "2023-03-14"^^xsd:date ;
    rdfs:comment "Coding for combined transport with swap bodies (for all freight and mixed-traffic lines) in accordance with the specification referenced in Appendix A-1, index [B]"@en ;
    rdfs:domain [ a owl:Class ;
            owl:unionOf ( <SubsetWithCommonCharacteristics> <Track> ) ] ;
    rdfs:isDefinedBy <> ;
    rdfs:range ns2:Concept ;
    ns1:term_status "stable" .

<protectionLegacySystem> a owl:ObjectProperty ;
    rdfs:label "Train protection legacy system"@en ;
    <XMLName> "CPO_LegacyTrainProtection" ;
    <eratvIndex> "4.13.1.5" ;
    <inSkosConceptScheme> <concepts/train-protection-legacy-systems/TrainProtectionLegacySystems> ;
    <rinfIndex> "1.1.1.3.5.3",
        "1.2.1.1.4.1" ;
    <usedInRCCCalculations> true ;
    dcterms:created "2020-08-31"^^xsd:date ;
    dcterms:modified "2021-09-12"^^xsd:date ;
    rdfs:comment "Indication of which class B system is installed."@en ;
    rdfs:domain [ a owl:Class ;
            owl:unionOf ( <SubsetWithCommonCharacteristics> <Track> <VehicleType> ) ] ;
    rdfs:isDefinedBy <> ;
    rdfs:range ns2:Concept ;
    ns1:term_status "stable" .

<publicNetworkRoaming> a owl:DatatypeProperty,
        owl:FunctionalProperty ;
    rdfs:label "Existence of GSM-R roaming to public networks"@en ;
    <XMLName> "CRG_RoamingPublic" ;
    <rinfIndex> "1.1.1.3.3.6",
        "1.2.1.1.2.6" ;
    dcterms:created "2021-08-09"^^xsd:date ;
    dcterms:modified "2024-01-08"^^xsd:date ;
    rdfs:comment """Existence of roaming to a public network.
In case of Y, provide the name of the public network under parameter "Details on GSM-R roaming to public networks"."""@en ;
    rdfs:domain [ a owl:Class ;
            owl:unionOf ( <SubsetWithCommonCharacteristics> <Track> ) ] ;
    rdfs:isDefinedBy <> ;
    rdfs:range xsd:boolean ;
    ns1:term_status "stable" .

<publicNetworkRoamingDetails> a owl:DatatypeProperty,
        owl:FunctionalProperty ;
    rdfs:label "Details on GSM-R roaming to public networks"@en ;
    <XMLName> "CRG_RoamingPublicDetails" ;
    <rinfIndex> "1.1.1.3.3.7",
        "1.2.1.1.2.7" ;
    dcterms:created "2021-08-09"^^xsd:date ;
    dcterms:modified "2024-01-08"^^xsd:date ;
    rdfs:comment """If roaming to public networks is configured, please indicate to which networks, 
for which users and in which areas."""@en ;
    rdfs:domain [ a owl:Class ;
            owl:unionOf ( <SubsetWithCommonCharacteristics> <Track> ) ] ;
    rdfs:isDefinedBy <> ;
    rdfs:range xsd:string ;
    ns1:term_status "stable" .

<qNvdriverAdhes> a owl:ObjectProperty ;
    rdfs:label "Q_NVDRIVER_ADHES"@en ;
    <appendixD3Index> "1.5.11" ;
    <rinfIndex> "1.1.1.3.2.16.11",
        "1.2.1.1.1.16.11 " ;
    dcterms:created "2023-03-14"^^xsd:date ;
    rdfs:comment """Qualifier determining whether the driver is allowed to modify the adhesion factor used by the ETCS on-board to calculate the braking curves. 
According to the specification referenced in Appendix A-1, index [C]. 
In https://www.era.europa.eu/sites/default/files/filesystem/ertms/ccs_tsi_annex_a_-_mandatory_specifications/set_of_specifications_3_etcs_b3_r2_gsm-r_b1/index004_-_subset-026_v360.zip
 Subset 26, chapter 7. 7.5.1.122 Q_NVDRIVER_ADHES."""@en ;
    rdfs:domain [ a owl:Class ;
            owl:unionOf ( <SubsetWithCommonCharacteristics> <Track> ) ] ;
    rdfs:isDefinedBy <> ;
    rdfs:range ns2:Concept ;
    ns1:term_status "stable" .

<qNvemrrls> a owl:ObjectProperty ;
    rdfs:label "Q_NVEMRRLS"@en ;
    <appendixD3Index> "1.5.2" ;
    <rinfIndex> "1.1.1.3.2.16.2",
        "1.2.1.1.1.16.2 " ;
    dcterms:created "2023-03-14"^^xsd:date ;
    rdfs:comment """Qualifier defining whether the application of the emergency brake for reasons other than a trip can be revoked as soon as the conditions for it have disappeared or after the train has come to a complete standstill.
According to the specification referenced in Appendix A-1, index [C]. 
In https://www.era.europa.eu/sites/default/files/filesystem/ertms/ccs_tsi_annex_a_-_mandatory_specifications/set_of_specifications_3_etcs_b3_r2_gsm-r_b1/index004_-_subset-026_v360.zip
Subset 26, chapter 7. 7.5.1.123 Q_NVEMRRLS."""@en ;
    rdfs:domain [ a owl:Class ;
            owl:unionOf ( <SubsetWithCommonCharacteristics> <Track> ) ] ;
    rdfs:isDefinedBy <> ;
    rdfs:range ns2:Concept ;
    ns1:term_status "unstable" .

<qNvsbtsmperm> a owl:DatatypeProperty ;
    rdfs:label "Q_NVSBTSMPERM"@en ;
    <rinfIndex> "1.1.1.3.2.16.12",
        "1.2.1.1.1.16.12" ;
    dcterms:created "2023-03-14"^^xsd:date ;
    rdfs:comment "Permission to use service brake in target speed monitoring."@en ;
    rdfs:domain [ a owl:Class ;
            owl:unionOf ( <SubsetWithCommonCharacteristics> <Track> ) ] ;
    rdfs:isDefinedBy <> ;
    rdfs:range xsd:boolean ;
    ns1:term_status "stable" .

<radioNetworkId> a owl:DatatypeProperty ;
    rdfs:label "Radio Network ID"@en ;
    <rinfIndex> "1.1.1.3.3.12",
        "1.2.1.1.2.13" ;
    dcterms:created "2023-03-14"^^xsd:date ;
    rdfs:comment "Unique identification of the GSM-R network the calling mobile station has to register with, as defined in the specification referenced in Appendix A-1, index [C]."@en ;
    rdfs:domain [ a owl:Class ;
            owl:unionOf ( <SubsetWithCommonCharacteristics> <Track> ) ] ;
    rdfs:isDefinedBy <> ;
    rdfs:range xsd:integer ;
    ns1:term_status "stable" .

<railInclination> a owl:FunctionalProperty,
        owl:ObjectProperty ;
    rdfs:label "Rail inclination"@en ;
    <XMLName> "ITP_RailInclination" ;
    <eratvIndex> "4.6.5" ;
    <inSkosConceptScheme> <concepts/rail-inclinations/RailInclinations> ;
    <rinfIndex> "1.1.1.1.4.3" ;
    <usedInRCCCalculations> true ;
    dcterms:created "2020-08-24"^^xsd:date ;
    dcterms:modified "2022-10-20"^^xsd:date ;
    rdfs:comment "An angle defining the inclination of the head of a rail relative to the running surface."@en ;
    rdfs:domain [ a owl:Class ;
            owl:unionOf ( <SubsetWithCommonCharacteristics> <Track> <VehicleType> ) ] ;
    rdfs:isDefinedBy <> ;
    rdfs:range ns2:Concept ;
    ns1:term_status "stable" .

<raisedPantographsDistanceAndSpeed> a owl:DatatypeProperty ;
    rdfs:label "Requirements for number of raised pantographs and spacing between them, at the given speed"@en ;
    <XMLName> "EPA_NumRaisedSpeed" ;
    <appendixD2Index> "3.3.4" ;
    <rinfIndex> "1.1.1.2.3.3" ;
    dcterms:created "2020-08-25"^^xsd:date ;
    dcterms:modified "2023-04-05"^^xsd:date ;
    dcterms:source <https://eur-lex.europa.eu/eli/reg_impl/2019/773/oj> ;
    rdfs:comment """Indication of maximum number of raised pantographs per train allowed and minimum spacing centre line to centre line of adjacent pantograph heads, expressed in metres, at the given speed.
Deprecated because of replacement by a class and three integer properties The reason is that the property is composed of three values: [N] is number of pantographs; [NNN] is minimum distance between pantographs, in metres; [NNN] is the speed considered in km/h."""@en ;
    rdfs:domain [ a owl:Class ;
            owl:unionOf ( <SubsetWithCommonCharacteristics> <Track> ) ] ;
    rdfs:isDefinedBy <> ;
    rdfs:range xsd:string ;
    owl:deprecated true ;
    ns1:term_status "stable" .

<reasonsEtcsRadioBlockCenterReject> a owl:ObjectProperty ;
    rdfs:label "Reasons for which an ETCS Radio Block Center can reject a train"@en ;
    <appendixD3Index> "1.4" ;
    <rinfIndex> "1.1.1.3.2.15",
        "1.2.1.1.1.15" ;
    dcterms:created "2022-11-07"^^xsd:date ;
    dcterms:modified "2023-03-14"^^xsd:date ;
    rdfs:comment """List of cases subject to system design choices made by the infrastructure manager according to the specification referenced in Appendix A-1, index [C]. 
In https://www.era.europa.eu/sites/default/files/filesystem/ertms/ccs_tsi_annex_a_-_mandatory_specifications/set_of_specifications_3_etcs_b3_r2_gsm-r_b1/index004_-_subset-026_v360.zip
Subset 26, Chapter 5 5.4 Procedure start of mission."""@en ;
    rdfs:domain [ a owl:Class ;
            owl:unionOf ( <SubsetWithCommonCharacteristics> <Track> ) ] ;
    rdfs:isDefinedBy <> ;
    rdfs:range ns2:Concept ;
    ns1:term_status "unstable" .

<redLightsRequired> a owl:DatatypeProperty,
        owl:FunctionalProperty ;
    rdfs:label "Steady red lights required"@en ;
    <XMLName> "IHS_RedLights" ;
    <rinfIndex> "1.1.1.1.7.10" ;
    dcterms:created "2021-08-08"^^xsd:date ;
    dcterms:modified "2024-01-08"^^xsd:date ;
    rdfs:comment "Sections where two steady red lights are required in accordance with TSI OPE."@en ;
    rdfs:domain [ a owl:Class ;
            owl:unionOf ( <SubsetWithCommonCharacteristics> <Track> ) ] ;
    rdfs:isDefinedBy <> ;
    rdfs:range xsd:boolean ;
    ns1:term_status "stable" .

<requiredSandingOverride> a owl:DatatypeProperty ;
    rdfs:label "Sanding override by driver required"@en ;
    <XMLName> "CTD_SandDriverOverride" ;
    <appendixD2Index> "3.2.6" ;
    <rinfIndex> "1.1.1.3.7.18" ;
    dcterms:created "2021-08-08"^^xsd:date ;
    dcterms:modified "2023-03-14"^^xsd:date ;
    dcterms:source <https://eur-lex.europa.eu/eli/reg_impl/2019/773/oj> ;
    rdfs:comment "Indication whether possibility to activate/deactivate sanding devices by driver, according to instructions from the Infrastructure Manager, is required or not. Deprecated according to the ammendment to the Regulation (EU) 2019/777."@en ;
    rdfs:domain <TrainDetectionSystem> ;
    rdfs:isDefinedBy <> ;
    rdfs:range xsd:boolean ;
    owl:deprecated true ;
    ns1:term_status "stable" .

<rollingStockFireCategory> a owl:FunctionalProperty,
        owl:ObjectProperty ;
    rdfs:label "Fire category of rolling stock required"@en ;
    <XMLName> "ITU_FireCatReq" ;
    <appendixD2Index> "3.2.3" ;
    <inSkosConceptScheme> <concepts/rolling-stock-fire/Categories> ;
    <rinfIndex> "1.1.1.1.8.10",
        "1.2.1.0.5.7",
        "1.2.2.0.5.7" ;
    <usedInRCCCalculations> true ;
    dcterms:created "2020-07-29"^^xsd:date ;
    dcterms:modified "2024-01-08"^^xsd:date ;
    dcterms:source <https://eur-lex.europa.eu/eli/reg_impl/2019/773/oj> ;
    rdfs:comment """Categorisation how a passenger train with a fire on board will continue to operate for a defined time period. 
Passenger train fire category in accordance with point 4.1.4 of TSI LOC&PAS."""@en ;
    rdfs:domain <Tunnel> ;
    rdfs:isDefinedBy <> ;
    rdfs:range ns2:Concept ;
    ns1:term_status "stable" .

<safeConsistLengthInformationNecessary> a owl:ObjectProperty ;
    rdfs:label "Safe consist length information from on-board necessary for access the line and SIL"@en ;
    <rinfIndex> "1.1.1.3.2.11",
        "1.2.1.1.1.11" ;
    dcterms:created "2023-03-14"^^xsd:date ;
    rdfs:comment """Indication whether safe consist train length information from on-board is required to access the line for safety reasons and the required safety integrity level.
"""@en ;
    rdfs:domain [ a owl:Class ;
            owl:unionOf ( <SubsetWithCommonCharacteristics> <Track> ) ] ;
    rdfs:isDefinedBy <> ;
    rdfs:range ns2:Concept ;
    ns1:term_status "stable" .

<schematicOverviewOP> a owl:DatatypeProperty ;
    rdfs:label "Schematic overview of the operational point"@en ;
    <rinfIndex> "1.2.0.0.0.7.1" ;
    dcterms:created "2023-03-14"^^xsd:date ;
    rdfs:comment "Document providing the schematic overview of the  operational point."@en ;
    rdfs:domain <OperationalPoint> ;
    rdfs:isDefinedBy <> ;
    rdfs:range xsd:anyURI ;
    ns1:term_status "stable" .

<siding> a owl:ObjectProperty ;
    rdfs:label "Siding"@en ;
    dcterms:created "2021-08-10"^^xsd:date ;
    dcterms:modified "2021-08-10"^^xsd:date ;
    rdfs:comment "Reference to a related siding."@en ;
    rdfs:domain <OperationalPoint> ;
    rdfs:isDefinedBy <> ;
    rdfs:range <Siding> ;
    ns1:term_status "stable" .

<sidingId> a owl:DatatypeProperty,
        owl:FunctionalProperty ;
    rdfs:label "Identification of siding"@en ;
    <XMLName> "OPSidingIdentification" ;
    <appendixD2Index> "2.2.1",
        "2.2.1.4" ;
    <rinfIndex> "1.2.2.0.0.2" ;
    dcterms:created "2021-09-13"^^xsd:date ;
    dcterms:modified "2023-03-14"^^xsd:date ;
    dcterms:source <https://eur-lex.europa.eu/eli/reg_impl/2019/773/oj> ;
    rdfs:comment "Unique siding identification or number within an Operational Point."@en ;
    rdfs:domain <Siding> ;
    rdfs:isDefinedBy <> ;
    rdfs:range xsd:string ;
    rdfs:subPropertyOf dcterms:identifier ;
    ns1:term_status "stable" .

<solNature> a owl:FunctionalProperty,
        owl:ObjectProperty ;
    rdfs:label "Nature of Section of Line"@en ;
    <XMLName> "SOLNature" ;
    <inSkosConceptScheme> <concepts/sol-natures/SoLNatures> ;
    <rinfIndex> "1.1.0.0.0.6" ;
    dcterms:created "2021-08-08"^^xsd:date ;
    dcterms:modified "2023-03-14"^^xsd:date ;
    rdfs:comment "Kind of section of line expressing size of presented data which depends on fact whether it connects OPs generated by division of a big node into several OPs or not."@en ;
    rdfs:domain <SectionOfLine> ;
    rdfs:isDefinedBy <> ;
    rdfs:range ns2:Concept ;
    ns1:term_status "stable" .

<specialTunnelArea> a owl:ObjectProperty ;
    rdfs:label "Special tunnel area"@en ;
    <appendixD2Index> "3.2.3" ;
    dcterms:created "2022-10-27"^^xsd:date ;
    dcterms:source <https://eur-lex.europa.eu/eli/reg_impl/2019/773/oj> ;
    rdfs:comment "Relates a tunnel with a special area or location."@en ;
    rdfs:domain <Tunnel> ;
    rdfs:isDefinedBy <> ;
    rdfs:range <SpecialTunnelArea> ;
    ns1:term_status "stable" .

<specificInformation> a owl:DatatypeProperty,
        owl:FunctionalProperty ;
    rdfs:label "Specific information"@en ;
    <XMLName> "ILL_SpecificInfo" ;
    <rinfIndex> "1.1.1.1.3.5.1" ;
    dcterms:created "2021-08-03"^^xsd:date ;
    dcterms:modified "2021-09-10"^^xsd:date ;
    rdfs:comment "Any relevant information from the IM relating to the line layout."@en ;
    rdfs:domain [ a owl:Class ;
            owl:unionOf ( <SubsetWithCommonCharacteristics> <Track> ) ] ;
    rdfs:isDefinedBy <> ;
    rdfs:range xsd:string ;
    ns1:term_status "stable" .

<standardCombinedTransporRollerUnits> a owl:ObjectProperty ;
    rdfs:label "Standard combined transport profile number for roller units"@en ;
    <rinfIndex> "1.1.1.1.3.9" ;
    dcterms:created "2023-03-14"^^xsd:date ;
    rdfs:comment """Coding for combined transport for roller units (for all freight and mixed-traffic lines) in accordance with the specification referenced in Appendix A-1, index [B]. 
"""@en ;
    rdfs:domain [ a owl:Class ;
            owl:unionOf ( <SubsetWithCommonCharacteristics> <Track> ) ] ;
    rdfs:isDefinedBy <> ;
    rdfs:range ns2:Concept ;
    ns1:term_status "unstable" .

<standardCombinedTransportContainers> a owl:ObjectProperty ;
    rdfs:label "Standard combined transport profile number for containers"@en ;
    <rinfIndex> "1.1.1.1.3.8" ;
    dcterms:created "2023-03-14"^^xsd:date ;
    rdfs:comment """Coding for combined transport for containers (for all freight and mixed-traffic lines) in accordance with the specification referenced in Appendix A-1, index [B].
"""@en ;
    rdfs:domain [ a owl:Class ;
            owl:unionOf ( <SubsetWithCommonCharacteristics> <Track> ) ] ;
    rdfs:isDefinedBy <> ;
    rdfs:range ns2:Concept ;
    ns1:term_status "unstable" .

<startLocation> a owl:ObjectProperty ;
    rdfs:label "Start of tunnel location"@en ;
    <XMLName> "SOLTunnelStart" ;
    <rinfIndex> "1.1.1.1.8.3" ;
    dcterms:created "2020-07-29"^^xsd:date ;
    dcterms:modified "2024-02-05"^^xsd:date ;
    rdfs:comment """Part of the Start of tunnel that indicates the Geographical coordinates according to the standard World Geodetic System (WGS). Precision for both geographical latitude and geographical longitude is assumed as [NN.NNNNNNN] in degrees with decimals what gives discretion of 10 cm in the network.
The Start of tunnel is the Geographical coordinates in decimal degrees and km of the line at the beginning of a tunnel."""@en ;
    rdfs:domain <Tunnel> ;
    rdfs:isDefinedBy <> ;
    rdfs:range [ a owl:Class ;
            owl:unionOf ( <http://www.opengis.net/ont/geosparql#Geometry> <http://www.w3.org/2003/01/geo/wgs84_pos#Point> ) ] ;
    rdfs:subPropertyOf <http://www.opengis.net/ont/geosparql#hasGeometry>,
        <http://www.w3.org/2003/01/geo/wgs84_pos#location> ;
    ns1:term_status "stable" .

<structureCheckLocation> a owl:DatatypeProperty ;
    rdfs:label "Railway location of structures requiring specific checks"@en ;
    <XMLName> "IPP_StructureCheckLoc" ;
    <rinfIndex> "1.1.1.1.2.4.3" ;
    <usedInRCCCalculations> true ;
    dcterms:created "2020-08-24"^^xsd:date ;
    dcterms:modified "2023-03-14"^^xsd:date ;
    rdfs:comment "Localisation of structures requiring specific checks."@en ;
    rdfs:domain [ a owl:Class ;
            owl:unionOf ( <SubsetWithCommonCharacteristics> <Track> ) ] ;
    rdfs:isDefinedBy <> ;
    rdfs:range xsd:double ;
    ns1:term_status "stable" .

<switchProtectControlWarning> a owl:DatatypeProperty,
        owl:FunctionalProperty ;
    rdfs:label "Existence of switch over between different protection, control and warning systems while running"@en ;
    <XMLName> "CTS_SwitchProtectControlWarn" ;
    <rinfIndex> "1.1.1.3.8.1",
        "1.2.1.1.7.1" ;
    dcterms:created "2021-08-09"^^xsd:date ;
    dcterms:modified "2021-09-12"^^xsd:date ;
    rdfs:comment "Indication whether a switch over between different systems whilst running exist."@en ;
    rdfs:domain [ a owl:Class ;
            owl:unionOf ( <SubsetWithCommonCharacteristics> <Track> ) ] ;
    rdfs:isDefinedBy <> ;
    rdfs:range xsd:boolean ;
    ns1:term_status "stable" .

<switchRadioSystem> a owl:DatatypeProperty,
        owl:FunctionalProperty ;
    rdfs:label "Existence of switch over between different radio systems"@en ;
    <XMLName> "CTS_SwitchRadioSystem" ;
    <rinfIndex> "1.1.1.3.8.2",
        "1.2.1.1.7.2" ;
    dcterms:created "2021-08-09"^^xsd:date ;
    dcterms:modified "2021-09-12"^^xsd:date ;
    rdfs:comment "Indication whether a switch over between different radio systems and no communication system whilst running exist."@en ;
    rdfs:domain [ a owl:Class ;
            owl:unionOf ( <SubsetWithCommonCharacteristics> <Track> ) ] ;
    rdfs:isDefinedBy <> ;
    rdfs:range xsd:boolean ;
    ns1:term_status "stable" .

<systemSeparationInfo> a owl:DatatypeProperty,
        owl:FunctionalProperty ;
    rdfs:label "Information on system separation"@en ;
    <XMLName> "EOS_InfoSystem" ;
    <rinfIndex> "1.1.1.2.4.2.2" ;
    dcterms:created "2021-08-08"^^xsd:date ;
    dcterms:isReplacedBy <SystemSeparationInfo>,
        <systemSeparationInfoKm>,
        <systemSeparationInfoLength>,
        <systemSeparationInfoSwitchOffBreaker>,
        <systemSeparationLoweredPantograph>,
        <trackSystemSeparationInfo> ;
    dcterms:modified "2023-04-05"^^xsd:date ;
    rdfs:comment """Indication of required several information on system separation.
Deprecated because of replacement by four properties. The reason is that the property is composed of four values: length [NNN], the length of the system separation in metres; switch off breaker [Y/N]. Single selection of ‘Y=yes’ or ‘N=no’ to show whether the breaker has to be switched off;  lower pantograph [Y/N]. Single selection of ‘Y=yes’ or ‘N=no’ to show whether the pantograph has to be lowered, and [CharacterString]  to show whether the supply system has to be changed."""@en ;
    rdfs:domain [ a owl:Class ;
            owl:unionOf ( <SubsetWithCommonCharacteristics> <Track> ) ] ;
    rdfs:isDefinedBy <> ;
    rdfs:range xsd:string ;
    owl:deprecated true ;
    ns1:term_status "stable" .

<tNvcontact> a owl:DatatypeProperty ;
    rdfs:label "T_NVCONTACT"@en ;
    <appendixD3Index> "1.5.8" ;
    <rinfIndex> "1.1.1.3.2.16.8",
        "1.2.1.1.1.16.8 " ;
    dcterms:created "2022-11-07"^^xsd:date ;
    dcterms:modified "2023-03-14"^^xsd:date ;
    rdfs:comment """Maximum time without a safe message from Radio Block Center before train reacts in seconds. 
According the specification referenced in Appendix A-1, index [C]. 
In https://www.era.europa.eu/sites/default/files/filesystem/ertms/ccs_tsi_annex_a_-_mandatory_specifications/set_of_specifications_3_etcs_b3_r2_gsm-r_b1/index004_-_subset-026_v360.zip
 Subset 26, chapter 7. 7.5.1.148 T_NVCONTACT."""@en ;
    rdfs:domain [ a owl:Class ;
            owl:unionOf ( <SubsetWithCommonCharacteristics> <Track> ) ] ;
    rdfs:isDefinedBy <> ;
    rdfs:range xsd:integer ;
    ns1:term_status "stable" .

<tNvovtrp> a owl:DatatypeProperty ;
    rdfs:label "T_NVOVTRP"@en ;
    <appendixD3Index> "1.5.6" ;
    <rinfIndex> "1.1.1.3.2.16.6",
        "1.2.1.1.1.16.6 " ;
    dcterms:created "2022-11-07"^^xsd:date ;
    dcterms:modified "2023-03-14"^^xsd:date ;
    rdfs:comment """MMaximum time for overriding the train trip in seconds. 
According to the specification referenced in Appendix A-1, index [C]. 
In https://www.era.europa.eu/sites/default/files/filesystem/ertms/ccs_tsi_annex_a_-_mandatory_specifications/set_of_specifications_3_etcs_b3_r2_gsm-r_b1/index004_-_subset-026_v360.zip
 Subset 26, chapter 7. 7.5.1.149 T_NVOVTRP."""@en ;
    rdfs:domain [ a owl:Class ;
            owl:unionOf ( <SubsetWithCommonCharacteristics> <Track> ) ] ;
    rdfs:isDefinedBy <> ;
    rdfs:range xsd:integer ;
    ns1:term_status "stable" .

<tafTAPCode> a owl:DatatypeProperty,
        owl:FunctionalProperty ;
    rdfs:label "OP primary location code"@en ;
    <XMLName> "OPTafTapCode" ;
    <appendixD2Index> "2.2.2" ;
    <rinfIndex> "1.2.0.0.0.3" ;
    dcterms:created "2020-07-29"^^xsd:date ;
    dcterms:modified "2024-01-08"^^xsd:date ;
    rdfs:comment "Primary location code developed for information exchange in accordance with the TSIs relating to the telematics applications subsystem."@en ;
    rdfs:domain <OperationalPoint> ;
    rdfs:isDefinedBy <> ;
    rdfs:range xsd:string ;
    rdfs:subPropertyOf dcterms:identifier ;
    ns1:term_status "stable" .

<tdsMaximumMagneticField> a owl:ObjectProperty ;
    rdfs:label "Maximum magnetic field"@en ;
    <rinfIndex> "1.1.1.3.4.2.3",
        "1.2.1.1.3.2.3" ;
    dcterms:created "2023-03-14"^^xsd:date ;
    rdfs:comment """Relates the TrainDetectionSystem with the MaximumMagneticField.
The maximum magnetic field limits allowed for axle counters (in dBµA/m) for a defined frequency band.
It should be provided in 3 directions."""@en ;
    rdfs:domain <TrainDetectionSystem> ;
    rdfs:isDefinedBy <> ;
    rdfs:range <MaximumMagneticField> ;
    ns1:term_status "stable" .

<tdsMinAxleLoadVehicleCategory> a owl:ObjectProperty ;
    rdfs:label "Train detection system min axle load vehicle category"@en ;
    <XMLName> "CTD_MinAxleLoadByVehicleCat" ;
    <rinfIndex> "1.1.1.3.7.11.1" ;
    dcterms:created "2023-01-25"^^xsd:date ;
    dcterms:modified "2023-03-14"^^xsd:date ;
    rdfs:comment "Indication of load given in tons depending of the category of vehicle. Deprecated according to the ammendment to the Regulation (EU) 2019/777."@en ;
    rdfs:domain <TrainDetectionSystem> ;
    rdfs:isDefinedBy <> ;
    rdfs:range <MinAxleLoadVehicleCategory> ;
    owl:deprecated true ;
    ns1:term_status "stable" .

<temperatureRange> a owl:ObjectProperty ;
    rdfs:label "Temperature range"@en ;
    <XMLName> "IPP_TempRange" ;
    <inSkosConceptScheme> <concepts/temperature-ranges/TemperatureRanges> ;
    <rinfIndex> "1.1.1.1.2.6" ;
    <usedInRCCCalculations> true ;
    dcterms:created "2023-01-20"^^xsd:date ;
    rdfs:comment "Temperature range for unrestricted access to the line according European standard."@en ;
    rdfs:domain [ a owl:Class ;
            owl:unionOf ( <SubsetWithCommonCharacteristics> <Track> ) ] ;
    rdfs:isDefinedBy <> ;
    rdfs:range ns2:Concept ;
    ns1:term_status "stable" .

<tenClassification> a owl:ObjectProperty ;
    rdfs:label "Trans-European Network (TEN) classification (of track, of platform, of siding)"@en ;
    <XMLName> "IPL_TENClass",
        "IPP_TENClass" ;
    <inSkosConceptScheme> <concepts/ten-classifications/TENClassifications> ;
    <rinfIndex> "1.1.1.1.2.1",
        "1.2.1.0.2.1",
        "1.2.1.0.6.3",
        "1.2.2.0.0.3" ;
    dcterms:created "2021-08-02"^^xsd:date ;
    dcterms:modified "2024-01-08"^^xsd:date ;
    rdfs:comment "Indicates the part of the trans-European network the (track, platform, siding) belongs to."@en ;
    rdfs:domain [ a owl:Class ;
            owl:unionOf ( <PlatformEdge> <Siding> <Track> ) ] ;
    rdfs:isDefinedBy <> ;
    rdfs:range ns2:Concept ;
    ns1:term_status "stable" .

<tenGISId> a owl:DatatypeProperty,
        owl:FunctionalProperty ;
    rdfs:label "TEN geographic information system identity (GIS ID)"@en ;
    <XMLName> "IPP_TENGISID" ;
    <rinfIndex> "1.1.1.1.2.1.2" ;
    dcterms:created "2021-08-03"^^xsd:date ;
    dcterms:modified "2024-01-08"^^xsd:date ;
    rdfs:comment "Indication of the GIS identity (GIS ID) of the section of TEN-T database to which the track belongs."@en ;
    rdfs:domain [ a owl:Class ;
            owl:unionOf ( <SubsetWithCommonCharacteristics> <Track> ) ] ;
    rdfs:isDefinedBy <> ;
    rdfs:range xsd:string ;
    ns1:term_status "stable" .

<tiltingSupported> a owl:DatatypeProperty ;
    rdfs:label "Indication whether tilting functions are supported by ETCS"@en ;
    <rinfIndex> "1.1.1.3.12.1" ;
    dcterms:created "2021-08-09"^^xsd:date ;
    dcterms:modified "2023-03-14"^^xsd:date ;
    rdfs:comment "Deprecated according to the ammendment to the Regulation (EU) 2019/777. Indication whether tilting functions are supported by ETCS."@en ;
    rdfs:domain [ a owl:Class ;
            owl:unionOf ( <SubsetWithCommonCharacteristics> <Track> ) ] ;
    rdfs:isDefinedBy <> ;
    rdfs:range xsd:boolean ;
    owl:deprecated true ;
    ns1:term_status "stable" .

<track> a owl:ObjectProperty ;
    rdfs:label "Track"@en ;
    dcterms:created "2021-08-09"^^xsd:date ;
    dcterms:modified "2021-09-09"^^xsd:date ;
    rdfs:comment "Reference to a related railway track."@en ;
    rdfs:domain [ a owl:Class ;
            owl:unionOf ( <OperationalPoint> <SectionOfLine> <Signal> ) ] ;
    rdfs:isDefinedBy <> ;
    rdfs:range <Track> ;
    ns1:term_status "stable" .

<trackDirection> a owl:FunctionalProperty,
        owl:ObjectProperty ;
    rdfs:label "Normal running direction"@en ;
    <XMLName> "SOLTrackDirection" ;
    <appendixD2Index> "2.2.1.1" ;
    <inSkosConceptScheme> <concepts/track-running-directions/TrackRunningDirections> ;
    <rinfIndex> "1.1.1.0.0.2" ;
    dcterms:created "2021-09-09"^^xsd:date ;
    dcterms:modified "2024-01-08"^^xsd:date ;
    rdfs:comment """The normal running direction is:
- the same as the direction defined by the start and end of the SoL: (N)
- the opposite to the direction defined by the start and end of the SoL: (O)
- both directions: (B)"""@en ;
    rdfs:domain <Track> ;
    rdfs:isDefinedBy <> ;
    rdfs:range ns2:Concept ;
    ns1:term_status "stable" .

<trackId> a owl:DatatypeProperty,
        owl:FunctionalProperty ;
    rdfs:label "Identification of track"@en ;
    <XMLName> "OPTrackIdentification",
        "SOLTrackIdentification" ;
    <appendixD2Index> "2.2.1.1" ;
    <rinfIndex> "1.1.1.0.0.1",
        "1.2.1.0.0.2" ;
    dcterms:created "2021-09-09"^^xsd:date ;
    dcterms:modified "2024-01-08"^^xsd:date ;
    dcterms:source <https://eur-lex.europa.eu/eli/reg_impl/2019/773/oj> ;
    rdfs:comment "Unique track identification or unique track number within an OP or a section of line."@en ;
    rdfs:domain <Track> ;
    rdfs:isDefinedBy <> ;
    rdfs:range xsd:string ;
    rdfs:subPropertyOf dcterms:identifier ;
    ns1:term_status "stable" .

<trackPhaseInfo> a owl:ObjectProperty ;
    rdfs:label "Track phase info"@en ;
    <XMLName> "EOS_InfoPhase" ;
    <rinfIndex> "1.1.1.2.4.1.2" ;
    dcterms:created "2023-04-05"^^xsd:date ;
    rdfs:comment "Relates the Track with PhaseInfo. Indication of required several information on phase separation."@en ;
    rdfs:domain [ a owl:Class ;
            owl:unionOf ( <SubsetWithCommonCharacteristics> <Track> ) ] ;
    rdfs:isDefinedBy <> ;
    rdfs:range <PhaseInfo> ;
    ns1:term_status "stable" .

<trackRaisedPantographsDistanceAndSpeed> a owl:ObjectProperty ;
    rdfs:label "Track raised pantograph distance and speed"@en ;
    <XMLName> "EPA_NumRaisedSpeed" ;
    <rinfIndex> "1.1.1.2.3.3" ;
    <usedInRCCCalculations> true ;
    dcterms:created "2023-04-05"^^xsd:date ;
    rdfs:comment "Relates the track with the class RaisePantporaphsDistanceAndSpeed. Indication of maximum number of raised pantographs per train allowed and minimum spacing centre line to centre line of adjacent pantograph heads, expressed in metres, at the given speed."@en ;
    rdfs:domain [ a owl:Class ;
            owl:unionOf ( <SubsetWithCommonCharacteristics> <Track> ) ] ;
    rdfs:isDefinedBy <> ;
    rdfs:range <RaisedPantographsDistanceAndSpeed> ;
    ns1:term_status "stable" .

<trainDetectionSystem> a owl:ObjectProperty ;
    rdfs:label "Train detection system"@en ;
    dcterms:created "2020-07-29"^^xsd:date ;
    dcterms:modified "2021-09-12"^^xsd:date ;
    rdfs:comment "Train detection systems installed in the section of line."@en ;
    rdfs:domain [ a owl:Class ;
            owl:unionOf ( <SubsetWithCommonCharacteristics> <Track> ) ] ;
    rdfs:isDefinedBy <> ;
    rdfs:range <TrainDetectionSystem> ;
    ns1:term_status "stable" .

<trainDetectionSystemSpecificCheck> a owl:ObjectProperty ;
    rdfs:label "Type of track circuits or axle counters to which specific checks are needed"@en ;
    <XMLName> "CTD_TCCheck" ;
    <inSkosConceptScheme> <concepts/train-detection-specific-checks/TrainDetectionSystemsSpecificChecks> ;
    <rinfIndex> "1.1.1.3.7.1.2",
        "1.2.1.1.6.1" ;
    <usedInRCCCalculations> true ;
    dcterms:created "2020-08-24"^^xsd:date ;
    dcterms:modified "2021-08-08"^^xsd:date ;
    rdfs:comment "Reference to the technical specification of train detection system, in accordance with the specification referenced in Appendix A-1, index [D]."@en ;
    rdfs:domain <TrainDetectionSystem> ;
    rdfs:isDefinedBy <> ;
    rdfs:range ns2:Concept ;
    ns1:term_status "stable" .

<trainDetectionSystemSpecificCheckDocument> a owl:ObjectProperty ;
    rdfs:label "Document with the procedure(s) related to the type of train detection systems declared in 1.1.1.3.7.1.2 or 1.2.1.1.6.1"@en ;
    <XMLName> "CTD_TCCheckDocRef" ;
    <rinfIndex> "1.1.1.3.7.1.3",
        "1.2.1.1.6.2" ;
    <usedInRCCCalculations> true ;
    dcterms:created "2021-08-03"^^xsd:date ;
    dcterms:modified "2024-04-23"^^xsd:date ;
    rdfs:comment "Electronic document from the IM stored by the Agency with precise values in accordance with TSI CCS Article13 and the specification referenced in Appendix A-1, index [D], for the specific check to be performed for train detection systems identified in parameter \"\"Type of track circuits or axle counters to which specific checks are needed\"."@en ;
    rdfs:domain <TrainDetectionSystem> ;
    rdfs:isDefinedBy <> ;
    rdfs:range <Document> ;
    ns1:term_status "stable" ;
    ns2:changeNote "Change from datatype property to object property in order to point to the class Document (reference document)"@en .

<trainIntegrityOnBoardRequired> a owl:DatatypeProperty,
        owl:FunctionalProperty ;
    rdfs:label "Train integrity confirmation from on-board (not from driver) necessary for line access"@en ;
    <XMLName> "CPE_IntegrityConfirmation" ;
    <rinfIndex> "1.1.1.3.2.8",
        "1.2.1.1.1.8" ;
    <usedInRCCCalculations> true ;
    dcterms:created "2020-08-31"^^xsd:date ;
    dcterms:modified "2021-09-12"^^xsd:date ;
    rdfs:comment "Indication whether train confirmation from on-board is required to access the line for safety reasons."@en ;
    rdfs:domain [ a owl:Class ;
            owl:unionOf ( <SubsetWithCommonCharacteristics> <Track> ) ] ;
    rdfs:isDefinedBy <> ;
    rdfs:range xsd:boolean ;
    ns1:term_status "stable" .

<tsiCompliantCompositeBrakeBlocks> a owl:ObjectProperty ;
    rdfs:label "TSI compliance of rules on the use of composite brake blocks"@en ;
    <XMLName> "CTD_TSICompositeBrakeBlocks" ;
    <inSkosConceptScheme> <concepts/tsi-compliances/TSICompliances> ;
    <rinfIndex> "1.1.1.3.7.21" ;
    dcterms:created "2021-08-08"^^xsd:date ;
    dcterms:modified "2023-03-14"^^xsd:date ;
    rdfs:comment "Deprecated according to the ammendment to the Regulation (EU) 2019/777. TSI compliance of rules on the use of composite brake blocks."@en ;
    rdfs:domain <TrainDetectionSystem> ;
    rdfs:isDefinedBy <> ;
    rdfs:range ns2:Concept ;
    owl:deprecated true ;
    ns1:term_status "stable" .

<tsiCompliantFerromagneticWheel> a owl:ObjectProperty ;
    rdfs:label "TSI compliance of Ferromagnetic characteristics of wheel material required"@en ;
    <XMLName> "CTD_TSIFerroWheelMat" ;
    <inSkosConceptScheme> <concepts/tsi-compliances/TSICompliances> ;
    <rinfIndex> "1.1.1.3.7.14" ;
    dcterms:created "2021-08-08"^^xsd:date ;
    dcterms:modified "2023-03-14"^^xsd:date ;
    rdfs:comment "TSI compliance of Ferromagnetic characteristics of wheel material required. Deprecated according to the ammendment to the Regulation (EU) 2019/777."@en ;
    rdfs:domain <TrainDetectionSystem> ;
    rdfs:isDefinedBy <> ;
    rdfs:range ns2:Concept ;
    owl:deprecated true ;
    ns1:term_status "stable" .

<tsiCompliantMaxDistConsecutiveAxles> a owl:ObjectProperty ;
    rdfs:label "TSI compliance of maximum permitted distance between two consecutive axles"@en ;
    <XMLName> "CTD_TSIMaxDistConsecutiveAxles" ;
    <inSkosConceptScheme> <concepts/tsi-compliances/TSICompliances> ;
    <rinfIndex> "1.1.1.3.7.2.1" ;
    dcterms:created "2021-08-07"^^xsd:date ;
    dcterms:modified "2023-03-14"^^xsd:date ;
    rdfs:comment "Indication whether required distance between two consecutive axles is compliant with the TSI. Deprecated according to the ammendment to the Regulation (EU) 2019/777."@en ;
    rdfs:domain <TrainDetectionSystem> ;
    rdfs:isDefinedBy <> ;
    rdfs:range ns2:Concept ;
    owl:deprecated true ;
    ns1:term_status "stable" .

<tsiCompliantMaxImpedanceWheelset> a owl:ObjectProperty ;
    rdfs:label "TSI compliance of maximum permitted impedance between opposite wheels of a wheelset"@en ;
    <XMLName> "CTD_TSIMaxImpedanceWheelset" ;
    <inSkosConceptScheme> <concepts/tsi-compliances/TSICompliances> ;
    <rinfIndex> "1.1.1.3.7.15.1" ;
    dcterms:created "2021-08-08"^^xsd:date ;
    dcterms:modified "2023-03-14"^^xsd:date ;
    rdfs:comment "TSI compliance of maximum permitted impedance between opposite wheels of a wheelset. Deprecated according to the ammendment to the Regulation (EU) 2019/777."@en ;
    rdfs:domain <TrainDetectionSystem> ;
    rdfs:isDefinedBy <> ;
    rdfs:range ns2:Concept ;
    owl:deprecated true ;
    ns1:term_status "stable" .

<tsiCompliantMetalConstruction> a owl:ObjectProperty ;
    rdfs:label "TSI compliance of rules for vehicle metal construction"@en ;
    <XMLName> "CTD_TSIMetalConstruction" ;
    <inSkosConceptScheme> <concepts/tsi-compliances/TSICompliances> ;
    <rinfIndex> "1.1.1.3.7.13" ;
    dcterms:created "2021-08-08"^^xsd:date ;
    dcterms:modified "2023-03-14"^^xsd:date ;
    rdfs:comment "TSI compliance of rules for vehicle metal construction. Deprecated according to the ammendment to the Regulation (EU) 2019/777."@en ;
    rdfs:domain <TrainDetectionSystem> ;
    rdfs:isDefinedBy <> ;
    rdfs:range ns2:Concept ;
    owl:deprecated true ;
    ns1:term_status "stable" .

<tsiCompliantMetalFreeSpace> a owl:ObjectProperty ;
    rdfs:label "TSI compliance of rules for metal-free space around wheels"@en ;
    <XMLName> "CTD_TSIMetalFree" ;
    <inSkosConceptScheme> <concepts/tsi-compliances/TSICompliances> ;
    <rinfIndex> "1.1.1.3.7.12" ;
    dcterms:created "2021-08-08"^^xsd:date ;
    dcterms:modified "2023-03-14"^^xsd:date ;
    rdfs:comment "TSI compliance of rules for metal-free space around wheels. Deprecated according to the ammendment to the Regulation (EU) 2019/777."@en ;
    rdfs:domain <TrainDetectionSystem> ;
    rdfs:isDefinedBy <> ;
    rdfs:range ns2:Concept ;
    owl:deprecated true ;
    ns1:term_status "stable" .

<tsiCompliantRSTShuntImpedance> a owl:ObjectProperty ;
    rdfs:label "TSI compliance of rules on combination of RST characteristics influencing shunting impedance"@en ;
    <XMLName> "CTD_TSIRSTShuntImpedance" ;
    <inSkosConceptScheme> <concepts/tsi-compliances/TSICompliances> ;
    <rinfIndex> "1.1.1.3.7.23" ;
    dcterms:created "2021-08-08"^^xsd:date ;
    dcterms:modified "2023-03-14"^^xsd:date ;
    rdfs:comment "TSI compliance of rules on combination of RST characteristics influencing shunting impedance. Deprecated according to the ammendment to the Regulation (EU) 2019/777."@en ;
    rdfs:domain <TrainDetectionSystem> ;
    rdfs:isDefinedBy <> ;
    rdfs:range ns2:Concept ;
    owl:deprecated true ;
    ns1:term_status "stable" .

<tsiCompliantSandCharacteristics> a owl:ObjectProperty ;
    rdfs:label "TSI Compliance of rules on sand characteristics"@en ;
    <XMLName> "CTD_TSISandCharacteristics" ;
    <inSkosConceptScheme> <concepts/tsi-compliances/TSICompliances> ;
    <rinfIndex> "1.1.1.3.7.19" ;
    dcterms:created "2021-08-08"^^xsd:date ;
    dcterms:modified "2023-03-14"^^xsd:date ;
    rdfs:comment "TSI Compliance of rules on sand characteristics. Deprecated according to the ammendment to the Regulation (EU) 2019/777." ;
    rdfs:domain <TrainDetectionSystem> ;
    rdfs:isDefinedBy <> ;
    rdfs:range ns2:Concept ;
    owl:deprecated true ;
    ns1:term_status "stable" .

<tsiCompliantSanding> a owl:ObjectProperty ;
    rdfs:label "TSI compliance of sanding"@en ;
    <inSkosConceptScheme> <concepts/tsi-compliances/TSICompliances> ;
    <rinfIndex> "1.1.1.3.7.16" ;
    dcterms:created "2021-08-08"^^xsd:date ;
    dcterms:modified "2023-03-14"^^xsd:date ;
    rdfs:comment "TSI compliance of sanding rules to allow compatibility with track circuits. Too much sand brings the risk of not detecting trains in tracks equipped with track circuits. Deprecated according to the ammendment to the Regulation (EU) 2019/777."@en ;
    rdfs:domain <TrainDetectionSystem> ;
    rdfs:isDefinedBy <> ;
    rdfs:range ns2:Concept ;
    owl:deprecated true ;
    ns1:term_status "unstable" .

<tsiCompliantShuntDevices> a owl:ObjectProperty ;
    rdfs:label "TSI compliance of rules on shunt assisting devices"@en ;
    <XMLName> "CTD_TSIShuntDevices" ;
    <inSkosConceptScheme> <concepts/tsi-compliances/TSICompliances> ;
    <rinfIndex> "1.1.1.3.7.22" ;
    dcterms:created "2021-08-08"^^xsd:date ;
    dcterms:modified "2023-03-14"^^xsd:date ;
    rdfs:comment "Deprecated according to the ammendment to the Regulation (EU) 2019/777. TSI compliance of rules on shunt assisting devices."@en ;
    rdfs:domain <TrainDetectionSystem> ;
    rdfs:isDefinedBy <> ;
    rdfs:range ns2:Concept ;
    owl:deprecated true ;
    ns1:term_status "stable" .

<tsiPantographHead> a owl:ObjectProperty ;
    rdfs:label "Accepted TSI compliant pantograph heads"@en ;
    <XMLName> "EPA_TSIHeads" ;
    <inSkosConceptScheme> <concepts/compliant-pantograph-heads/CompliantPantographHeads> ;
    <rinfIndex> "1.1.1.2.3.1" ;
    <usedInRCCCalculations> true ;
    dcterms:created "2020-08-25"^^xsd:date ;
    dcterms:modified "2021-09-11"^^xsd:date ;
    rdfs:comment "Indication of TSI compliant pantograph heads which are allowed to be used. The allowed values for this property belong to the SKOS Concept Scheme http://data.europa.eu/949/concepts/compliant-pantograph-heads/CompliantPantographHeads."@en ;
    rdfs:domain [ a owl:Class ;
            owl:unionOf ( <SubsetWithCommonCharacteristics> <Track> ) ] ;
    rdfs:isDefinedBy <> ;
    rdfs:range ns2:Concept ;
    ns1:term_status "stable" .

<tsiSwitchCrossing> a owl:DatatypeProperty,
        owl:FunctionalProperty ;
    rdfs:label "TSI compliance of in service values for switches and crossings"@en ;
    <XMLName> "ISC_TSISwitchCrossing" ;
    <rinfIndex> "1.1.1.1.5.1" ;
    dcterms:created "2021-08-03"^^xsd:date ;
    dcterms:modified "2021-09-10"^^xsd:date ;
    rdfs:comment "Switches and crossings are maintained to in service limit dimension as specified in TSI."@en ;
    rdfs:domain [ a owl:Class ;
            owl:unionOf ( <SubsetWithCommonCharacteristics> <Track> ) ] ;
    rdfs:isDefinedBy <> ;
    rdfs:range xsd:boolean ;
    ns1:term_status "stable" .

<tunnelDocRef> a owl:ObjectProperty ;
    rdfs:label "Document available from the IM with precise description of the tunnel"@en ;
    <XMLName> "ITU_TunnelDocRef" ;
    <rinfIndex> "1.1.1.1.8.8.2" ;
    dcterms:created "2021-08-03"^^xsd:date ;
    dcterms:modified "2024-04-23"^^xsd:date ;
    rdfs:comment "Electronic document available from the IM stored by the Agency with precise description of the clearance gauge and geometry of the tunnel."@en ;
    rdfs:domain <Tunnel> ;
    rdfs:isDefinedBy <> ;
    rdfs:range <Document> ;
    ns1:term_status "stable" ;
    ns2:changeNote "Change from datatype property to object property in order to point to the class Document (reference document)"@en .

<tunnelIdentification> a owl:DatatypeProperty,
        owl:FunctionalProperty ;
    rdfs:label "Tunnel identification"@en ;
    <XMLName> "OPSidingTunnelIdentification",
        "OPTrackTunnelIdentification",
        "SOLTunnelIdentification" ;
    <appendixD2Index> "3.2.3" ;
    <rinfIndex> "1.1.1.1.8.2",
        "1.2.1.0.5.2",
        "1.2.2.0.5.2" ;
    dcterms:created "2021-08-03"^^xsd:date ;
    dcterms:modified "2021-09-13"^^xsd:date ;
    dcterms:source <https://eur-lex.europa.eu/eli/reg_impl/2019/773/oj> ;
    rdfs:comment "Unique tunnel identification or unique number within Member State."@en ;
    rdfs:domain <Tunnel> ;
    rdfs:isDefinedBy <> ;
    rdfs:range xsd:string ;
    rdfs:subPropertyOf dcterms:identifier ;
    ns1:term_status "stable" .

<tunnelKilometerEnd> a owl:DatatypeProperty ;
    rdfs:label "End of tunnel kilometer"@en ;
    <XMLName> "SOLTunnelEnd" ;
    <rinfIndex> "1.1.1.1.8.4" ;
    dcterms:created "2023-03-29"^^xsd:date ;
    dcterms:isReplacedBy <lineReferenceTunnelEnd> ;
    dcterms:modified "2024-02-05" ;
    rdfs:comment """Part of the End of tunnel that indicates the km of the line at the end of a tunnel.
The End of tunnel is the Geographical coordinates in decimal degrees and km of the line at the end of a tunnel. The reason for deprecation is that the property is now a subproperty of lineReference in order to represent the kilometer in relation to a national railway line"""@en ;
    rdfs:domain <Tunnel> ;
    rdfs:isDefinedBy <> ;
    rdfs:range xsd:double ;
    owl:deprecated true ;
    ns1:term_status "stable" .

<tunnelKilometerStart> a owl:DatatypeProperty ;
    rdfs:label "Start of tunnel kilometer"@en ;
    <XMLName> "SOLTunnelEnd" ;
    <rinfIndex> "1.1.1.1.8.4" ;
    dcterms:created "2023-03-29"^^xsd:date ;
    dcterms:isReplacedBy <lineReferenceTunnelStart> ;
    dcterms:modified "2024-02-05" ;
    rdfs:comment """Part of the Start of tunnel that indicates the km of the line at the beginning of a tunnel.
The Start of tunnel is the Geographical coordinates in decimal degrees and km of the line at the beginning of a tunnel. The reason for deprecation is that the property is now a subproperty of lineReference in order to represent the kilometer in relation to a national railway line"""@en ;
    rdfs:domain <Tunnel> ;
    rdfs:isDefinedBy <> ;
    rdfs:range xsd:double ;
    owl:deprecated true ;
    ns1:term_status "stable" .

<umax2> a owl:DatatypeProperty ;
    rdfs:label "Umax2 for the French network"@en ;
    <XMLName> "ECS_Umax2" ;
    <rinfIndex> "1.1.1.2.2.1.3" ;
    <unitOfMeasure> <http://qudt.org/vocab/unit/V> ;
    <usedInRCCCalculations> true ;
    dcterms:created "2020-08-24"^^xsd:date ;
    dcterms:modified "2024-01-08"^^xsd:date ;
    rdfs:comment "Highest non-permanent voltage (Umax2) for France on lines not compliant with values defined in the the specification referenced in Appendix A-2, index [1]."@en ;
    rdfs:domain <ContactLineSystem> ;
    rdfs:isDefinedBy <> ;
    rdfs:range xsd:integer ;
    ns1:term_status "stable" .

<uopid> a owl:DatatypeProperty,
        owl:FunctionalProperty ;
    rdfs:label "Unique OP ID"@en ;
    <XMLName> "UniqueOPID" ;
    <appendixD2Index> "2.2.2" ;
    <rinfIndex> "1.2.0.0.0.2" ;
    dcterms:created "2020-07-29"^^xsd:date ;
    dcterms:modified "2024-01-08"^^xsd:date ;
    dcterms:source <https://eur-lex.europa.eu/eli/reg_impl/2019/773/oj> ;
    rdfs:comment "Code composed of country code and alphanumeric operational point code."@en ;
    rdfs:domain <OperationalPoint> ;
    rdfs:isDefinedBy <> ;
    rdfs:range xsd:string ;
    rdfs:subPropertyOf dcterms:identifier ;
    ns1:term_status "stable" .

<usesGroup555> a owl:DatatypeProperty,
        owl:FunctionalProperty ;
    rdfs:label "GSM-R use of group 555"@en ;
    <XMLName> "CRG_Needof555" ;
    <eratvIndex> "4.13.2.12" ;
    <rinfIndex> "1.1.1.3.3.4",
        "1.2.1.1.2.4" ;
    <usedInRCCCalculations> true ;
    dcterms:created "2020-08-31"^^xsd:date ;
    dcterms:modified "2021-09-12"^^xsd:date ;
    rdfs:comment "Indication if group 555 is used."@en ;
    rdfs:domain [ a owl:Class ;
            owl:unionOf ( <SubsetWithCommonCharacteristics> <Track> <VehicleType> ) ] ;
    rdfs:isDefinedBy <> ;
    rdfs:range xsd:boolean ;
    ns1:term_status "stable" .

<vNvallowovtrp> a owl:DatatypeProperty ;
    rdfs:label "V_NVALLOWOVTRP"@en ;
    <appendixD3Index> "1.5.3" ;
    <rinfIndex> "1.1.1.3.2.16.3",
        "1.2.1.1.1.16.3 " ;
    dcterms:created "2022-11-07"^^xsd:date ;
    dcterms:modified "2023-03-14"^^xsd:date ;
    rdfs:comment """Speed limit allowing the driver to select the “override” function in km/h.
According to the specification referenced in Appendix A-1, index [C]. 
In https://www.era.europa.eu/sites/default/files/filesystem/ertms/ccs_tsi_annex_a_-_mandatory_specifications/set_of_specifications_3_etcs_b3_r2_gsm-r_b1/index004_-_subset-026_v360.zip
 Chapter 7. 7.5.1.161"""@en ;
    rdfs:domain [ a owl:Class ;
            owl:unionOf ( <SubsetWithCommonCharacteristics> <Track> ) ] ;
    rdfs:isDefinedBy <> ;
    rdfs:range xsd:integer ;
    ns1:term_status "stable" .

<vNvsupovtrp> a owl:DatatypeProperty ;
    rdfs:label "V_NVSUPOVTRP"@en ;
    <appendixD3Index> "1.5.4" ;
    <rinfIndex> "1.1.1.3.2.16.4",
        "1.2.1.1.1.16.4 " ;
    dcterms:created "2022-11-07"^^xsd:date ;
    dcterms:modified "2023-03-14"^^xsd:date ;
    rdfs:comment """Override speed limit to be supervised when the “override” function is active  in km/h.
According to the specification referenced in Appendix A-1, index [C]. 
In https://www.era.europa.eu/sites/default/files/filesystem/ertms/ccs_tsi_annex_a_-_mandatory_specifications/set_of_specifications_3_etcs_b3_r2_gsm-r_b1/index004_-_subset-026_v360.zip
 Subset 26, chapter 7. 7.5.1.163 V_NVSUPOVTRP."""@en ;
    rdfs:domain [ a owl:Class ;
            owl:unionOf ( <SubsetWithCommonCharacteristics> <Track> ) ] ;
    rdfs:isDefinedBy <> ;
    rdfs:range xsd:integer ;
    ns1:term_status "stable" .

<validityEndDate> a owl:DatatypeProperty ;
    rdfs:label "Validity end date"@en ;
    dcterms:created "2022-10-19"^^xsd:date ;
    rdfs:comment "Defines the validity end date (e.g., an operational point that is not valid anymore), so that it is possible to filter out those that are not applicable for a specific application (e.g., for route planning)"@en ;
    rdfs:domain <InfrastructureObject> ;
    rdfs:isDefinedBy <> ;
    rdfs:range xsd:date ;
    ns1:term_status "stable" .

<validityStartDate> a owl:DatatypeProperty ;
    rdfs:label "Validity start date"@en ;
    dcterms:created "2022-10-20"^^xsd:date ;
    rdfs:comment "Defines the validity start date (e.g., an operational point that is not valid now since it is planned for the future), so that it is possible to filter out those that are not applicable for a specific application (e.g., for route planning)"@en ;
    rdfs:domain <InfrastructureObject> ;
    rdfs:isDefinedBy <> ;
    rdfs:range xsd:date ;
    ns1:term_status "stable" .

<vehicleTypesCompatibleTrafficLoad> a owl:DatatypeProperty ;
    rdfs:label "List of vehicle types already identified as compatible with Traffic load and load carrying capacity of infrastructure and train detection systems"@en ;
    <rinfIndex> "1.1.1.5.1" ;
    dcterms:created "2023-03-14"^^xsd:date ;
    rdfs:comment "The infrastructure managers shall provide through RINF the information to the RU regarding list of vehicle types compatible with the route for which they have already verified compatibility for parameter Traffic load and load carrying capacity of infrastructure and train detection systems, where such information is available."@en ;
    rdfs:domain [ a owl:Class ;
            owl:unionOf ( <SubsetWithCommonCharacteristics> <Track> ) ] ;
    rdfs:isDefinedBy <> ;
    rdfs:range xsd:anyURI ;
    ns1:term_status "unstable" .

<vehiclesCompatibleTrafficLoad> a owl:DatatypeProperty ;
    rdfs:label "List of vehicles already identified as compatible with Traffic load and load carrying capacity of infrastructure and train detection systems"@en ;
    <rinfIndex> "1.1.1.5.2" ;
    dcterms:created "2023-03-14"^^xsd:date ;
    rdfs:comment "The infrastructure managers shall provide through RINF the information or a document to the RU regarding list of vehicle(s) compatible with the route for which they have already verified compatibility for parameter Traffic load and load carrying capacity of infrastructure and train detection systems, where such information is available."@en ;
    rdfs:domain [ a owl:Class ;
            owl:unionOf ( <SubsetWithCommonCharacteristics> <Track> ) ] ;
    rdfs:isDefinedBy <> ;
    rdfs:range xsd:anyURI ;
    ns1:term_status "unstable" .

<verificationCCS> a owl:DatatypeProperty ;
    rdfs:label "EC declaration of verification for track relating to compliance with the requirements from TSIs applicable to control, command signalling subsystem"@en ;
    <XMLName> "CDE_ECVerification" ;
    <rinfIndex> "1.1.1.3.1.1" ;
    dcterms:created "2021-08-08"^^xsd:date ;
    dcterms:modified "2024-01-08"^^xsd:date ;
    rdfs:comment "Unique number for EC declarations in accordance with Commission Implementing Regulation (EU) 2019/250"@en ;
    rdfs:domain [ a owl:Class ;
            owl:unionOf ( <SubsetWithCommonCharacteristics> <Track> ) ] ;
    rdfs:isDefinedBy <> ;
    rdfs:range xsd:string ;
    ns1:term_status "stable" .

<verificationENE> a owl:DatatypeProperty ;
    rdfs:label "EC declaration of verification for track relating to compliance with the requirements from TSIs applicable to energy subsystem"@en ;
    <XMLName> "EDE_ECVerification" ;
    <rinfIndex> "1.1.1.2.1.1" ;
    dcterms:created "2021-08-08"^^xsd:date ;
    dcterms:modified "2024-01-08"^^xsd:date ;
    rdfs:comment "Unique number for EC declarations in accordance with Commission Implementing Regulation (EU) 2019/250."@en ;
    rdfs:domain [ a owl:Class ;
            owl:unionOf ( <SubsetWithCommonCharacteristics> <Track> ) ] ;
    rdfs:isDefinedBy <> ;
    rdfs:range xsd:string ;
    ns1:term_status "stable" .

<verificationSRT> a owl:DatatypeProperty ;
    rdfs:label "EC declaration of verification relating to compliance with the requirements from TSIs applicable to railway tunnel"@en ;
    <XMLName> "ITU_ECVerification" ;
    <rinfIndex> "1.1.1.1.8.5",
        "1.2.1.0.5.3",
        "1.2.2.0.5.3" ;
    dcterms:created "2021-08-03"^^xsd:date ;
    dcterms:modified "2024-01-08"^^xsd:date ;
    rdfs:comment "Unique number for EC declarations in accordance with Commission Implementing Regulation (EU) 2019/250."@en ;
    rdfs:domain <Tunnel> ;
    rdfs:isDefinedBy <> ;
    rdfs:range xsd:string ;
    ns1:term_status "stable" .

<voiceRadioCompatible> a owl:ObjectProperty ;
    rdfs:label "Radio system compatibility voice"@en ;
    <XMLName> "CRG_RadioCompVoice" ;
    <eratvIndex> "4.13.2.5" ;
    <inSkosConceptScheme> <concepts/radio-system-compatibilities-voice/RadioSystemCompatibilitiesVoice> ;
    <rinfIndex> "1.1.1.3.3.9",
        "1.2.1.1.2.9" ;
    dcterms:created "2020-08-31"^^xsd:date ;
    dcterms:modified "2021-09-12"^^xsd:date ;
    rdfs:comment """Radio requirements used for demonstrating technical compatibility voice.
 The allowed values for this property belong to the SKOS Concept Scheme http://data.europa.eu/949/concepts/voice-radio-system-compatibilities/VoiceRadioSystemCompatibilities. This concept scheme is temporatily non-deferenceable."""@en ;
    rdfs:domain [ a owl:Class ;
            owl:unionOf ( <Track> <VehicleType> ) ] ;
    rdfs:isDefinedBy <> ;
    rdfs:range ns2:Concept ;
    ns1:term_status "stable" .

<wheelSetGauge> a owl:FunctionalProperty,
        owl:ObjectProperty ;
    rdfs:label "Nominal track gauge"@en ;
    <XMLName> "ITP_NomGauge" ;
    <eratvIndex> "4.1.3" ;
    <inSkosConceptScheme> <concepts/nominal-track-gauges/NominalTrackGauges> ;
    <rinfIndex> "1.1.1.1.4.1",
        "1.2.1.0.4.1" ;
    <usedInRCCCalculations> true ;
    dcterms:created "2020-07-29"^^xsd:date ;
    dcterms:modified "2024-01-08"^^xsd:date ;
    rdfs:comment """Value expressed in millimetres that identifies the track gauge.
The allowed values for this property belong to the SKOS Concept Scheme http://data.europa.eu/949/concepts/nominal-track-gauges/NominalTrackGauges"""@en ;
    rdfs:domain [ a owl:Class ;
            owl:unionOf ( <Track> <VehicleType> ) ] ;
    rdfs:isDefinedBy <> ;
    rdfs:range ns2:Concept ;
    ns1:term_status "stable" .

<ETCSLevel> a owl:Class ;
    rdfs:label "ETCS Level"@en ;
    <rinfIndex> "1.1.1.3.2" ;
    dcterms:created "2021-08-07"^^xsd:date ;
    dcterms:modified "2021-08-07"^^xsd:date ;
    rdfs:comment "ERTMS / ETCS application level related to the track side equipment."@en ;
    rdfs:isDefinedBy <> ;
    ns1:term_status "stable" .

<InfrastructureManager> a owl:Class ;
    rdfs:label "Infrastructure manager"@en ;
    rdfs:comment "The infrastructure manager owns and operates the railway network and related infrastructure."@en ;
    rdfs:isDefinedBy <> ;
    rdfs:seeAlso "https://wiki3.railml.org/wiki/CO:infrastructureManager"^^xsd:anyURI ;
    rdfs:subClassOf <http://www.w3.org/ns/org#Organization> ;
    ns2:scopeNote "See point (2) of Article 3 of Directive 2012/34/EU of the European Parliament and of the Council establishing a single European railway area."@en .

<MaximumMagneticField> a owl:Class ;
    rdfs:label "Maximum magnetic field"@en ;
    dcterms:created "2023-03-14"^^xsd:date ;
    rdfs:comment """The maximum magnetic field limits allowed for axle counters (in dBµA/m) for a defined frequency band.
It should be provided in 3 directions."""@en ;
    rdfs:isDefinedBy <> ;
    ns1:term_status "stable" .

<MinAxleLoadVehicleCategory> a owl:Class ;
    rdfs:label "Min axle load vehicle category"@en ;
    dcterms:created "2023-01-25"^^xsd:date ;
    dcterms:modified "2023-03-14"^^xsd:date ;
    rdfs:comment "Deprecated according to the ammendment to the Regulation (EU) 2019/777. Represents information that indicates the load given in tons depending of the category of vehicle. Its properties are minAxleLoadVehicleCategory and minAxleLoad."@en ;
    rdfs:isDefinedBy <> ;
    owl:deprecated true ;
    ns1:term_status "stable" .

<RaisedPantographsDistanceAndSpeed> a owl:Class ;
    rdfs:label "Raised pantographs distance and speed"@en ;
    dcterms:created "2023-04-05"^^xsd:date ;
    rdfs:comment """Indication of maximum number of raised pantographs per train allowed and minimum spacing centre line to centre line of adjacent pantograph heads, expressed in metres, at the given speed.
Each track can have several raised pantographs per train allowed (structured) values, and each one has values for number of pantographs, minimum distance between pantographs, in metres, and speed considered in km/h."""@en ;
    rdfs:isDefinedBy <> ;
    ns1:term_status "stable" .

<Signal> a owl:Class ;
    rdfs:label "Signal"@en ;
    <rinfIndex> "1.2.1.0.8" ;
    ns3:source <https://eur-lex.europa.eu/eli/reg_impl/2019/773/oj> ;
    dcterms:created "2021-04-01"^^xsd:date ;
    dcterms:modified "2022-10-27"^^xsd:date ;
    rdfs:comment """A railway signal is an installation next to the railway track for signalling the maximum allowed speed in the next block section to the train driver.
Definition RSM: Apparatus by means of which a conventional visual or acoustic indication is given, generally concerning the movements of railway vehicles."""@en ;
    rdfs:isDefinedBy <> ;
    rdfs:seeAlso <https://rsm-evolution.org/220927_RSM/EARoot/EA4/EA3/EA978.html>,
        <https://wiki3.railml.org/DataModel/3.2/IS/EARoot/EA271.htm> ;
    rdfs:subClassOf <InfrastructureObject> ;
    ns1:term_status "stable" .

<SpecialArea> a owl:Class ;
    rdfs:label "Special area"@en ;
    ns3:source <https://eur-lex.europa.eu/eli/reg_impl/2019/773/oj> ;
    dcterms:created "2022-10-27"^^xsd:date ;
    rdfs:comment "Encompasses all those areas or sections such as safe areas, restricted areas (non-stopping areas or industrial risk locations)."@en ;
    rdfs:isDefinedBy <> ;
    rdfs:seeAlso <https://wiki3.railml.org/DataModel/3.2/IS/EARoot/EA258.htm> ;
    rdfs:subClassOf <InfrastructureObject> ;
    ns1:term_status "stable" .

<SpecialTunnelArea> a owl:Class ;
    rdfs:label "Special tunnel area"@en ;
    ns3:source <https://eur-lex.europa.eu/eli/reg_impl/2019/773/oj> ;
    dcterms:created "2022-10-27"^^xsd:date ;
    rdfs:comment "Area or location within a tunnel where  there is a walkway, evacuation and rescue points."@en ;
    rdfs:isDefinedBy <> ;
    rdfs:subClassOf <SpecialArea> ;
    ns1:term_status "stable" .

<Vehicle> a owl:Class ;
    rdfs:label "Vehicle"@en ;
    dcterms:created "2020-11-22"^^xsd:date ;
    dcterms:modified "2020-11-22"^^xsd:date ;
    rdfs:comment "A specific vehicle or wagon able to operate over railway lines."@en ;
    rdfs:isDefinedBy <> ;
    ns1:term_status "stable" .

<frenchTrainDetectionSystemLimitationApplicable> a owl:DatatypeProperty ;
    rdfs:label "Section with train detection limitation"@en ;
    <XMLName> "CTD_TCLimitation" ;
    <rinfIndex> "1.2.1.1.6.3"^^rdfs:Literal,
        "1.1.1.3.7.1.4" ;
    <usedInRCCCalculations> true ;
    dcterms:created "2023-04-05"^^xsd:date ;
    rdfs:comment "Part of the section with train detection limitation that indicates if it is applicable. Only for the French network."@en ;
    rdfs:domain <FrenchTrainDetectionSystemLimitation> ;
    rdfs:isDefinedBy <> ;
    rdfs:range xsd:boolean ;
    ns1:term_status "stable" .

<frenchTrainDetectionSystemLimitationNumber> a owl:ObjectProperty ;
    rdfs:label "Section with train detection limitation number, only for French  network"@en ;
    <XMLName> "CTD_TCLimitation" ;
    <inSkosConceptScheme> <concepts/train-detection-numbers/FrenchTrainDetectionSystemLimitationNumbers> ;
    <rinfIndex> "1.1.1.3.7.1.4",
        "1.2.1.1.6.3" ;
    <usedInRCCCalculations> true ;
    dcterms:created "2023-04-05"^^xsd:date ;
    rdfs:comment "Part of the section with train detection limitation that indicates the type of train detection limitation."@en ;
    rdfs:domain <FrenchTrainDetectionSystemLimitation> ;
    rdfs:isDefinedBy <> ;
    rdfs:range ns2:Concept ;
    ns1:term_status "stable" .

<lineNationalId> a owl:FunctionalProperty,
        owl:ObjectProperty ;
    rdfs:label "National line identification"@en ;
    <XMLName> "SOLLineIdentification" ;
    <appendixD2Index> "2.2.1.1" ;
    <rinfIndex> "1.1.0.0.0.2" ;
    dcterms:created "2020-09-30"^^xsd:date ;
    dcterms:modified "2023-03-14"^^xsd:date ;
    rdfs:comment "Unique line identification or unique line number within Member State."@en ;
    rdfs:domain [ a owl:Class ;
            owl:unionOf ( <LineReference> <SectionOfLine> ) ] ;
    rdfs:isDefinedBy <> ;
    rdfs:range <NationalRailwayLine> ;
    ns1:term_status "stable" .

<lineReferenceTunnelEnd> a owl:ObjectProperty ;
    rdfs:label "End of tunnel kilometer"@en ;
    <XMLName> "SOLTunnelEnd" ;
    <rinfIndex> "1.1.1.1.8.4" ;
    dcterms:created "2024-02-05"^^xsd:date ;
    rdfs:comment """Part of the End of tunnel that indicates the km of the line at the end of a tunnel.
The End of tunnel is the Geographical coordinates in decimal degrees and km of the line at the end of a tunnel."""@en ;
    rdfs:domain <Tunnel> ;
    rdfs:isDefinedBy <> ;
    rdfs:range <LineReference> ;
    rdfs:subPropertyOf <lineReference> ;
    ns1:term_status "stable" .

<lineReferenceTunnelStart> a owl:ObjectProperty ;
    rdfs:label "Start of tunnel kilometer"@en ;
    <XMLName> "SOLTunnelStart" ;
    <rinfIndex> "1.1.1.1.8.3" ;
    dcterms:created "2024-02-05"^^xsd:date ;
    rdfs:comment """Part of the Start of tunnel that indicates the km of the line at the beginning of a tunnel.
The Start of tunnel is the Geographical coordinates in decimal degrees and km of the line at the end of a tunnel."""@en ;
    rdfs:domain <Tunnel> ;
    rdfs:isDefinedBy <> ;
    rdfs:range <LineReference> ;
    rdfs:subPropertyOf <lineReference> ;
    ns1:term_status "stable" .

<loadCapabilityLineCategory> a owl:ObjectProperty ;
    rdfs:label "Load capability line category"@en ;
    <XMLName> "IPP_LoadCap" ;
    <inSkosConceptScheme> <concepts/load-capability-line-categories/LoadCapabilityLineCategories> ;
    <rinfIndex> "1.1.1.1.2.4" ;
    <usedInRCCCalculations> true ;
    dcterms:created "2023-01-20"^^xsd:date ;
    rdfs:comment """Part of the load capability of a track that corresponds to the line category of the load model. 
The load capability is a value selected from the list of load models representing: line category which is amended by value of speed [km/h] permitted for a specific load model. The list of values may also be Route Availability which is amended by value of speed [miles/h] permitted for a specific load model."""@en ;
    rdfs:domain <LoadCapability> ;
    rdfs:isDefinedBy <> ;
    rdfs:range ns2:Concept ;
    ns1:term_status "stable" .

<loadCapabilitySpeed> a owl:DatatypeProperty ;
    rdfs:label "Load capability speed"@en ;
    <XMLName> "IPP_LoadCap" ;
    <rinfIndex> "1.1.1.1.2.4" ;
    <unitOfMeasure> <http://qudt.org/vocab/unit/KiloM-PER-HR> ;
    <usedInRCCCalculations> true ;
    dcterms:created "2023-01-20"^^xsd:date ;
    rdfs:comment """Part of the load capability of a track that corresponds to the speed of the load model. 
The load capability is a value selected from the list of load models representing: line category which is amended by value of speed [km/h] permitted for a specific load model. The list of values may also be Route Availability which is amended by value of speed [miles/h] permitted for a specific load model."""@en ;
    rdfs:domain <LoadCapability> ;
    rdfs:isDefinedBy <> ;
    rdfs:range xsd:integer ;
    ns1:term_status "stable" .

<manufacturer> a owl:ObjectProperty ;
    rdfs:label "Manufacturer"@en ;
    dcterms:created "2020-07-29"^^xsd:date ;
    dcterms:modified "2020-11-19"^^xsd:date ;
    rdfs:comment "Vehicle manufacturer company."@en ;
    rdfs:domain <VehicleType> ;
    rdfs:isDefinedBy <> ;
    rdfs:range <Manufacturer> ;
    ns1:term_status "stable" .

<minimumVerticalRadiusCrest> a owl:DatatypeProperty ;
    rdfs:label "Minimum radius of vertical curve crest"@en ;
    <XMLName> "ILL_MinRadVertCurve" ;
    <rinfIndex> "1.2.2.0.3.3" ;
    <unitOfMeasure> <http://qudt.org/vocab/unit/M> ;
    <usedInRCCCalculations> true ;
    dcterms:created "2023-04-05"^^xsd:date ;
    rdfs:comment """Part of the minimum radius of vertical curve that indicates the crest. 
The minimum radius of vertical curve is the radius of the smallest vertical curve expressed in metres."""@en ;
    rdfs:domain <Siding> ;
    rdfs:isDefinedBy <> ;
    rdfs:range xsd:integer ;
    ns1:term_status "stable" .

<minimumVerticalRadiusHollow> a owl:DatatypeProperty ;
    rdfs:label "Minimum radius of vertical curve hollow"@en ;
    <XMLName> "ILL_MinRadVertCurve" ;
    <rinfIndex> "1.2.2.0.3.3" ;
    <unitOfMeasure> <http://qudt.org/vocab/unit/M> ;
    <usedInRCCCalculations> true ;
    dcterms:created "2023-04-05"^^xsd:date ;
    rdfs:comment """Part of the minimum radius of vertical curve that indicates the hollow. 
The minimum radius of vertical curve is the radius of the smallest vertical curve expressed in metres."""@en ;
    rdfs:domain <Siding> ;
    rdfs:isDefinedBy <> ;
    rdfs:range xsd:integer ;
    ns1:term_status "stable" .

<opEnd> a owl:ObjectProperty ;
    rdfs:label "Operational point at end of section of line"@en ;
    <XMLName> "SOLOPEnd" ;
    <appendixD2Index> "3.1.2" ;
    <rinfIndex> "1.1.0.0.0.4" ;
    dcterms:created "2021-09-09"^^xsd:date ;
    dcterms:modified "2024-01-08"^^xsd:date ;
    dcterms:source <https://eur-lex.europa.eu/eli/reg_impl/2019/773/oj> ;
    rdfs:comment "Unique OP ID at end of section of line (kilometres increasing from start OP to the end OP)."@en ;
    rdfs:domain <SectionOfLine> ;
    rdfs:isDefinedBy <> ;
    rdfs:range <OperationalPoint> ;
    ns1:term_status "stable" .

<opStart> a owl:ObjectProperty ;
    rdfs:label "Operational point at start of section of line"@en ;
    <XMLName> "SOLOPStart" ;
    <appendixD2Index> "3.1.1" ;
    <rinfIndex> "1.1.0.0.0.3" ;
    dcterms:created "2021-09-09"^^xsd:date ;
    dcterms:modified "2024-01-08"^^xsd:date ;
    dcterms:source <https://eur-lex.europa.eu/eli/reg_impl/2019/773/oj> ;
    rdfs:comment "Unique OP ID at start of section of line (kilometres increasing from start OP to the end OP)."@en ;
    rdfs:domain <SectionOfLine> ;
    rdfs:isDefinedBy <> ;
    rdfs:range <OperationalPoint> ;
    ns1:term_status "stable" .

<phaseInfoLength> a owl:DatatypeProperty ;
    rdfs:label "Phase info length"@en ;
    <XMLName> "EOS_InfoPhase" ;
    <rinfIndex> "1.1.1.2.4.1.2" ;
    <unitOfMeasure> <http://qudt.org/vocab/unit/M> ;
    dcterms:created "2023-04-05"^^xsd:date ;
    rdfs:comment """Part of the phase info of a track that corresponds to the length of the phase separation in metres. 
The phase info is the indication of required several information on phase separation."""@en ;
    rdfs:domain <PhaseInfo> ;
    rdfs:isDefinedBy <> ;
    rdfs:range xsd:integer ;
    ns1:term_status "stable" .

<phaseInfoPantographLowered> a owl:DatatypeProperty ;
    rdfs:label "Phase info pantograph lowered"@en ;
    <XMLName> "EOS_InfoPhase" ;
    <rinfIndex> "1.1.1.2.4.1.2" ;
    dcterms:created "2023-04-05"^^xsd:date ;
    rdfs:comment """Part of the phase info of a track that shows whether a pantograph has to be lowered.
The phase info is the indication of required several information on phase separation."""@en ;
    rdfs:domain <PhaseInfo> ;
    rdfs:isDefinedBy <> ;
    rdfs:range xsd:boolean ;
    ns1:term_status "stable" .

<phaseInfoSwitchOffBreaker> a owl:DatatypeProperty ;
    rdfs:label "Phase info switch off breaker"@en ;
    <XMLName> "EOS_InfoPhase" ;
    <rinfIndex> "1.1.1.2.4.1.2" ;
    dcterms:created "2023-04-05"^^xsd:date ;
    rdfs:comment """Part of the phase info of a track that shows whether the breaker has to be switched off.
The phase info is the indication of required several information on phase separation."""@en ;
    rdfs:domain <PhaseInfo> ;
    rdfs:isDefinedBy <> ;
    rdfs:range xsd:boolean ;
    ns1:term_status "stable" .

<systemSeparationInfoKm> a owl:DatatypeProperty ;
    rdfs:label "System separation info Km"@en ;
    <XMLName> "EOS_InfoSystem" ;
    <rinfIndex> "1.1.1.2.4.2.2" ;
    dcterms:created "2023-04-05"^^xsd:date ;
    rdfs:comment """Part of the system separation info of a track.  Indicates the the location from the start of the line where the new value is valid.
The system separation info is the Indication of required several information on system separation."""@en ;
    rdfs:domain <SystemSeparationInfo> ;
    rdfs:isDefinedBy <> ;
    rdfs:range xsd:double ;
    ns1:term_status "stable" .

<systemSeparationInfoLength> a owl:DatatypeProperty ;
    rdfs:label "System separation info length"@en ;
    <XMLName> "EOS_InfoSystem" ;
    <rinfIndex> "1.1.1.2.4.2.2" ;
    <unitOfMeasure> <http://qudt.org/vocab/unit/M> ;
    dcterms:created "2023-04-05"^^xsd:date ;
    rdfs:comment """Part of the system separation info of a track that shows the length of the system separation in metres.
The system separation info is the Indication of required several information on system separation."""@en ;
    rdfs:domain <SystemSeparationInfo> ;
    rdfs:isDefinedBy <> ;
    rdfs:range xsd:integer ;
    ns1:term_status "stable" .

<systemSeparationInfoSwitchOffBreaker> a owl:DatatypeProperty ;
    rdfs:label "System separation info switch off breaker"@en ;
    <XMLName> "EOS_InfoSystem" ;
    <rinfIndex> "1.1.1.2.4.2.2" ;
    dcterms:created "2023-04-05"^^xsd:date ;
    rdfs:comment """Part of the system separation info of a track that shows whether the breaker has to be switched off.
The system separation info is the Indication of required several information on system separation."""@en ;
    rdfs:domain <SystemSeparationInfo> ;
    rdfs:isDefinedBy <> ;
    rdfs:range xsd:boolean ;
    ns1:term_status "stable" .

<tdsFrenchTrainDetectionSystemLimitation> a owl:ObjectProperty ;
    rdfs:label "Section with train detection limitation, only for the French network"@en ;
    <XMLName> "CTD_TCLimitation" ;
    <rinfIndex> "1.1.1.3.7.1.4",
        "1.2.1.1.6.3" ;
    <usedInRCCCalculations> true ;
    dcterms:created "2023-04-05"^^xsd:date ;
    rdfs:comment """Relates the class train detection system with the class that represents the section with train detection limitation. 
Specific for route compatibility check on French network."""@en ;
    rdfs:domain <TrainDetectionSystem> ;
    rdfs:isDefinedBy <> ;
    rdfs:range <FrenchTrainDetectionSystemLimitation> ;
    ns1:term_status "stable" .

<trackLoadCapability> a owl:ObjectProperty ;
    rdfs:label "Track load capability"@en ;
    <XMLName> "IPP_LoadCap" ;
    <rinfIndex> "1.1.1.1.2.4" ;
    <usedInRCCCalculations> true ;
    dcterms:created "2023-01-20"^^xsd:date ;
    rdfs:comment "Relates the track with the class LoadCapability. A combination of the line category and speed at the weakest point of the track."@en ;
    rdfs:domain [ a owl:Class ;
            owl:unionOf ( <SubsetWithCommonCharacteristics> <Track> ) ] ;
    rdfs:isDefinedBy <> ;
    rdfs:range <LoadCapability> ;
    rdfs:subPropertyOf owl:topObjectProperty ;
    ns1:term_status "stable" .

<trackSystemSeparationInfo> a owl:ObjectProperty ;
    rdfs:label "Track system separation info"@en ;
    <XMLName> "EOS_InfoSystem" ;
    <rinfIndex> "1.1.1.2.4.2.2" ;
    dcterms:created "2023-04-05"^^xsd:date ;
    rdfs:comment "Relates the Track with the SystemSeparationInfo. Indication of required several information on system separation."@en ;
    rdfs:domain [ a owl:Class ;
            owl:unionOf ( <SubsetWithCommonCharacteristics> <Track> ) ] ;
    rdfs:isDefinedBy <> ;
    rdfs:range <SystemSeparationInfo> ;
    ns1:term_status "stable" .

<http://www.opengis.net/ont/geosparql#wktLiteral> a rdfs:Datatype .

ns2:ConceptScheme a owl:Class .

<http://xmlns.com/foaf/0.1/Agent> a owl:Class .

<http://xmlns.com/foaf/0.1/Document> a owl:Class ;
    rdfs:label "Document" ;
    rdfs:comment "A document." ;
    rdfs:isDefinedBy <http://xmlns.com/foaf/0.1/> ;
    owl:disjointWith <http://xmlns.com/foaf/0.1/Organization>,
        <http://xmlns.com/foaf/0.1/Project> ;
    ns1:term_status "stable" .

<http://xmlns.com/foaf/0.1/Organization> a owl:Class .

<http://xmlns.com/foaf/0.1/Project> a owl:Class .

<http://xmlns.com/foaf/0.1/based_near> a owl:AnnotationProperty .

<Feature> a owl:Class ;
    rdfs:label "ERA Feature"@en ;
    dcterms:created "2022-07-07"^^xsd:date ;
    dcterms:modified "2022-10-27"^^xsd:date ;
    rdfs:comment "Class that encompasses the features that are part of the physical infrastructure (class InfrastructureObject) and the topological objects (class TopologicalObject). It is a subclass of the geographical Feature class that has a spatial representation."@en ;
    rdfs:isDefinedBy <> ;
    rdfs:subClassOf <http://www.opengis.net/ont/geosparql#Feature> .

<Manufacturer> a owl:Class ;
    rdfs:label "Manufacturer"@en ;
    dcterms:created "2020-11-19"^^xsd:date ;
    dcterms:modified "2020-11-19"^^xsd:date ;
    rdfs:comment "A company or organization that manufactures vehicles."@en ;
    rdfs:isDefinedBy <> ;
    rdfs:subClassOf <http://www.w3.org/ns/org#Organization> ;
    ns1:term_status "stable" .

<NationalRailwayLine> a owl:Class ;
    rdfs:label "National railway line"@en ;
    dcterms:created "2021-01-25"^^xsd:date ;
    dcterms:modified "2021-08-03"^^xsd:date ;
    rdfs:comment "Railway line within a member state."@en ;
    rdfs:isDefinedBy <> ;
    rdfs:seeAlso <https://wiki3.railml.org/DataModel/3.2/IS/EARoot/EA210.htm> ;
    ns1:term_status "stable" .

<lineReference> a owl:ObjectProperty ;
    rdfs:label "Railway location of an infrastructure object"@en ;
    dcterms:created "2021-01-29"^^xsd:date ;
    dcterms:modified "2023-03-14"^^xsd:date ;
    rdfs:comment "Indicates a relationship with a national railway line at a specific kilometer point."@en ;
    rdfs:domain <InfrastructureObject> ;
    rdfs:isDefinedBy <> ;
    rdfs:range <LineReference> ;
    ns1:term_status "stable" .

<http://www.opengis.net/ont/geosparql#Feature> a owl:Class .

<http://www.opengis.net/ont/geosparql#hasGeometry> a owl:ObjectProperty ;
    rdfs:label "hasGeometry"@en ;
    <XMLName> "OPGeographicLocation" ;
    <rinfIndex> "1.1.0.0.1.1",
        "1.1.1.0.1.1",
        "1.1.1.3.14.6",
        "1.2.0.0.0.5",
        "1.2.1.0.8.5" ;
    <usedInRCCCalculations> true ;
    ns3:contributor "Matthew Perry" ;
    ns3:creator "OGC GeoSPARQL 1.0 Standard Working Group" ;
    ns3:date "2011-06-16"^^xsd:date ;
    ns3:description """
      A spatial representation for a given feature.
    """@en ;
    rdfs:comment """
      A spatial representation for a given feature.
    """@en ;
    rdfs:domain <http://www.opengis.net/ont/geosparql#Feature> ;
    rdfs:isDefinedBy <http://www.opengis.net/ont/geosparql>,
        <http://www.opengis.net/spec/geosparql/1.0> ;
    rdfs:range <http://www.opengis.net/ont/geosparql#Geometry> ;
    ns2:definition """
      A spatial representation for a given feature.
    """@en ;
    ns2:prefLabel "hasGeometry"@en .

xsd:date a rdfs:Datatype .

<http://www.w3.org/2003/01/geo/wgs84_pos#Point> a owl:Class ;
    rdfs:label "Point" ;
    rdfs:comment """ 
Uniquely identified by lat/long/alt. i.e.

spaciallyIntersects(P1, P2) :- lat(P1, LAT), long(P1, LONG), alt(P1, ALT),
  lat(P2, LAT), long(P2, LONG), alt(P2, ALT).

sameThing(P1, P2) :- type(P1, Point), type(P2, Point), spaciallyIntersects(P1, P2).
  """,
        """A point, typically described using a coordinate system relative to Earth, such as WGS84.
  """ ;
    rdfs:subClassOf <http://www.w3.org/2003/01/geo/wgs84_pos#SpatialThing> .

<http://www.w3.org/2003/01/geo/wgs84_pos#SpatialThing> a owl:Class ;
    rdfs:label "SpatialThing" ;
    rdfs:comment """Anything with spatial extent, i.e. size, shape, or position.
 e.g. people, places, bowling balls, as well as abstract areas like cubes.
""" .

<http://www.w3.org/2003/01/geo/wgs84_pos#location> a owl:AnnotationProperty,
        owl:ObjectProperty ;
    rdfs:label "Location" ;
    <rinfIndex> "1.1.0.0.1.1",
        "1.1.1.0.1.1",
        "1.1.1.3.14.6",
        "1.2.0.0.0.5",
        "1.2.1.0.8.5" ;
    <usedInRCCCalculations> true ;
    rdfs:comment """The relation between something and the point, 
 or other geometrical thing in space, where it is.  For example, the realtionship between
 a radio tower and a Point with a given lat and long.
 Or a relationship between a park and its outline as a closed arc of points, or a road and
 its location as a arc (a sequence of points).
 Clearly in practice there will be limit to the accuracy of any such statement, but one would expect
 an accuracy appropriate for the size of the object and uses such as mapping .
 """ ;
    rdfs:range <http://www.w3.org/2003/01/geo/wgs84_pos#SpatialThing> ;
    rdfs:subPropertyOf <http://xmlns.com/foaf/0.1/based_near> .

<http://www.w3.org/ns/org#Organization> a owl:Class ;
    rdfs:label "Organization"@en,
        "organización"@es,
        "Organisation"@fr,
        "Organizzazione"@it ;
    rdfs:comment "Represents a collection of people organized together into a community or other social, commercial or political structure. The group has some common purpose or reason for existence which goes beyond the set of people belonging to it and can act as an Agent. Organizations are often decomposable into hierarchical structures.  It is recommended that SKOS lexical labels should be used to label the Organization. In particular `skos:prefLabel` for the primary (possibly legally recognized name), `skos:altLabel` for alternative names (trading names, colloquial names) and `skos:notation` to denote a code from a code list. Alternative names: _Collective_ _Body_ _Org_ _Group_"@en,
        "Grupo de personas que se organiza en una comunidad u otro tipo de estructura social, comercial o política. Dicho grupo tiene un objetivo o motivo común para su existencia que va más allá del conjunto de personas que lo forman y que puede actuar como “agente”. A menudo las organizaciones se pueden agrupar en estructuras jerárquicas. Se recomienda el uso de etiquetas de SKOS para denominar a cada “organización”. En concreto, `skos:prefLabel` para la denominación principal o recomendada (aquella reconocida legalmente, siempre que sea posible), `skos:altLabel` para denominaciones alternativas (nombre comercial, sigla, denominación por la que se conoce a la organización coloquialmente) y `skos:notation` para referirse al código que identifique a la organización en una lista de códigos. Denominaciones alternativas: _colectivo_ _corporación_ _grupo_"@es,
        "Représente un groupe de personnes organisées en communauté où tout autre forme de structure sociale, commerciale ou politique. Le groupe a un but commun ou une raison d'être qui va au-delà de la somme des personnes qui en font partie et peut agir en tant que \"Agent\". Les organisations sont souvent décomposables en structures hiérarchisées. Il est recommandé que des labels lexicaux SKOS soient utilisés pour nommer l'Organisation. En particulier `skos:prefLabel` pour le nom principal (en général le nom légal), `skos:altLabel` pour les noms alternatifs (marques, sigles, appellations familières) et `skos:notation` pour indiquer un code provenant d'une liste de code."@fr,
        "Rappresenta una collezione di persone organizzate all'interno di una communità o di una qualche struttura sociale, commerciale o politica. Il gruppo condivide un obiettivo o una ragione d'essere che va oltre gli stessi membri appartenenti al gruppo e  può agire come un Agent. Le organizzazioni si possono spesso suddividere in strutture gerarchiche. Si raccomanda di usare le label per l'Organization mediante le proprietà di SKOS. In particolare, `skos:prefLabel` per il nome principale (possibilmente un nome legalmente riconosciuto)”, `skos:altLabel` come nome alternativo (denominazione commerciale, denominazione colloquiale) e `skos:notation` per indicare un codice di una lista di codici."@it,
        "コミュニティー、その他の社会、商業、政治的な構造に共に編入された人々の集合を表わします。グループには、そこに属する人々を超えた、存在に対するある共通の目的や理由があり、エージェント（代理）を務めることができます。組織は、多くの場合、階層構造に分割できます。"@ja ;
    rdfs:isDefinedBy <http://www.w3.org/ns/org> ;
    rdfs:subClassOf <http://xmlns.com/foaf/0.1/Agent> .

<FrenchTrainDetectionSystemLimitation> a owl:Class ;
    rdfs:label "Section with train detection limitation, only for the French network"@en ;
    dcterms:created "2023-04-05"^^xsd:date ;
    rdfs:comment """Specific for route compatibility check on French network. Sections with: 
-1 Tonnage circulated per track is inferior to 15000 tons/day/track 
-2 Directional Interlocking 
-3 45-second delay for directional interlocking 
-4 Installation with track circuit announcement 
-5 Absence of a shunting assistance pedal in the normal direction of circulation for non-reversible double track lines 
-6 Absence of a shunting assistance pedal regardless of the direction of traffic for single track lines and tracks for two way working 
-7 Absence of a pedal announcement mechanism 
-8 45-second delay for specific announcement reset devices"""@en ;
    rdfs:isDefinedBy <> ;
    ns1:term_status "stable" .

<http://www.opengis.net/ont/geosparql#Geometry> a owl:Class .

<LineReference> a owl:Class ;
    rdfs:label "Railway location"@en ;
    dcterms:created "2021-01-29"^^xsd:date ;
    dcterms:modified "2021-01-29"^^xsd:date ;
    rdfs:comment "A reference to a specific national railway line."@en ;
    rdfs:isDefinedBy <> ;
    ns1:term_status "stable" ;
    ns2:altLabel "Line reference" .

<LoadCapability> a owl:Class ;
    rdfs:label "Load capability"@en ;
    dcterms:created "2023-03-14"^^xsd:date ;
    rdfs:comment """A combination of the line category and speed at the weakest point of the track. 
Each track can have several load capability (structured) values, and each one has values for load model line category and load model speed."""@en,
        "This class together with properties loadCapabilityLineCategory and loadCapabilitySpeed replaces the previous loadCapability SKOS property."@en ;
    rdfs:isDefinedBy <> ;
    ns1:term_status "stable" .

<PhaseInfo> a owl:Class ;
    rdfs:label "Phase info"@en ;
    dcterms:created "2023-04-05"^^xsd:date ;
    rdfs:comment "Indication of required several information on phase separation."@en ;
    rdfs:isDefinedBy <> ;
    ns1:term_status <stable> .

<length> a owl:DatatypeProperty,
        owl:FunctionalProperty ;
    rdfs:label "Length"@en ;
    <XMLName> "IPL_Length",
        "IPP_Length",
        "ITU_Length",
        "SOLLength" ;
    <appendixD2Index> "2.3.6" ;
    <eratvIndex> "4.8.1" ;
    <rinfIndex> "1.1.0.0.0.5",
        "1.1.1.1.8.12.1",
        "1.1.1.1.8.13.1",
        "1.1.1.1.8.7",
        "1.1.1.3.14.5",
        "1.2.1.0.5.10.1",
        "1.2.1.0.5.11.1",
        "1.2.1.0.5.5",
        "1.2.1.0.6.4",
        "1.2.2.0.2.1",
        "1.2.2.0.5.10.1",
        "1.2.2.0.5.5",
        "1.2.2.0.5.9.1" ;
    <unitOfMeasure> <http://qudt.org/vocab/unit/M> ;
    <usedInRCCCalculations> true ;
    dcterms:created "2021-04-01"^^xsd:date ;
    dcterms:modified "2024-01-08"^^xsd:date ;
    dcterms:source <https://eur-lex.europa.eu/eli/reg_impl/2019/773/oj> ;
    rdfs:comment """Length of an infrastructure object which can be a section of line, a tunnel, a platform, a siding, and length of other areas such as a non-stopping area, a walkway, an evacuation and rescue point.
Vehicle length."""@en ;
    rdfs:domain [ a owl:Class ;
            owl:unionOf ( <Feature> <Vehicle> ) ] ;
    rdfs:isDefinedBy <> ;
    rdfs:range xsd:double ;
    ns1:term_status "stable" .

<SystemSeparationInfo> a owl:Class ;
    rdfs:label "System separation info"@en ;
    dcterms:created "2023-04-05"^^xsd:date ;
    rdfs:comment "Indication of required several information on system separation."@en ;
    rdfs:isDefinedBy <> ;
    ns1:term_status "stable" .

<SectionOfLine> a owl:Class ;
    rdfs:label "Section Of Line"@en ;
    <appendixD2Index> "2.1.1" ;
    <rinfIndex> 1.1 ;
    ns3:source <https://eur-lex.europa.eu/eli/reg_impl/2019/773/oj> ;
    dcterms:created "2021-04-02"^^xsd:date ;
    dcterms:modified "2022-07-07"^^xsd:date ;
    rdfs:comment "A section of line means the part of line between adjacent operational points and may consist of several tracks."@en ;
    rdfs:isDefinedBy <> ;
    rdfs:subClassOf [ a owl:Restriction ;
            owl:onClass <NationalRailwayLine> ;
            owl:onProperty <lineNationalId> ;
            owl:qualifiedCardinality "1"^^xsd:nonNegativeInteger ],
        [ a owl:Restriction ;
            owl:onClass <OperationalPoint> ;
            owl:onProperty <opEnd> ;
            owl:qualifiedCardinality "1"^^xsd:nonNegativeInteger ],
        [ a owl:Restriction ;
            owl:onClass <OperationalPoint> ;
            owl:onProperty <opStart> ;
            owl:qualifiedCardinality "1"^^xsd:nonNegativeInteger ],
        <InfrastructureObject> ;
    ns1:term_status "stable" .

dcterms:identifier a owl:DatatypeProperty ;
    rdfs:label "Identifier"@en ;
    dcterms:description "Recommended practice is to identify the resource by means of a string conforming to an identification system. Examples include International Standard Book Number (ISBN), Digital Object Identifier (DOI), and Uniform Resource Name (URN).  Persistent identifiers should be provided as HTTP URIs."@en ;
    rdfs:comment "An unambiguous reference to the resource within a given context."@en ;
    rdfs:isDefinedBy dcterms: ;
    rdfs:range rdfs:Literal .

<PlatformEdge> a owl:Class ;
    rdfs:label "Platform edge"@en ;
    <rinfIndex> "1.2.1.0.6" ;
    dcterms:created "2021-08-02"^^xsd:date ;
    dcterms:modified "2023-11-10"^^xsd:date ;
    rdfs:comment "Platform for the purpose of RINF is understood as a platform edge. A platform concerns only the part of the structure neighbouring to the track (interfaced with trains)."@en ;
    rdfs:isDefinedBy <> ;
    rdfs:seeAlso <https://wiki3.railml.org/DataModel/3.2/IS/EARoot/EA250.htm> ;
    rdfs:subClassOf <InfrastructureObject> ;
    ns1:term_status "stable" .

<Document> a owl:Class ;
    rdfs:label "ERA Document"@en ;
    dcterms:created "2024-04-23"^^xsd:date ;
    rdfs:comment "Document in any of the ERA systems, e.g. reference document in RINF."@en ;
    rdfs:isDefinedBy <> ;
    rdfs:subClassOf <http://xmlns.com/foaf/0.1/Document> ;
    ns1:term_status "stable" .

<ContactLineSystem> a owl:Class ;
    rdfs:label "Contact Line System"@en ;
    <rinfIndex> "1.1.1.2.2" ;
    dcterms:created "2021-08-04"^^xsd:date ;
    dcterms:modified "2021-08-04"^^xsd:date ;
    rdfs:comment "System that is used to transmit electrical energy to road or rail vehicles."@en ;
    rdfs:isDefinedBy <> ;
    ns1:term_status "stable" .

<InfrastructureObject> a owl:Class ;
    rdfs:label "Infrastructure object"@en ;
    dcterms:created "2022-07-07"^^xsd:date ;
    dcterms:modified "2022-10-27"^^xsd:date ;
    rdfs:comment """This class encompasses all those classes that represent features that are  implemented in the European railway infrastructure. It is a subclass of the ERA Feature that has a spatial representation. It covers tracks, platforms, signals, tunnels, operational points, and sections of line.
A feature that belongs to the infrastructure can be abstracted (hasAbstraction) as a topological object. It also is related to the infrastructure manager through the property infrastructureMgr."""@en ;
    rdfs:isDefinedBy <> ;
    rdfs:seeAlso <https://wiki3.railml.org/DataModel/3.2/IS/EARoot/EA246.htm> ;
    rdfs:subClassOf <Feature> .

<OperationalPoint> a owl:Class ;
    rdfs:label "Operational Point"@en ;
    <appendixD2Index> "2.1.2" ;
    <rinfIndex> 1.2 ;
    dcterms:created "2020-07-29"^^xsd:date ;
    dcterms:modified "2022-07-07"^^xsd:date ;
    rdfs:comment "An operational point (OP) means any location for train service operations, where train services may begin and end or change route, and where passenger or freight services may be provided; operational point also means any location at boundaries between Member States or infrastructure managers."@en ;
    rdfs:isDefinedBy <> ;
    rdfs:seeAlso <https://wiki3.railml.org/DataModel/3.2/IS/EARoot/EA238.htm> ;
    rdfs:subClassOf <InfrastructureObject> ;
    ns1:term_status "stable" .

<Siding> a owl:Class ;
    rdfs:label "Siding"@en ;
    <rinfIndex> "1.2.2" ;
    dcterms:created "2021-08-10"^^xsd:date ;
    dcterms:modified "2022-10-27"^^xsd:date ;
    dcterms:source "Official Journal of the European Union L 139 I/85" ;
    rdfs:comment "Sidings are all those tracks where running trains in service movements ends and which are not used for operational routing of a train."@en ;
    rdfs:isDefinedBy <> ;
    rdfs:subClassOf <Track> ;
    ns1:term_status "stable" ;
    ns2:definition "Siding Any track(s) within an operational point which is not used for operational routing of a train."@en .

<Tunnel> a owl:Class ;
    rdfs:label "Tunnel"@en ;
    <rinfIndex> "1.2.2.0.5" ;
    ns3:source <https://eur-lex.europa.eu/eli/reg_impl/2019/773/oj> ;
    dcterms:created "2020-07-29"^^xsd:date ;
    dcterms:modified "2022-07-07"^^xsd:date ;
    rdfs:comment "A railway tunnel is an excavation or a construction around the track provided to allow the railway to pass for example higher land, buildings or water."@en ;
    rdfs:isDefinedBy <> ;
    rdfs:subClassOf <InfrastructureObject> ;
    ns1:term_status "stable" .

<TrainDetectionSystem> a owl:Class ;
    rdfs:label "Train Detection System"@en ;
    <rinfIndex> "1.1.1.3.4" ;
    dcterms:created "2021-08-07"^^xsd:date ;
    dcterms:modified "2021-08-07"^^xsd:date ;
    rdfs:comment "System used to detect the position of vehicles in the railway track."@en ;
    rdfs:isDefinedBy <> ;
    rdfs:seeAlso <https://wiki3.railml.org/DataModel/3.2/IS/EARoot/EA402.htm> ;
    ns1:term_status "stable" .

<VehicleType> a owl:Class ;
    rdfs:label "Vehicle Type"@en ;
    dcterms:created "2020-07-29"^^xsd:date ;
    dcterms:modified "2020-07-29"^^xsd:date ;
    rdfs:comment "A vehicle type that has been authorized to operate on the EU railway infrastructure."@en ;
    rdfs:isDefinedBy <> ;
    rdfs:subClassOf [ a owl:Restriction ;
            owl:onClass <Manufacturer> ;
            owl:onProperty <manufacturer> ;
            owl:qualifiedCardinality "1"^^xsd:nonNegativeInteger ] ;
    ns1:term_status "stable" .

ns2:Concept a owl:Class ;
    rdfs:label "Concept"@en ;
    rdfs:isDefinedBy <http://www.w3.org/2004/02/skos/core> ;
    owl:disjointWith ns2:ConceptScheme ;
    ns2:definition "An idea or notion; a unit of thought."@en .

<SubsetWithCommonCharacteristics> a owl:Class ;
    rdfs:label "Subset with common characteristics"@en ;
    dcterms:created "2022-11-04"^^xsd:date ;
    dcterms:modified "2023-03-14"^^xsd:date ;
    rdfs:comment "Subset of items shared by sections of lines and/or operational points of a member state. For the purposes of the register of infrastructure, each infrastructure manager shall describe its railway network at least by sections of line and operational points and optionally via common characteristic subsets."@en ;
    rdfs:isDefinedBy <> ;
    ns1:term_status "stable" .

<Track> a owl:Class ;
    rdfs:label "Track"@en ;
    <rinfIndex> "1.1.1" ;
    dcterms:created "2020-07-29"^^xsd:date ;
    dcterms:modified "2022-07-07"^^xsd:date ;
    rdfs:comment "A running track that is used for train service movements."@en ;
    rdfs:isDefinedBy <> ;
    rdfs:seeAlso <https://wiki3.railml.org/DataModel/3.2/IS/EARoot/EA400.htm> ;
    rdfs:subClassOf <InfrastructureObject> ;
    ns1:term_status "stable" .

<> a owl:Ontology ;
    rdfs:label "ERA Ontology"@en ;
    ns4:license <https://creativecommons.org/licenses/by/4.0/> ;
    ns3:contributor "Dragos Patru, (ERA)",
        "Ghislain Atemezing, (ERA)",
        "Maarten Duhoux, (ERA)",
        "Marina Aguado, (ERA)",
        "Polymnia Vasilopoulou, (ERA)" ;
    ns3:creator "Edna Ruckhaus, (UPM)",
        "Oscar Corcho, (UPM)" ;
    dcterms:issued "2020-07-29"^^xsd:date ;
    dcterms:modified "2024-06-18"^^xsd:date ;
    dcterms:publisher "European Union Agency for Railways" ;
    dcterms:title "ERA Ontology"@en ;
    rdfs:comment """This is the human and machine readable Ontology governed by the European Union Agency for Railways (https://www.era.europa.eu/). It represents the concepts and relationships linked to the sectorial legal framework and the use cases under the Agency´s remit, as described in the Commission Implementing Regulation (EU) [to be updated after publication] on the common specifications for the register of railway infrastructure [to be updated after publication].

Currently, this Ontology covers the European railway infrastructure and the vehicles types authorized to operate over it. It is a semantic/browsable representation of the RINF application guide (https://www.era.europa.eu/sites/default/files/registers/docs/rinf_application_guide_for_register_en.pdf) and ERATV application guide (https://www.era.europa.eu/sites/default/files/registers/docs/iu-eratv_application_guide_for_register_2016-797_en.pdf) that were built by domain experts in the RINF and ERATV working parties.

The Ontology also includes the routebook concepts described in appendix D2 "Elements the infrastructure manager has to provide to the railway undertaking for the Route Book" as presented in the Commission Implementing Regulation (EU) [to be updated after publication] 2019/773 of 16 May 2019 on the technical specification for interoperability relating to the operation and traffic management subsystem of the rail system within the European Union and [to be updated after publication] and the Appendix D3 [to be updated after publication]."""@en ;
    owl:imports <http://www.opengis.net/ont/geosparql#> ;
    owl:priorVersion <https://github.com/Interoperable-data/ERA_vocabulary/releases/tag/v3.0.0> ;
    owl:versionInfo "v3.0.1"@en ;
    owl:versionURI <https://github.com/Interoperable-data/ERA_vocabulary/releases/tag/v3.0.1> ;
    ns2:changeNote """Following changes in this release:
1. Added four subproperties of length: lengthOfSectionOfLine, lengthOfPlatform, lengthOfSiding, lengthOfTunnel
2. Added unit of measure annotation property, annotate corresponding parameters
3. Changed in all of the documentation, "Vocabulary" to "Ontology:
4. Added TSI existence and compliances SKOS (instead of a single TSI compliances
SKOS). For properties TSIMagneticFields 1.1.1.3.9.1 and TSITractionHarmonics
1.1.1.3.9.2.
5. Updated all data properties that point to reference documents (properties are
now object properties that point to the class Document).
6. Thorough review of latest legal text. Updated labels and definitions in order to
be aligned with legal text
7. Refactored properties that are comprised of several parts into a Class and its
properties: PhaseInfo 1.1.1.2.4.1.2, SystemSeparationInfo 1.1.1.2.4.2.2,
8. Changed definition canonical URI. Add annotation property hashSource for
canonical URIs. Modify properties hasAbstraction and hasImplementation no
more inverses.
9. Updated data properties 1.1.1.1.8.3 and 1.1.1.1.8.4., tunnel Start and tunnel
End. Changed to object properties that point to the class LineReference
(kilometer with respect to line)
10. Renamed class and property Platform to PlatformEdge to correctly denote the
concept, i.e. now a plaform with two edges will have two instances instead of
one, each one with its own length.
11. Changed label and definition of property Not yet available to Not provided
12. Added RINF indexes to classes according to RINF hierarchy
13. Added annotation property isUsedInRCCCalculations, annotated corresponding
parameters
14. Refactored properties that are comprised of several parts into a Class and its properties: 1.1.1.3.7.1.4 French train detection system limitation, 1.2.2.0.3.3 minimum radius of vertical curve, ERATV property maximum speed and cant deficiency.
15. Included company properties: schema:url, foaf:name, foaf:nick, companyCodeCategory, org:identifier"""@en .

